###############################################################
##                                                           ##
##  PHYSICALISTIC INTERPRETATION OF MODELLING & SIMULATION:  ##
##         INTEROPERABILITY INFRASTRUCTURE (PIMS-II)         ##
##                                                           ##
##                      VERSION II.1.12a                     ##
##                      DATED 2023-05-04                     ##
##                                                           ##
##   INNOVATIONSZENTRUM FÜR PROZESSDATENTECHNIK (INPRODAT)   ##
##                                                           ##
###############################################################

@base <http://www.molmod.info/semantics/pims-ii.ttl>.
@prefix pims-ii: <http://www.molmod.info/semantics/pims-ii.ttl#>.

@prefix dcelem: <http://purl.org/dc/elements/1.1/>.
@prefix dcterms: <http://purl.org/dc/terms/>.
@prefix owl: <http://www.w3.org/2002/07/owl#>.
@prefix rdf: <http://www.w3.org/1999/02/22-rdf-syntax-ns#>.
@prefix rdfs: <http://www.w3.org/2000/01/rdf-schema#>.
@prefix schema: <http://schema.org/>.
@prefix skos: <http://www.w3.org/2004/02/skos/core#>.
@prefix vann: <http://purl.org/vocab/vann/>.
@prefix xs: <http://www.w3.org/2001/XMLSchema#>.

<http://www.molmod.info/semantics/pims-ii.ttl> a owl:Ontology;
   owl:versionIRI <http://www.molmod.info/semantics/pims-ii/II.1.12a/>;
   dcterms:title "Physicalistic Interpretation of Modelling and Simulation - Interoperability Infrastructure (PIMS-II)"^^xs:string;
   owl:versionInfo "PIMS-II version II.1.12a"^^xs:string;
   dcterms:created "2023-05-04"^^xs:date;
   dcterms:issued "2023-05-04"^^xs:date;
   dcterms:publisher "Innovation Centre for Process Data Technology (Inprodat e.V.)"^^xs:string;
   dcterms:license "https://www.gnu.org/licenses/lgpl-3.0.en.html"^^xs:string;
   dcterms:creator "Martin Thomas Horsch (ORCID 0000-0002-9464-6739)"^^xs:string;
   dcterms:references <http://www.molmod.info/semantics/pims-ii-latex-symbols.tex>;
   vann:preferredNamespacePrefix "pims-ii"^^xs:string;
   vann:preferredNamespaceUri "http://www.molmod.info/semantics/pims-ii.ttl#"^^xs:string;
   dcelem:description "The Physicalistic Interpretation of Modelling and Simulation - Interoperability Infrastructure (PIMS-II) is a mid-level ontology with a focus on documenting cognitive processes and epistemic metadata"@en;
   dcterms:bibliographicCitation "Cite this vocabulary as: M. T. Horsch, PIMS-II ontology, http://www.molmod.info/semantics/pims-ii/, version II.1.12a, 2023. Also reference at least one the following papers: (a) http://ceur-ws.org/Vol-2969/paper3-FOUST.pdf (b) http://ceur-ws.org/Vol-3249/paper2-CAOS.pdf"@en.

##############################
# TOP CONCEPTS AND RELATIONS #
##############################

pims-ii:Object a owl:Class;
   rdfs:label "Object"@en;
   rdfs:subClassOf [
      a owl:Restriction;
      owl:onProperty pims-ii:hasProperPart;
      owl:someValuesFrom pims-ii:Object
   ], [
      a owl:Restriction;
      owl:onProperty pims-ii:isSpatiotemporallyDisconnectedFrom;
      owl:someValuesFrom pims-ii:Object
   ], [
      a owl:Restriction;
      owl:onProperty pims-ii:temporallyPrecedes;
      owl:someValuesFrom pims-ii:Object
   ], [
      a owl:Restriction;
      owl:onProperty [owl:inverseOf pims-ii:temporallyPrecedes];
      owl:someValuesFrom pims-ii:Object
   ];
   owl:equivalentClass [
      a owl:Restriction;
      owl:onProperty pims-ii:isProperPartOf;
      owl:someValuesFrom pims-ii:Object
   ];
   owl:disjointUnionOf (pims-ii:Item pims-ii:MereotopologicalCollective);
   rdfs:comment "Object (PIMS-II top class) = cognizable entity"@en;
   skos:scopeNote "following Peirce, all that exists is regarded as cognizable, i.e., all in principle be referred to by a sign, hence the label 'Object'"@en.

pims-ii:Collective a owl:Class;
   rdfs:label "Collective"@en;
   rdfs:subClassOf pims-ii:Object, [
      a owl:Restriction;
      owl:onProperty [owl:inverseOf pims-ii:isMemberOf];
      owl:minCardinality 2
   ];
   owl:equivalentClass [
      a owl:Restriction;
      owl:onProperty [owl:inverseOf pims-ii:isMemberOf];
      owl:someValuesFrom pims-ii:Object
   ];
   owl:unionOf (pims-ii:MereotopologicalCollective pims-ii:SemioticCollective);
   rdfs:comment "Collective, i.e., an object that has multiple items as members"@en.

pims-ii:isMereosemioticallyRelatedTo a owl:ObjectProperty, owl:ReflexiveProperty, owl:SymmetricProperty, owl:TransitiveProperty;
   rdfs:label "isMereosemioticallyRelatedTo"@en;
   rdfs:comment "Top mereosemiotic relation: Direct or indirect connection through mereotopological and semiotic relations"@en.

pims-ii:isMemberOf a owl:ObjectProperty;
   rdfs:label "isMemberOf"@en;
   skos:altLabel "\\leq"@en;
   rdfs:range pims-ii:Collective;
   rdfs:subPropertyOf pims-ii:isProperPartOf, pims-ii:isConstitutiveOf;
   rdfs:comment "membership relation, i.e., relation between an item/member and a collective"@en.

###########################################
# MEREOTOPOLOGY: CONCEPTS AND INDIVIDUALS #
###########################################

pims-ii:MereotopologicalCollective a owl:Class;
   rdfs:label "MereotopologicalCollective"@en;
   rdfs:subClassOf pims-ii:Collective, [
      a owl:Restriction;
      owl:onProperty [owl:inverseOf pims-ii:isMereotopologicalMemberOf];
      owl:minCardinality 2
   ];
   owl:equivalentClass [
      a owl:Restriction;
      owl:onProperty [owl:inverseOf pims-ii:isMereotopologicalMemberOf];
      owl:someValuesFrom pims-ii:Item
   ];
   rdfs:comment "Mereotopological collective, i.e., a region of spacetime that consists of multiple connected components, which are its mereotopological members"@en.

pims-ii:Item a owl:Class;
   rdfs:label "Item"@en;
   rdfs:subClassOf pims-ii:Object;
   #
   # negative statement commented out to support SROIQ(D) compliance for domain ontologies situated below PIMS-II
   #
   # owl:intersectionOf (
   # pims-ii:Object [
   #       a owl:Restriction;
   #       owl:onProperty [owl:inverseOf pims-ii:isMereotopologicalMemberOf];
   #       owl:cardinality 0
   #    ]
   # );
   #
   rdfs:comment "Item, i.e., a connected region of spacetime that does not consist of multiple connected components"@en;
   skos:scopeNote "Alternative definition: An item is an object that cannot be split into two spatiotemporally disconnected parts"@en.

pims-ii:Process a owl:Class;
   rdfs:label "Process"@en;
   rdfs:subClassOf pims-ii:Item;
   owl:equivalentClass [
      a owl:Restriction;
      owl:onProperty [owl:inverseOf pims-ii:isParticipantIn];
      owl:someValuesFrom pims-ii:Object
   ];
   rdfs:comment "Process, i.e., a connected region that has at least one participant, an entity with which it overlaps spatiotemporally and that plays a certain role in the process"@en;
   skos:scopeNote "n.b., 'participation' here does not imply agency, anything that somehow plays a role in the process, and does so by virtue of overlapping with it spatiotemporally, is a participant in it"@en.

############################
# MEREOTOPOLOGY: RELATIONS #
############################

pims-ii:directlyPrecedesStep a owl:ObjectProperty;
   rdfs:label "directlyPrecedesStep"@en;
   skos:altLabel "\\ddot\\hookrightarrow"@en;
   rdfs:domain pims-ii:Process;
   rdfs:range pims-ii:Process;
   rdfs:subPropertyOf pims-ii:precedesStep, pims-ii:hasDirectCausalConnectionWith;
   rdfs:comment "(x directlyPrecedesStep y) means that x and y are processes such that y can commence when x (and possibly other steps that also directly precede y) has finished"@en;
   skos:scopeNote "(x directlyPrecedesStep y) implies that there is a direct causal connection between x and y"@en.

pims-ii:doesNotOverlapWith a owl:ObjectProperty, owl:SymmetricProperty;
   rdfs:label "doesNotOverlapWith"@en;
   skos:altLabel "\\lnot(\\dot{P}^-\\dot{P})"@en;
   rdfs:subPropertyOf pims-ii:isMereosemioticallyRelatedTo;
   rdfs:comment "(x doesNotOverlapWith y) is the negation of (x overlapsWith y); i.e., the spatiotemporal intersection of x and y is empty"@en.

pims-ii:doesNotTemporallyOverlapWith a owl:ObjectProperty, owl:SymmetricProperty;
   rdfs:label "doesNotTemporallyOverlapWith"@en;
   skos:altLabel "\\lnot(\\equiv_t\\dot{P}^-\\dot{P})"@en;
   rdfs:subPropertyOf pims-ii:doesNotOverlapWith;
   rdfs:comment "(x doesNotTemporallyOverlapWith y) is the negation of (x temporallyOverlapsWith y); i.e., there is no temporal overlap between x and y"@en.

pims-ii:hasImproperPart a owl:ObjectProperty, owl:ReflexiveProperty, owl:TransitiveProperty;
   rdfs:label "hasImproperPart"@en;
   rdfs:subPropertyOf pims-ii:overlapsWith;
   owl:inverseOf pims-ii:isImproperPartOf;
   rdfs:comment "Spatiotemporal (mereological) improper parthood relation; in other words, it is the reflexive closure of proper parthood: (x hasImproperPart y) means that all points within y are also within x"^^xs:string.

pims-ii:hasProperPart a owl:ObjectProperty, owl:TransitiveProperty;
   rdfs:label "hasProperPart"@en;
   skos:altLabel "\\dot{P}^-"@en;
   rdfs:subPropertyOf pims-ii:hasImproperPart;
   owl:inverseOf pims-ii:isProperPartOf;
   rdfs:comment "(x hasProperPart y) means that y is an improper part of x such that x and y are not the same, in other words, all points within y are also within x, but not vice versa"@en;
   skos:scopeNote "Spatiotemporal (mereological) proper parthood relation"@en.

pims-ii:isInitialStepIn a owl:ObjectProperty;
   rdfs:label "isInitialStepIn"@en;
   rdfs:domain pims-ii:Process;
   #
   # negative statement commented out to support SROIQ(D) compliance for domain ontologies situated below PIMS-II
   #
   # rdfs:domain [
   #    a owl:Restriction;
   #    owl:onProperty [owl:inverseOf pims-ii:directlyPrecedesStep];
   #    owl:cardinality 0
   # ];
   #
   rdfs:range pims-ii:Process;
   rdfs:subPropertyOf pims-ii:isStepIn;
   rdfs:comment "(x isInitialStepIn y) means that y is a step in x (i.e., a subprocess of x) that is not preceded by any other step"^^xs:string.

pims-ii:isImproperPartOf a owl:ObjectProperty, owl:ReflexiveProperty, owl:TransitiveProperty;
   rdfs:label "isImproperPartOf"@en;
   skos:altLabel "P";
   rdfs:subPropertyOf pims-ii:overlapsWith;
   owl:inverseOf pims-ii:hasImproperPart;
   rdfs:comment "Spatiotemporal (mereological) improper parthood relation; in other words, it is the reflexive closure of proper parthood: (x isImproperPartOf y) means that all points within x are also within y"@en.

pims-ii:isMereotopologicalMemberOf a owl:ObjectProperty;
   rdfs:label "isMereotopologicalMemberOf"@en;
   rdfs:domain pims-ii:Item;
   rdfs:range pims-ii:MereotopologicalCollective;
   rdfs:subPropertyOf pims-ii:isMemberOf, pims-ii:isMereologicallyConstitutiveOf;
   rdfs:comment "(x isMereotopologicalMemberOf y) means that x is one out of several mereotopologically connected components of y"^^xs:string.

pims-ii:isParticipantIn a owl:ObjectProperty;
   rdfs:label "isParticipantIn"@en;
   rdfs:range pims-ii:Process;
   rdfs:subPropertyOf pims-ii:overlapsWith, pims-ii:hasDirectCausalConnectionWith;
   rdfs:comment "(x isParticipantIn y) means that y is a process in which x plays a certain role (e.g., x is a well-defined step within y, or x is an object that undergoes some change within y, or x is a sign that is read or an object that is perceived within y); this requires a spatiotemporal overlap between x and y"^^xs:string.

pims-ii:isProperPartOf a owl:ObjectProperty, owl:TransitiveProperty;
   rdfs:label "isProperPartOf"@en;
   rdfs:subPropertyOf pims-ii:isImproperPartOf, pims-ii:isTemporallyIncludedIn;
   owl:inverseOf pims-ii:hasProperPart;
   owl:propertyChainAxiom (pims-ii:isOldReferentInPartToWhole [owl:inverseOf pims-ii:isNewReferentInPartToWhole]);
   owl:propertyChainAxiom (pims-ii:isNewReferentInWholeToPart [owl:inverseOf pims-ii:isOldReferentInWholeToPart]);
   rdfs:comment "Spatiotemporal (mereological) proper parthood relation; (x isProperPartOf y) means that x is an improper part of y such that x and y are not the same, in other words, all points within x are also within y, but not vice versa"^^xs:string.

pims-ii:isProperParticipantIn a owl:ObjectProperty;
   rdfs:label "isProperParticipantIn"@en;
   rdfs:range pims-ii:Process;
   rdfs:subPropertyOf pims-ii:isProperPartOf, pims-ii:isParticipantIn;
   rdfs:comment "(x isProperParticipantIn y) is the conjunction of (x isProperPartOf y) and (x isParticipantIn y)"^^xs:string.

pims-ii:isSpatiotemporallyConnectedWith a owl:ObjectProperty, owl:ReflexiveProperty, owl:SymmetricProperty;
   rdfs:label "isSpatiotemporallyConnectedWith"@en;
   rdfs:subPropertyOf pims-ii:isTemporallyConnectedWith;
   owl:propertyChainAxiom (pims-ii:hasImproperPart pims-ii:isSpatiotemporallyConnectedWith);
   rdfs:comment "(x isSpatiotemporallyConnectedWith y) means that x and y overlap or are directly adjacent to each other at some point; i.e., there is a point p_x in x and a point p_y in y such that you can go from p_x to p_y without ever leaving the fusion (x U y)"^^xs:string.

pims-ii:isSpatiotemporallyDisconnectedFrom a owl:ObjectProperty, owl:SymmetricProperty;
   rdfs:label "isSpatiotemporallyDisconnectedFrom"@en;
   rdfs:subPropertyOf pims-ii:doesNotOverlapWith;
   rdfs:comment "(x isSpatiotemporallyDisconnectedFrom y) is the negation of (x isSpatiotemporallyConnectedWith y); i.e., to go from any point in x to any point in y, it is necessary to leave the fusion (x U y)"^^xs:string.

pims-ii:isStepIn a owl:ObjectProperty;
   rdfs:label "isStepIn"@en;
   rdfs:domain pims-ii:Process;
   rdfs:range pims-ii:Process, [
      a owl:Restriction;
      owl:onProperty [owl:inverseOf pims-ii:isInitialStepIn];
      owl:someValuesFrom pims-ii:Process
   ], [
      a owl:Restriction;
      owl:onProperty [owl:inverseOf pims-ii:isTerminalStepIn];
      owl:someValuesFrom pims-ii:Process
   ];
   rdfs:subPropertyOf pims-ii:isProperParticipantIn;
   rdfs:comment "(x isStepIn y) means that x and y are processes, where x is a proper part of y that plays a well-defined role within y (e.g., a task within a project, the execution of a single command within the execution of a program, etc.)"^^xs:string.

pims-ii:isTemporallyConnectedWith a owl:ObjectProperty, owl:ReflexiveProperty, owl:SymmetricProperty;
   rdfs:label "isTemporallyConnectedWith"@en;
   rdfs:subPropertyOf pims-ii:isMereosemioticallyRelatedTo;
   owl:propertyChainAxiom (pims-ii:isSpatiotemporallyConnectedWith pims-ii:temporallyCoextendsWith);
   owl:propertyChainAxiom (pims-ii:temporallyCoextendsWith pims-ii:isSpatiotemporallyConnectedWith);
   rdfs:comment "(x isTemporallyConnectedWith y) means that there is a point in time where both x and y exist"^^xs:string.

pims-ii:isTerminalStepIn a owl:ObjectProperty;
   rdfs:label "isTerminalStepIn"@en;
   rdfs:domain pims-ii:Process;
   #
   # negative statement commented out to support SROIQ(D) compliance for domain ontologies situated below PIMS-II
   #
   # rdfs:domain [
   #    a owl:Restriction;
   #    owl:onProperty pims-ii:directlyPrecedesStep;
   #    owl:cardinality 0
   # ];
   #
   rdfs:range pims-ii:Process;
   rdfs:subPropertyOf pims-ii:isStepIn;
   rdfs:comment "(x isTerminalStepIn y) means that y is a step in x (i.e., a subprocess of x) that does not precede any other step"^^xs:string.

pims-ii:overlapsWith a owl:ObjectProperty, owl:ReflexiveProperty, owl:SymmetricProperty;
   rdfs:label "overlapsWith"@en;
   rdfs:subPropertyOf pims-ii:isSpatiotemporallyConnectedWith, pims-ii:temporallyOverlapsWith;
   owl:propertyChainAxiom (pims-ii:hasImproperPart pims-ii:isImproperPartOf);
   rdfs:comment "(x overlapsWith y) means that x and y share a spatiotemporal region where x and y intersect"^^xs:string.

pims-ii:precedesStep a owl:ObjectProperty, owl:TransitiveProperty;
   rdfs:label "precedesStep"@en;
   rdfs:domain pims-ii:Process;
   rdfs:range pims-ii:Process;
   rdfs:subPropertyOf pims-ii:temporallyPrecedes, pims-ii:hasCausalConnectionWith;
   rdfs:comment "'precedesStep' is the transitive closure of 'directlyPrecedesStep'; (x precedesStep y) means that the processes x and y are, possibly indirectly, causally connected such that x needs to be concluded before y can commence"^^xs:string.

pims-ii:temporallyCoextendsWith a owl:ObjectProperty, owl:ReflexiveProperty, owl:SymmetricProperty, owl:TransitiveProperty;
   rdfs:label "temporallyCoextendsWith"@en;
   rdfs:subPropertyOf pims-ii:temporallyOverlapsWith;
   rdfs:comment "(x temporallyCoextendsWith y) means that x and y have exactly the same extension in time, i.e., disregarding their spatial extension"^^xs:string.

pims-ii:isTemporallyIncludedIn a owl:ObjectProperty, owl:TransitiveProperty;
   rdfs:label "isTemporallyIncludedIn"@en;
   rdfs:subPropertyOf pims-ii:temporallyOverlapsWith;
   owl:propertyChainAxiom (pims-ii:isProperPartOf pims-ii:temporallyCoextendsWith);
   owl:propertyChainAxiom (pims-ii:temporallyCoextendsWith pims-ii:isProperPartOf);
   rdfs:comment "(x isTemporallyIncludedIn y) means that the temporal extension of x is a proper part of the temporal extension of y"^^xs:string.

pims-ii:temporallyOverlapsWith a owl:ObjectProperty, owl:ReflexiveProperty, owl:SymmetricProperty;
   rdfs:label "temporallyOverlapsWith"@en;
   rdfs:subPropertyOf pims-ii:isTemporallyConnectedWith;
   owl:propertyChainAxiom (pims-ii:overlapsWith pims-ii:temporallyCoextendsWith);
   owl:propertyChainAxiom (pims-ii:temporallyCoextendsWith pims-ii:overlapsWith);
   rdfs:comment "(x temporallyOverlapsWith y) means that there is an (extended) interval in time where both x and y exist"^^xs:string.

pims-ii:temporallyPrecedes a owl:ObjectProperty, owl:TransitiveProperty;
   rdfs:label "temporallyPrecedes"@en;
   rdfs:subPropertyOf pims-ii:doesNotTemporallyOverlapWith;
   owl:propertyChainAxiom (pims-ii:temporallyPrecedes pims-ii:hasProperPart);
   owl:propertyChainAxiom (pims-ii:isProperPartOf pims-ii:temporallyPrecedes);
   owl:propertyChainAxiom (pims-ii:temporallyPrecedes pims-ii:temporallyCoextendsWith);
   owl:propertyChainAxiom (pims-ii:temporallyCoextendsWith pims-ii:temporallyPrecedes);
   rdfs:comment "(x temporallyPrecedes y) means that every point in x is earlier in time than every point in y; the spacetime regions x and y may be connected, but they cannot overlap temporally"^^xs:string.

#################################
# CORE MEREOSEMIOTICS: CONCEPTS #
#################################

pims-ii:Accumulation a owl:Class;
   rdfs:label "Accumulation"@en;
   rdfs:subClassOf pims-ii:InformationProcessing, [
      a owl:Restriction;
      owl:onProperty [owl:inverseOf pims-ii:isAccumulationInputIn];
      owl:someValuesFrom pims-ii:Object
   ], [
      a owl:Restriction;
      owl:onProperty [owl:inverseOf pims-ii:isObjectInAccumulation];
      owl:someValuesFrom pims-ii:Object
   ], [
      a owl:Restriction;
      owl:onProperty [owl:inverseOf pims-ii:isAccumulationOutputIn];
      owl:someValuesFrom pims-ii:Object
   ], [
      a owl:Restriction;
      owl:onProperty [owl:inverseOf pims-ii:isIncludedInAccumulation];
      owl:someValuesFrom pims-ii:Object
   ];
   rdfs:comment "Accumulation, i.e., an information-processing step in which the given information is extended/complemented such that the input (sign) and one or multiple additional representamina (cf. relation isIncludedInAccumulation) are jointly constitutive of the output (interpretant); this includes conditional accumulation, where the choice and the way in which information is combined depends on an accumulation condition (cf. relation isAccumulationConditionIn)"^^xs:string.

pims-ii:Articulation a owl:Class;
   rdfs:label "Articulation"@en;
   skos:altLabel "AN"@en;
   rdfs:subClassOf pims-ii:SemioticCollective, [
      a owl:Restriction;
      owl:onProperty [owl:inverseOf pims-ii:realizes];
      owl:minCardinality 2
   ];
   owl:equivalentClass [
      a owl:Restriction;
      owl:onProperty [owl:inverseOf pims-ii:realizes];
      owl:someValuesFrom [owl:complementOf pims-ii:SemioticCollective]
   ];
   owl:disjointWith [
      a owl:Restriction;
      owl:onProperty [owl:inverseOf pims-ii:isSemioticMemberOf];
      owl:someValuesFrom pims-ii:SemioticCollective
   ];
   rdfs:comment "Articulation (collective expression), i.e., a semiotic collective the semiotic members (i.e., realizations) of which are not semiotic collectives, but individual literal (written or digital) or non-literal (e.g., spoken) items with the same semiotic function (or undergoing evaluation whether such a function is present)"^^xs:string.

pims-ii:Assessment a owl:Class;
   rdfs:label "Assessment"@en;
   rdfs:subClassOf pims-ii:Ground;
   owl:equivalentClass [
      a owl:Restriction;
      owl:onProperty pims-ii:isAssessmentFor;
      owl:someValuesFrom pims-ii:CognitiveStep
   ];
   rdfs:comment "Assessment (of a cognitive step), i.e., a ground that provides an explanation including a proposition on the extent (quantitatively or qualitatively) to which the grounded cognitive step is reliable/accurate/valid (or similar), why that is the case, and how that relates to the reliability/accuracy/etc. of the preceding step"^^xs:string.

pims-ii:Assignment a owl:Class;
   rdfs:label "Assignment"@en;
   skos:altLabel "ASG"@en;
   rdfs:subClassOf pims-ii:DigitalConventional, pims-ii:EqualityArticulation, [
      a owl:Restriction;
      owl:onProperty [owl:inverseOf pims-ii:isVariableInAssignment];
      owl:someValuesFrom pims-ii:Variable
   ], [
      a owl:Restriction;
      owl:onProperty [owl:inverseOf pims-ii:isValueInAssignment];
      owl:someValuesFrom pims-ii:Value
   ], [
      a owl:Restriction;
      owl:onProperty pims-ii:isAssignmentFor;
      owl:someValuesFrom pims-ii:Object
   ];
   rdfs:comment "Assignment, i.e., an equality articulation by which a value is assigned to a variable with respect to a particular referent (e.g., T = 200 K for substance o as it was measured in a particular cognitive step); therein, T is the variable, related to the assignment by [inverseOf isVariableInAssignment], 200 K is the value, related to the assignment by [inverseOf isValueInAssignment], and o is the referent, related to the assignment by isAssignmentFor"^^xs:string.

pims-ii:BasicGround a owl:Class;
   rdfs:label "BasicGround"@en;
   rdfs:subClassOf pims-ii:Ground, [
      a owl:Restriction;
      owl:onProperty pims-ii:isGroundFor;
      owl:allValuesFrom pims-ii:Presupposition
   ];
   rdfs:comment "Basic ground, i.e., a ground that is assumed to be valid and reliable a priori; a cognitive step for which there is a basic ground is a presupposition"@en.

pims-ii:CanonicalTUCAN a owl:Class;
   rdfs:label "CanonicalTUCAN"@en;
   rdfs:subClassOf pims-ii:MaterialIdentifier;
   rdfs:comment "Canonical TUCAN, i.e., the material identifier as developed within the NFDI4Chem project"@en.

pims-ii:Claim a owl:Class;
   rdfs:label "Claim"@en;
   rdfs:subClassOf pims-ii:Proposition;
   owl:equivalentClass [owl:intersectionOf
      (
         pims-ii:Proposition
         [
            owl:unionOf ( [
                  a owl:Restriction;
                  owl:onProperty pims-ii:isAssertedBy;
                  owl:someValuesFrom pims-ii:Interlocutor
               ] [
                  a owl:Restriction;
                  owl:onProperty pims-ii:isClaimOf;
                  owl:someValuesFrom pims-ii:IntelligentAgent
               ]
            )
         ]
      )
   ];
   rdfs:comment "Claim, i.e., a proposition that is expressed by an interlocutor or believed/held by an intelligent agent"^^xs:string.

pims-ii:Cognition a owl:Class;
   rdfs:label "Cognition"@en;
   rdfs:subClassOf pims-ii:Process;
   owl:unionOf (pims-ii:CognitiveStep pims-ii:CognitiveChain);
   rdfs:comment "Cognition, i.e., a process dealing with representamina (signs) consisting either of a single cognitive step, of multiple steps that are connected to each other as a cognitive chain, or of an anchor point for epistemic grounding"^^xs:string.

pims-ii:CognitiveChain a owl:Class;
   rdfs:label "CognitiveChain"@en;
   rdfs:subClassOf pims-ii:Cognition, [
      a owl:Restriction;
      owl:onProperty [owl:inverseOf pims-ii:isStepInCognitiveChain];
      owl:minCardinality 2
   ];
   rdfs:comment "Cognitive chain, i.e., a cognition that consists of multiple (sub)steps"^^xs:string.

pims-ii:CognitiveRupture a owl:Class;
   rdfs:label "CognitiveRupture"@en;
   rdfs:subClassOf pims-ii:CognitiveStep;
   #
   # negative statement commented out to support SROIQ(D) compliance for domain ontologies situated below PIMS-II
   #
   # rdfs:subClassOf [
   #    a owl:Restriction;
   #    owl:onProperty pims-ii:directlyGrounds;
   #    owl:cardinality 0
   # ];
   #
   rdfs:comment "Cognitive rupture, i.e., a cognitive step that constitutes a break in the chain of epistemic grounding"^^xs:string.

pims-ii:CognitiveStep a owl:Class;
   rdfs:label "CognitiveStep"@en;
   rdfs:subClassOf pims-ii:Cognition;
   owl:disjointUnionOf (pims-ii:CognitiveRupture pims-ii:Metonymization pims-ii:Presupposition pims-ii:Semiosis);
   rdfs:comment "Cognitive step, i.e., an elementary cognition that can form an part of a cognitive chain"^^xs:string.

pims-ii:CollectiveLiteral a owl:Class;
   rdfs:label "CollectiveLiteral"@en;
   rdfs:subClassOf pims-ii:Articulation;
   owl:equivalentClass [
      a owl:Restriction;
      owl:onProperty pims-ii:isLiterally;
      owl:minCardinality 1
   ];
   owl:disjointWith pims-ii:CollectiveUtterance;
   rdfs:comment "Collective literal, i.e., a semiotic collective the members of which all have a digital, printed, or written textual/numerical form in that they are all instances/copies of the same RDFS literal (or multiple RDFS literals that are very similar, e.g., different ways of spelling/abbreviating the same word or denoting the same number); n.b., collective literals are not permitted to have other semiotic collectives as their semiotic members"^^xs:string.
pims-ii:isLiterally a owl:DatatypeProperty;
   rdfs:label "isLiterally"@en;
   rdfs:domain pims-ii:CollectiveLiteral;
   rdfs:comment "points to the expression of a collective literal as an RDFS literal (e.g., xs:string or xs:decimal)"^^xs:string.

pims-ii:CollectiveUtterance a owl:Class;
   rdfs:label "CollectiveUtterance"@en;
   rdfs:subClassOf pims-ii:Articulation;
   owl:disjointWith pims-ii:CollectiveLiteral;
   rdfs:comment "Collective utterance, i.e., a semiotic collective the members of which do not have digital, printed, or written textual/numerical form and the members of which are all attributed the same semantics and pragmatics; n.b., collective utterances are not permitted to have other semiotic collectives as their semiotic members"^^xs:string.

pims-ii:ConceptualIRI a owl:Class;
   rdfs:label "ConceptualIRI"@en;
   rdfs:subClassOf pims-ii:IRI;
   owl:disjointWith pims-ii:RelationalIRI;
   rdfs:comment "Conceptual IRI, i.e., the internationalized resource identifier of a concept (i.e., of an owl:Class)"^^xs:string.

pims-ii:Conventional a owl:Class;
   rdfs:label "Conventional"@en;
   skos:altLabel "CV"@en;
   rdfs:subClassOf pims-ii:Articulation, [
      a owl:Restriction;
      owl:onProperty pims-ii:isRepresentamenFor;
      owl:someValuesFrom pims-ii:Object
   ];
   rdfs:comment "Conventional, i.e., a semiotic collective articulation the members of which jointly fulfill a certain semiotic function by social convention; e.g., many spoken or written occurrences of the words 'enthalpy of vaporization' or 'latent heat' may act together as a property in this sense"^^xs:string.

pims-ii:DataItem a owl:Class;
   rdfs:label "DataItem"@en;
   skos:altLabel "DI"@en;
   rdfs:subClassOf pims-ii:DigitalArticulation, [
      a owl:Restriction;
      owl:onProperty [owl:inverseOf pims-ii:isSemioticallyConstitutiveOf];
      owl:minQualifiedCardinality 2;
      owl:onClass pims-ii:DigitalConventional
   ];
   rdfs:comment "Data item, i.e., a digital articulation given as a tuple of digital conventionals"@en;
   skos:example "e.g., a key-value dyad with a left-hand side and a right-hand side"@en.

pims-ii:Dataset a owl:Class;
   rdfs:label "Dataset"@en;
   rdfs:subClassOf pims-ii:DigitalArticulation, [
      a owl:Restriction;
      owl:onProperty [owl:inverseOf pims-ii:isSemioticallyConstitutiveOf];
      owl:minQualifiedCardinality 2;
      owl:onClass pims-ii:DataItem
   ];
   rdfs:comment "Dataset, i.e., a digital articulation that is composed of multiple data items that are similar in shape, kind, and content type"@en.

pims-ii:DigitalArticulation a owl:Class;
   rdfs:label "DigitalArticulation"@en;
   skos:altLabel "DAN"@en;
   rdfs:subClassOf pims-ii:Articulation, [
      a owl:Restriction;
      owl:onProperty [owl:inverseOf pims-ii:isSemioticallyConstitutiveOf];
      owl:minQualifiedCardinality 2;
      owl:onClass pims-ii:CollectiveLiteral
   ];
   rdfs:comment "Digital articulation, i.e., an articulation the members of which are copies of the same digital content (a file, assignment of a value to a variable, a data set, etc.)"@en.
   
pims-ii:DigitalConventional a owl:Class;
   rdfs:label "DigitalConventional"@en;
   skos:altLabel "DCV"@en;
   rdfs:subClassOf pims-ii:Conventional, pims-ii:DigitalArticulation;
   owl:intersectionOf (pims-ii:Conventional pims-ii:DigitalArticulation);
   rdfs:comment "Digital conventional, i.e., a conventional that is a digital articulation"@en.

pims-ii:Dyad a owl:Class;
   rdfs:label "Dyad"@en;
   rdfs:subClassOf pims-ii:DataItem, [
      a owl:Restriction;
      owl:onProperty [owl:inverseOf pims-ii:isFirstInDyad];
      owl:someValuesFrom pims-ii:DigitalConventional
   ], [
      a owl:Restriction;
      owl:onProperty [owl:inverseOf pims-ii:isSecondInDyad];
      owl:someValuesFrom pims-ii:DigitalConventional
   ];
   rdfs:comment "Dyad, i.e., a data item by which two conventionals are grouped together; e.g., an equality or inequality articulation"^^xs:string.

pims-ii:Duplication a owl:Class;
   rdfs:label "Duplication"@en;
   rdfs:subClassOf pims-ii:InformationProcessing, [
      a owl:Restriction;
      owl:onProperty [owl:inverseOf pims-ii:isOriginalIn];
      owl:someValuesFrom pims-ii:Object
   ], [
      a owl:Restriction;
      owl:onProperty [owl:inverseOf pims-ii:isObjectInDuplication];
      owl:someValuesFrom pims-ii:Object
   ], [
      a owl:Restriction;
      owl:onProperty [owl:inverseOf pims-ii:isDuplicateIn];
      owl:someValuesFrom pims-ii:Object
   ];
   rdfs:comment "Duplication, i.e., an information-processing step in which the given information is reproduced, copied, converted into a different, but equivalent format, or any similar procedure; e.g., this may be based on a legisign to which the original (sign) and the duplicate (interpretant) jointly conform or on a semiotic collective of which they both semiotic members"^^xs:string.

pims-ii:EqualityArticulation a owl:Class;
   rdfs:label "EqualityArticulation"@en;
   skos:altLabel "EAN"@en;
   rdfs:subClassOf pims-ii:Dyad, [
      a owl:Restriction;
      owl:onProperty [owl:inverseOf pims-ii:isLeftHandSideIn];
      owl:someValuesFrom pims-ii:Term
   ], [
      a owl:Restriction;
      owl:onProperty [owl:inverseOf pims-ii:isRightHandSideIn];
      owl:someValuesFrom pims-ii:Term
   ];
   rdfs:comment "Equality articulation, i.e., a dyad by which two terms are asserted to be equal or to become equal"^^xs:string.

pims-ii:Evaluation a owl:Class;
   rdfs:label "Evaluation"@en;
   skos:altLabel "EVA"@en;
   rdfs:subClassOf pims-ii:Telesis, pims-ii:Interpretation, [
      a owl:Restriction;
      owl:onProperty [owl:inverseOf pims-ii:isTelosInEvaluation];
      owl:someValuesFrom pims-ii:Object
   ], [
      a owl:Restriction;
      owl:onProperty [owl:inverseOf pims-ii:isEvaluatedIn];
      owl:someValuesFrom pims-ii:Object
   ], [
      a owl:Restriction;
      owl:onProperty [owl:inverseOf pims-ii:isEvaluationOutcomeIn];
      owl:someValuesFrom pims-ii:Object
   ], [
      a owl:Restriction;
      owl:onProperty [owl:inverseOf pims-ii:directlyGrounds];
      owl:someValuesFrom [owl:unionOf (pims-ii:Telesis pims-ii:Undertaking)]
   ], [
      a owl:Restriction;
      owl:onProperty [owl:inverseOf pims-ii:isEvaluatorIn];
      owl:someValuesFrom [owl:intersectionOf (pims-ii:GoalDirectedAgent pims-ii:Interlocutor)]
   ];
   owl:intersectionOf (pims-ii:Telesis pims-ii:Interpretation);
   rdfs:comment "Evaluation, i.e., a reflection ex post (Reflexion des Vollzugs following Baumann and Tulatz) or redetermination, carried out after an action has terminated, either by the same agent or by somebody else"^^xs:string.

pims-ii:Examination a owl:Class;
   rdfs:label "Examination"@en;
   skos:altLabel "EXA"@en;
   rdfs:subClassOf pims-ii:Observation, [
      a owl:Restriction;
      owl:onProperty [owl:inverseOf pims-ii:isLegisignIn];
      owl:someValuesFrom pims-ii:Object
   ], [
      a owl:Restriction;
      owl:onProperty [owl:inverseOf pims-ii:isExaminedIn];
      owl:someValuesFrom pims-ii:Object
   ], [
      a owl:Restriction;
      owl:onProperty [owl:inverseOf pims-ii:isExaminationOutcomeIn];
      owl:someValuesFrom pims-ii:Object
   ];
   rdfs:comment "Examination (by pattern matching & similar), i.e., an observation by which a legisign (specifying patterns or rules) is applied to an examined object, yielding an examination outcome that expresses in what way or to what extent the object matches the legisign"^^xs:string.

pims-ii:ExperimentalWorkflow a owl:Class;
   rdfs:label "ExperimentalWorkflow"@en;
   rdfs:subClassOf pims-ii:CognitiveWorkflow, [
      a owl:Restriction;
      owl:onProperty [owl:inverseOf pims-ii:isStepInCognitiveChain];
      owl:someValuesFrom pims-ii:Measurement
   ];
   rdfs:comment "experimental workflow, i.e., a cognition that is purposefully conducted in a controlled environment and has at least one measurement as a step"^^xs:string.

pims-ii:Ground a owl:Class;
   rdfs:label "Ground"@en;
   rdfs:subClassOf pims-ii:Proposition;
   owl:equivalentClass [
      a owl:Restriction;
      owl:onProperty pims-ii:isGroundFor;
      owl:someValuesFrom pims-ii:CognitiveStep
   ];
   rdfs:comment "Ground (of a cognitive step), i.e., a proposition that justifies a cognitive step by explaning it and stating from what preceding step (which directly grounds that step) a sign-object relation is carried over, and in what way"^^xs:string.

pims-ii:GroundingChain a owl:Class;
   rdfs:label "GroundingChain"@en;
   rdfs:subClassOf pims-ii:CognitiveChain, [
      a owl:Restriction;
      owl:onProperty [owl:inverseOf pims-ii:isStepInCognitiveChain];
      owl:allValuesFrom [owl:unionOf (pims-ii:GroundingStep pims-ii:Presupposition)]
   ];
   rdfs:comment "Grounding chain, i.e., a cognitive chain that establishes epistemic grounding"^^xs:string.

pims-ii:GroundedCognition a owl:Class;
   rdfs:label "GroundedCognition"@en;
   rdfs:subClassOf pims-ii:Cognition;
   owl:equivalentClass [
      owl:unionOf (
         pims-ii:Presupposition [
            a owl:Restriction;
            owl:onProperty [owl:inverseOf pims-ii:logicallyPrecedes];
            owl:someValuesFrom pims-ii:Presupposition
         ]
      )
   ], [
      a owl:Restriction;
      owl:onProperty [owl:inverseOf pims-ii:isJustificationFor];
      owl:someValuesFrom pims-ii:GroundingChain
   ];
   rdfs:comment "Grounded cognition, i.e., a cognition that is logically preceded by a presupposition such that there is a grounding chain establishing its epistemic status as a grounded cognition"^^xs:string.

pims-ii:GroundingInterpretation a owl:Class;
   rdfs:label "GroundingInterpretation"@en;
   rdfs:subClassOf pims-ii:GroundingStep, pims-ii:Interpretation, [
      a owl:Restriction;
      owl:onProperty [owl:inverseOf pims-ii:groundsPresentStepIn];
      owl:someValuesFrom pims-ii:Object
   ], [
      a owl:Restriction;
      owl:onProperty [owl:inverseOf pims-ii:isPresentStepInGrounding];
      owl:someValuesFrom pims-ii:Object
   ], [
      a owl:Restriction;
      owl:onProperty [owl:inverseOf pims-ii:groundsNextStepIn];
      owl:someValuesFrom pims-ii:Object
   ];
   owl:intersectionOf (pims-ii:GroundingStep pims-ii:Semiosis);
   rdfs:comment "Grounding interpretation, i.e., an interpretation where the sign is a ground for the considered cognitive step, the object is the considered cognitive step, and the interpretant is a ground for a subsequent cognitive step"^^xs:string.

pims-ii:GroundingMetonymization a owl:Class;
   rdfs:label "GroundingMetonymization"@en;
   rdfs:subClassOf pims-ii:GroundingStep, pims-ii:Metonymization, [
      a owl:Restriction;
      owl:onProperty [owl:inverseOf pims-ii:isGroundingStepIn];
      owl:someValuesFrom pims-ii:Object
   ], [
      a owl:Restriction;
      owl:onProperty [owl:inverseOf pims-ii:isGroundingPropositionIn];
      owl:someValuesFrom pims-ii:Object
   ], [
      a owl:Restriction;
      owl:onProperty [owl:inverseOf pims-ii:isGroundedStepIn];
      owl:someValuesFrom pims-ii:Object
   ];
   owl:intersectionOf (pims-ii:GroundingStep pims-ii:SemanticChange);
   rdfs:comment "Grounding metonymization, i.e., a metonymization where a the old referent is a cognitive step (i.e., the grounding step) that grounds another (i.e., the grounded step), which is the new referent; the referent for both is a ground (i.e., the grounding proposition) that is a ground for the grounded step"^^xs:string.

pims-ii:GroundingStep a owl:Class;
   rdfs:label "GroundingStep"@en;
   rdfs:subClassOf pims-ii:TriadicCognition;
   owl:disjointUnionOf (pims-ii:GroundingMetonymization pims-ii:GroundingInterpretation);
   rdfs:comment "Grounding step, i.e., a triadic cognition that establishes epistemic grounding"^^xs:string.

pims-ii:IndividualIRI a owl:Class;
   rdfs:label "IndividualIRI"@en;
   rdfs:subClassOf pims-ii:IRI, pims-ii:UniqueIdentifier;
   owl:disjointWith pims-ii:RelationalIRI;
   rdfs:comment "Individual IRI, i.e., the internationalized resource identifier of an individual (owl:Thing or pims-ii:Object)"^^xs:string.

pims-ii:InformationProcessing a owl:Class;
   rdfs:label "InformationProcessing"@en;
   rdfs:subClassOf pims-ii:Interpretation, [
      a owl:Restriction;
      owl:onProperty [owl:inverseOf pims-ii:isInformationProcessingInputIn];
      owl:someValuesFrom pims-ii:Object
   ], [
      a owl:Restriction;
      owl:onProperty [owl:inverseOf pims-ii:isObjectInInformationProcessing];
      owl:someValuesFrom pims-ii:Object
   ], [
      a owl:Restriction;
      owl:onProperty [owl:inverseOf pims-ii:isInformationProcessingOutputIn];
      owl:someValuesFrom pims-ii:Object
   ];
   rdfs:comment "Information processing, i.e., an interpretation in which information is handled, revised, reformatted, extended, or narrowed down (or anything comparable to such actions), e.g., preprocessing or postprocessing in a simulation workflow"^^xs:string.

pims-ii:Interpretation a owl:Class;
   rdfs:label "Interpretation"@en;
   skos:altLabel "IPR"@en;
   rdfs:subClassOf pims-ii:Semiosis, [
      a owl:Restriction;
      owl:onProperty [owl:inverseOf pims-ii:isSignInInterpretation];
      owl:someValuesFrom pims-ii:Object
   ], [
      a owl:Restriction;
      owl:onProperty [owl:inverseOf pims-ii:isObjectInInterpretation];
      owl:someValuesFrom pims-ii:Object
   ], [
      a owl:Restriction;
      owl:onProperty [owl:inverseOf pims-ii:isInterpretantInInterpretation];
      owl:someValuesFrom pims-ii:Object
   ];
   rdfs:comment "Interpretation, i.e., a semiosis where the sign-object relation is carried over from the preceding cognitive step, without the need for the represented object to be present physically"^^xs:string.

pims-ii:InvestigationSetup a owl:Class;
   rdfs:label "InvestigationSetup"@en;
   rdfs:subClassOf pims-ii:Metonymization, [
      a owl:Restriction;
      owl:onProperty [owl:inverseOf pims-ii:isObjectOfApplicationIn];
      owl:someValuesFrom pims-ii:Object
   ], [
      a owl:Restriction;
      owl:onProperty [owl:inverseOf pims-ii:isSignInInvestigation];
      owl:someValuesFrom pims-ii:Object
   ], [
      a owl:Restriction;
      owl:onProperty [owl:inverseOf pims-ii:isObjectOfInvestigationIn];
      owl:someValuesFrom pims-ii:Object
   ];
   rdfs:comment "Investigation setup, i.e., a metonymization where a sign (e.g., a model and/or open question) that has come up for an 'object of application' (the old referent, e.g., the system to which a use case refers) is reassigned to an 'object of investigation' to which dedicated studies can be applied, such as a system that will be simulated or investigated experimentally; n.b., there needs to be a causal connection between the old and the new referent, i.e., between the object of application and the object of investigation"^^xs:string.

pims-ii:IRI a owl:Class;
   rdfs:label "IRI"@en;
   rdfs:subClassOf pims-ii:CollectiveLiteral, pims-ii:DigitalArticulation;
   owl:unionOf (pims-ii:ConceptualIRI pims-ii:ContextualIRI pims-ii:IndividualIRI pims-ii:RelationalIRI);
   rdfs:comment "Internationalized resource identifier (IRI) as defined by RFC 3987; an IRI object should be related by 'isLiterally' to an xs:string containing the IRI literal"^^xs:string.

pims-ii:KnowledgeBase a owl:Class;
   rdfs:label "KnowledgeBase"@en;
   rdfs:subClassOf pims-ii:Interlocutor;
   rdfs:comment "Knowledge base, i.e., an interlocutor that makes a consistent set of claims and will respond consistently if queried; n.b., that propositional content which 'isHeldBy' a knowledge base needs to be invariable over the whole 4D spacetime in which the knowledge base exist. Since technical knowledge bases do happen to change their propositional content over time, it may make sense either to define proper parts with a short temporal extension or to take care with what a knowledge base is stated to hold. Other kinds of propositional content (varying over time or depending on who makes the query) can be said to be asserted rather than held by the knowledge base."^^xs:string.

pims-ii:Lexeme a owl:Class;
   rdfs:label "Lexeme"@en;
   rdfs:subClassOf pims-ii:CollectiveLiteral, pims-ii:Conventional;
   rdfs:comment "Lexeme, i.e., a semiotic collective the members of which are all instances/utterances/copies of the same word (or a fragment or group of words that fulfills the corresponding function) which acts as a conventional articulation due to social convention; different ways of writing the word, such as an abbreviation and the full version, may belong to the same lexeme"^^xs:string.

pims-ii:MaterialIdentifier a owl:Class;
   rdfs:label "MaterialIdentifier"@en;
   rdfs:subClassOf pims-ii:Name;
   rdfs:comment "Name or label that identifies the material of its referent, or the material that some semiotic collective is about"@en;
   skos:scopeNote "in particular, the TUCAN identifiers from NFDI4Chem can be used".

pims-ii:MathematicalOperator a owl:Class;
   rdfs:label "MathematicalOperator"@en;
   rdfs:subClassOf pims-ii:Lexeme;
   rdfs:comment "Mathematical operator, i.e., a lexeme that articulates a mathematical operation, such as the collective containing realizations of '*', '·', 'times', etc."^^xs:string.

pims-ii:Measurement a owl:Class;
   rdfs:label "Measurement"@en;
   rdfs:subClassOf pims-ii:Observation, [
      a owl:Restriction;
      owl:onProperty [owl:inverseOf pims-ii:isMeasurementInputIn];
      owl:someValuesFrom pims-ii:Object
   ], [
      a owl:Restriction;
      owl:onProperty [owl:inverseOf pims-ii:isMeasuredObjectIn];
      owl:someValuesFrom pims-ii:Object
   ], [
      a owl:Restriction;
      owl:onProperty [owl:inverseOf pims-ii:isMeasurementOutcomeIn];
      owl:someValuesFrom pims-ii:Object
   ];
   rdfs:comment "Measurement, i.e., an observation that follows a standard procedure, so that it can be expected to yield an objective (rather than subjective) outcome"^^xs:string.

pims-ii:MeasurementUnit a owl:Class;
   rdfs:label "MeasurementUnit"@en;
   rdfs:subClassOf pims-ii:Lexeme;
   rdfs:comment "Measurement unit, i.e., a 'real scalar quantity, defined and adopted by convention' (EMMO, ISO 80000-1)"^^xs:string.

pims-ii:Metonymization a owl:Class;
   rdfs:label "Metonymization"@en;
   rdfs:subClassOf pims-ii:SemanticChange, [
      a owl:Restriction;
      owl:onProperty [owl:inverseOf pims-ii:isOldReferentInMetonymization];
      owl:someValuesFrom pims-ii:Object
   ], [
      a owl:Restriction;
      owl:onProperty [owl:inverseOf pims-ii:changesReferentInMetonymization];
      owl:someValuesFrom pims-ii:Object
   ], [
      a owl:Restriction;
      owl:onProperty [owl:inverseOf pims-ii:isNewReferentInMetonymization];
      owl:someValuesFrom pims-ii:Object
   ];
   rdfs:comment "Metonymization, i.e., a semantic change where there is a causal connection between the old and the new referent, so that the criterion of a 'real causal connection' (between signs and objects) from Peircean semiotics is preserved"^^xs:string.

pims-ii:Modelling a owl:Class;
   rdfs:label "Modelling"@en;
   rdfs:subClassOf pims-ii:Interpretation, [
      a owl:Restriction;
      owl:onProperty [owl:inverseOf pims-ii:isModellingInputIn];
      owl:someValuesFrom pims-ii:Object
   ], [
      a owl:Restriction;
      owl:onProperty [owl:inverseOf pims-ii:isModelledIn];
      owl:someValuesFrom pims-ii:Object
   ], [
      a owl:Restriction;
      owl:onProperty [owl:inverseOf pims-ii:isModellingOutputIn];
      owl:someValuesFrom pims-ii:Object
   ];
   rdfs:comment "Modelling, i.e., an interpretation in which the sign is the basis for the modelling process (e.g., an unparameterized or previously parameterized model, knowledge about the modelled system, etc.), the object is the modelled system, and the interpretant is the modelling output (e.g., a parameterized model)"^^xs:string.

pims-ii:Name a owl:Class;
   rdfs:label "Name"@en;
   rdfs:subClassOf pims-ii:Lexeme, [
      a owl:Restriction;
      owl:onProperty pims-ii:isNameFor;
      owl:someValuesFrom pims-ii:Object
   ];
   rdfs:comment "Name, i.e., a lexeme that acts as a rigid designator due to social convention"^^xs:string.

pims-ii:Number a owl:Class;
   rdfs:label "Number"@en;
   rdfs:subClassOf pims-ii:Lexeme;
   rdfs:comment "Number, i.e., a lexeme that is numerical in nature, such as the collective containing realizations of 'two', '2', and '2.0'"^^xs:string.

pims-ii:Observation a owl:Class;
   rdfs:label "Observation"@en;
   rdfs:subClassOf pims-ii:Perception, pims-ii:PurposefulAction, [
      a owl:Restriction;
      owl:onProperty [owl:inverseOf pims-ii:isObservationInputIn];
      owl:someValuesFrom pims-ii:Object
   ], [
      a owl:Restriction;
      owl:onProperty [owl:inverseOf pims-ii:isObservedIn];
      owl:someValuesFrom pims-ii:Object
   ], [
      a owl:Restriction;
      owl:onProperty [owl:inverseOf pims-ii:isObservationOutcomeIn];
      owl:someValuesFrom pims-ii:Object
   ];
   rdfs:comment "Observation, i.e., a perception by which characteristic aspects of an object (e.g., a target property or some more complex kind of behaviour) are purposefully investigated through specific means of perception; the procedure and evaluation may occur based on subjective judgement or according to an agreed procedure"^^xs:string.

pims-ii:OwnClaim a owl:Class;
   rdfs:label "OwnClaim"@en;
   rdfs:subClassOf pims-ii:Claim;
   owl:equivalentClass [
      a owl:Restriction;
      owl:onProperty pims-ii:isAssertedBy;
      owl:someValuesFrom pims-ii:ReferenceToSelf
   ];
   rdfs:comment "Own claim, i.e., a claim that is asserted by a self reference (i.e., a/the present interlocutor)"@en;
   skos:scopeNote "Specifically this could be used as a concept to be applied to propositional content of the present knowledge base"@en.

pims-ii:Optimization a owl:Class;
   rdfs:label "Optimization"@en;
   rdfs:subClassOf pims-ii:Interpretation, [
      a owl:Restriction;
      owl:onProperty [owl:inverseOf pims-ii:isOptimizationProblemIn];
      owl:someValuesFrom pims-ii:OptimizationProblem
   ], [
      a owl:Restriction;
      owl:onProperty [owl:inverseOf pims-ii:isObjectInOptimization];
      owl:someValuesFrom pims-ii:Object
   ], [
      a owl:Restriction;
      owl:onProperty [owl:inverseOf pims-ii:isOptimizationOutputIn];
      owl:someValuesFrom pims-ii:Object
   ];
   rdfs:comment "Optimization, i.e., an interpretation in which the sign is the optimization problem, the object is that which the optimization problem is ultimately about, and the interpretant is the optimization output"^^xs:string.

pims-ii:PartToWhole a owl:Class;
   rdfs:label "PartToWhole"@en;
   rdfs:subClassOf pims-ii:Synecdoche, [
      a owl:Restriction;
      owl:onProperty [owl:inverseOf pims-ii:isOldReferentInPartToWhole];
      owl:someValuesFrom pims-ii:Object
   ], [
      a owl:Restriction;
      owl:onProperty [owl:inverseOf pims-ii:changesReferentInPartToWhole];
      owl:someValuesFrom pims-ii:Object
   ], [
      a owl:Restriction;
      owl:onProperty [owl:inverseOf pims-ii:isNewReferentInPartToWhole];
      owl:someValuesFrom pims-ii:Object
   ];
   rdfs:comment "Part-to-whole synecdoche, i.e., a metonymization where the old referent is a spatiotemporal proper part of the new referent (additionally, the old and new referent need to be connected causally)"^^xs:string.

pims-ii:Perception a owl:Class;
   rdfs:label "Perception"@en;
   skos:altLabel "PCN"@en;
   rdfs:subClassOf pims-ii:Semiosis, [
      a owl:Restriction;
      owl:onProperty [owl:inverseOf pims-ii:isSignInPerception];
      owl:someValuesFrom pims-ii:Object
   ], [
      a owl:Restriction;
      owl:onProperty [owl:inverseOf pims-ii:isPerceivedIn];
      owl:someValuesFrom pims-ii:Object
   ], [
      a owl:Restriction;
      owl:onProperty [owl:inverseOf pims-ii:isInterpretantInPerception];
      owl:someValuesFrom pims-ii:Object
   ];
   rdfs:comment "Perception, i.e., a semiosis in which the referent is a participant (as a perceived object) and therefore needs to be physically present"@en;
   skos:scopeNote "the perception is conducted by an agent, namely, the interpreter who perceives the object"@en.

pims-ii:Person a owl:Class;
   rdfs:label "Person"@en;
   rdfs:subClassOf pims-ii:Interlocutor, [
      a owl:Restriction;
      owl:onProperty [owl:inverseOf pims-ii:isNameFor];
      owl:someValuesFrom pims-ii:Name
   ];
   rdfs:comment "Person, i.e., an interlocutor that is socially identified as a natural or legal person by social convention that involves using a name (or multiple names) for it as rigid designators"^^xs:string.

pims-ii:Planning a owl:Class;
   rdfs:label "Planning"@en;
   rdfs:subClassOf pims-ii:Telesis, pims-ii:Perception, [
      a owl:Restriction;
      owl:onProperty [owl:inverseOf pims-ii:isTelosInPlanning];
      owl:someValuesFrom pims-ii:Object
   ], [
      a owl:Restriction;
      owl:onProperty [owl:inverseOf pims-ii:isSituationInPlanning];
      owl:someValuesFrom pims-ii:Object
   ], [
      a owl:Restriction;
      owl:onProperty [owl:inverseOf pims-ii:isResolutionInPlanning];
      owl:someValuesFrom pims-ii:Object
   ];
   rdfs:comment "Planning, i.e., a reflection ex ante or predetermination, carried out by analysing the perceived present situation in advance of potentially undertaking an action"^^xs:string.

pims-ii:Plurality a owl:Class;
   rdfs:label "Plurality"@en;
   skos:altLabel "PL"@en;
   rdfs:subClassOf pims-ii:SemioticCollective, [
      a owl:Restriction;
      owl:onProperty [owl:inverseOf pims-ii:isMemberOfPlurality];
      owl:minCardinality 2
   ];
   owl:equivalentClass [
      a owl:Restriction;
      owl:onProperty [owl:inverseOf pims-ii:isMemberOfPlurality];
      owl:someValuesFrom pims-ii:Object
   ];
   owl:disjointWith [
      a owl:Restriction;
      owl:onProperty [owl:inverseOf pims-ii:isSemioticMemberOf];
      owl:someValuesFrom [owl:unionOf (pims-ii:Plurality pims-ii:Structure)]
   ];
   rdfs:comment "Plurality, i.e., a semiotic collective the semiotic members of which are a representational element (referent or representamen) together, whereby all act/contribute in the same way - this latter point distinguishes a plurality from a structure; e.g., the referent of the expression 'the four seasons/quarters of the year' (for a given year, within a given spatial region) is a plurality, and each of the four seasons/quarters is one of its semiotic members"^^xs:string.

pims-ii:Presupposition a owl:Class;
   rdfs:label "Presupposition"@en;
   rdfs:subClassOf pims-ii:GroundedCognition;
   owl:equivalentClass [
      a owl:Restriction;
      owl:onProperty [owl:inverseOf pims-ii:isGroundFor];
      owl:someValuesFrom pims-ii:BasicGround
   ];
   rdfs:comment "Presupposition, i.e., a cognition that has a basic ground, so that it is accepted a priori as an ultimate anchor point for epistemic grounding; any cognition that is logically preceded by a presupposition is a grounded cognition"^^xs:string.

pims-ii:Property a owl:Class;
   rdfs:label "Property"@en;
   rdfs:subClassOf pims-ii:Variable;
   rdfs:comment "Property, i.e., a variable that is employed for the possible outcome of observations and similar processes (this may include different words used for the same property, in one or multiple languages, and different ways of expressing these words)"^^xs:string.

pims-ii:Proposition a owl:Class;
   rdfs:label "Proposition"@en;
   skos:altLabel "PN"@en;
   rdfs:subClassOf pims-ii:SemioticCollective, [
      a owl:Restriction;
      owl:onProperty [owl:inverseOf pims-ii:articulatesLiterally];
      owl:someValuesFrom pims-ii:CollectiveLiteral
   ], [
      a owl:Restriction;
      owl:onProperty [owl:inverseOf pims-ii:isSemioticMemberOf];
      owl:allValuesFrom pims-ii:Articulation
   ], [
      a owl:Restriction;
      owl:onProperty pims-ii:isAbout;
      owl:minCardinality 1
   ];
   owl:equivalentClass [
      a owl:Restriction;
      owl:onProperty [owl:inverseOf pims-ii:articulates];
      owl:someValuesFrom pims-ii:Articulation
   ];
   rdfs:comment "Proposition, i.e., a semiotic collective the members of which are collective literals and collective utterances understood to be attributed some joint semantic and/or pragmatic content, or undergoing evaluation jointly for the presence of such a content"@en;
   skos:scopeNote "Note that this here includes any kind of semiotic collective that fits the given definition; the semantic/pragmatic content may be assertive, but also interrogative or of any other character - in particular, by this definition, 'Question' is a subclass of 'Proposition'"@en.

pims-ii:QuantityValue a owl:Class;
   rdfs:label "QuantityValue"@en;
   rdfs:subClassOf pims-ii:Value;
   owl:equivalentClass [
      owl:intersectionOf (
         [
            a owl:Restriction;
            owl:onProperty [owl:inverseOf pims-ii:isMagnitudeOf];
            owl:someValuesFrom pims-ii:Number
         ] [
            a owl:Restriction;
            owl:onProperty [owl:inverseOf pims-ii:isUnitOf];
            owl:someValuesFrom pims-ii:MeasurementUnit
         ]
      )
   ];
   rdfs:comment "Quantity value, i.e., a value that has a numerical magnitude and a physical unit"@en.

pims-ii:Query a owl:Class;
   rdfs:label "Query"@en;
   rdfs:subClassOf pims-ii:DigitalArticulation;
   owl:equivalentClass [
      owl:intersectionOf (
         pims-ii:DigitalArticulation [
            a owl:Restriction;
            owl:onProperty pims-ii:articulates;
            owl:someValuesFrom pims-ii:Question
         ]
      )
   ];
   rdfs:comment "Query, i.e., a digital articulation of a question"@en.

pims-ii:Question a owl:Class;
   rdfs:label "Question"@en;
   skos:altLabel "QN"@en;
   rdfs:subClassOf pims-ii:Topical;
   rdfs:comment "Question, i.e., a topical proposition the semantics/pragmatics of which are of interrogative character"@en;
   skos:scopeNote "A question contains interrogative pronouns or other interrogative elements, such as blank nodes when articulated as a query"@en;
   skos:scopeNote "Questions are articulated digitally by queries"@en.

pims-ii:RelationalIRI a owl:Class;
   rdfs:label "RelationalIRI"@en;
   rdfs:subClassOf pims-ii:IRI;
   owl:disjointWith pims-ii:ConceptualIRI, pims-ii:ContextualIRI, pims-ii:IndividualIRI;
   rdfs:comment "Relational IRI, i.e., the internationalized resource identifier of a something that can play the role of the predicate in a triple; this includes 'rdf:type', object properties, datatype properties, their negations"^^xs:string.

pims-ii:ResearchQuestion a owl:Class;
   rdfs:label "ResearchQuestion"@en;
   skos:altLabel "RQN"@en;
   rdfs:subClassOf pims-ii:Question;
   rdfs:comment "Research question, i.e., a question that could, has been, or is being addressed by scientific research and e.g. could be answered by a knowledge claim formulated on the grounds of scientific research data"@en.

pims-ii:Rule a owl:Class;
   rdfs:label "Rule"@en;
   rdfs:subClassOf pims-ii:Proposition, [
      a owl:Restriction;
      owl:onProperty [owl:inverseOf pims-ii:isAntecedentWithin];
      owl:someValuesFrom pims-ii:Proposition
   ], [
      a owl:Restriction;
      owl:onProperty [owl:inverseOf pims-ii:isConsequentWithin];
      owl:someValuesFrom pims-ii:Proposition
   ], [
      a owl:Restriction;
      owl:onProperty [owl:inverseOf pims-ii:articulates];
      owl:someValuesFrom pims-ii:Dyad
   ], [
      a owl:Restriction;
      owl:onProperty [owl:inverseOf pims-ii:isOrthodataWithin];
      owl:someValuesFrom pims-ii:DigitalArticulation
   ];
   rdfs:comment "Rule, i.e., a proposition consisting of an antecedent and one or multiple consequent(s) such that the antecedent is stated to imply the consequent(s)"^^xs:string.

pims-ii:Selection a owl:Class;
   rdfs:label "Selection"@en;
   rdfs:subClassOf pims-ii:InformationProcessing, [
      a owl:Restriction;
      owl:onProperty [owl:inverseOf pims-ii:isSelectionInputIn];
      owl:someValuesFrom pims-ii:Object
   ], [
      a owl:Restriction;
      owl:onProperty [owl:inverseOf pims-ii:isObjectInSelection];
      owl:someValuesFrom pims-ii:Object
   ], [
      a owl:Restriction;
      owl:onProperty [owl:inverseOf pims-ii:isSelectionOutputIn];
      owl:someValuesFrom pims-ii:Object
   ];
   rdfs:comment "Selection, i.e., an information-processing step in which the given information is narrowed down such that the output (interpretant) is constitutive of the input (sign); this includes conditional selection, where one component of the input or another is retained depending on a selection condition (cf. relation isSelectionConditionIn)"^^xs:string.

pims-ii:ReferenceToSelf a owl:Class;
   rdfs:label "ReferenceToSelf"@en;
   rdfs:subClassOf pims-ii:Interlocutor;
   rdfs:comment "Reference to self, i.e., an entity for the interlocutor who *is* the present system, i.e., the system containing the present triples, etc., and whose claims are to be accepted as the present system's 'own claims.' A self-reference is an entity that is either identical with the system at hand, namely, the digital infrastructure or other interlocutor that stores the present semantic content, or a component of it"@en;
   skos:example "If the present triples are processed by a research data infrastructure with a federated architecture, consisting of several repositories (which are interlocutors, i.e., they can be queried and communicate with the outside world), both the research data infrastructure as a whole and the individual repositories are self-references"@en;
   skos:scopeNote "This is relevant for distinguishing anybody's claims from the present system's own claims: If and only if a proposition is asserted by a self-reference, it is an own claim"@en.

pims-ii:SemanticChange a owl:Class;
   rdfs:label "SemanticChange"@en;
   rdfs:subClassOf pims-ii:TriadicCognition, [
      a owl:Restriction;
      owl:onProperty [owl:inverseOf pims-ii:isOldReferentIn];
      owl:someValuesFrom pims-ii:Object
   ], [
      a owl:Restriction;
      owl:onProperty [owl:inverseOf pims-ii:changesReferentIn];
      owl:someValuesFrom pims-ii:Object
   ], [
      a owl:Restriction;
      owl:onProperty [owl:inverseOf pims-ii:isNewReferentIn];
      owl:someValuesFrom pims-ii:Object
   ];
   rdfs:comment "Semantic change, i.e., a triadic cognition by which a representamen is assigned a new referent"^^xs:string.

pims-ii:Semiosis a owl:Class;
   rdfs:label "Semiosis"@en;
   rdfs:subClassOf pims-ii:TriadicCognition, [
      a owl:Restriction;
      owl:onProperty [owl:inverseOf pims-ii:isSignIn];
      owl:someValuesFrom pims-ii:Object
   ], [
      a owl:Restriction;
      owl:onProperty [owl:inverseOf pims-ii:isObjectIn];
      owl:someValuesFrom pims-ii:Object
   ], [
      a owl:Restriction;
      owl:onProperty [owl:inverseOf pims-ii:isInterpretantIn];
      owl:someValuesFrom pims-ii:Object
   ];
   owl:disjointUnionOf (pims-ii:Perception pims-ii:Interpretation);
   rdfs:comment "Semiosis, i.e., a triadic congition that relates 'the sign', 'the object', and 'the interpretant' to each other; a semiosis is either a perception (if the object needs to be present and participate physically in the process) or an interpretation (if the physical participation of the object is not inherently necessary)"^^xs:string.

pims-ii:SemioticCollective a owl:Class;
   rdfs:label "SemioticCollective"@en;
   skos:altLabel "SCO"@en;
   rdfs:subClassOf pims-ii:Collective, [
      a owl:Restriction;
      owl:onProperty [owl:inverseOf pims-ii:isSemioticMemberOf];
      owl:minCardinality 2
   ];
   owl:equivalentClass [
      a owl:Restriction;
      owl:onProperty [owl:inverseOf pims-ii:isSemioticMemberOf];
      owl:someValuesFrom pims-ii:Item
   ], [
      a owl:Restriction;
      owl:onProperty pims-ii:isRepresentationalElementIn;
      owl:someValuesFrom pims-ii:CognitiveStep
   ];
   owl:disjointUnionOf (pims-ii:Articulation pims-ii:Proposition pims-ii:Structure pims-ii:Plurality);
   rdfs:comment "Semiotic collective, i.e., a collective the semiotic members of which act together as one representational element (i.e., referent or representamen) in a cognitive process"^^xs:string.

pims-ii:Simulation a owl:Class;
   rdfs:label "Simulation"@en;
   rdfs:subClassOf pims-ii:Interpretation, pims-ii:PurposefulAction, [
      a owl:Restriction;
      owl:onProperty [owl:inverseOf pims-ii:isSimulationInputIn];
      owl:someValuesFrom pims-ii:Object
   ], [
      a owl:Restriction;
      owl:onProperty [owl:inverseOf pims-ii:isSimulatedIn];
      owl:someValuesFrom pims-ii:Object
   ], [
      a owl:Restriction;
      owl:onProperty [owl:inverseOf pims-ii:isSimulationOutputIn];
      owl:someValuesFrom pims-ii:Object
   ];
   rdfs:comment "Simulation, i.e., a purposefully conducted numerical interpretation of simulation input (model, etc.), where the interpretant is the simulation result"^^xs:string.

pims-ii:SimulationWorkflow a owl:Class;
   rdfs:label "SimulationWorkflow"@en;
   rdfs:subClassOf pims-ii:CognitiveWorkflow, [
      a owl:Restriction;
      owl:onProperty [owl:inverseOf pims-ii:isStepInCognitiveChain];
      owl:someValuesFrom pims-ii:Simulation
   ];
   rdfs:comment "simulation workflow, i.e., a cognitive workflow in which simulation plays a major role"^^xs:string.

pims-ii:Steering a owl:Class;
   rdfs:label "Steering"@en;
   rdfs:subClassOf pims-ii:Telesis, pims-ii:Perception, [
      a owl:Restriction;
      owl:onProperty [owl:inverseOf pims-ii:isTelosInSteering];
      owl:someValuesFrom pims-ii:Object
   ], [
      a owl:Restriction;
      owl:onProperty [owl:inverseOf pims-ii:isActionInSteering];
      owl:someValuesFrom pims-ii:Object
   ], [
      a owl:Restriction;
      owl:onProperty [owl:inverseOf pims-ii:isResolutionInSteering];
      owl:someValuesFrom pims-ii:Object
   ];
   rdfs:comment "Steering, i.e., a reflection in actu (Reflexion im Vollzug following Baumann and Tulatz) or determination, carried out while undertaking an action and playing a role in that action by proper participation"^^xs:string.

pims-ii:Structure a owl:Class;
   rdfs:label "Structure"@en;
   rdfs:subClassOf pims-ii:SemioticCollective, [
      a owl:Restriction;
      owl:onProperty [owl:inverseOf pims-ii:isMemberOfStructure];
      owl:minCardinality 2
   ];
   owl:equivalentClass [
      a owl:Restriction;
      owl:onProperty [owl:inverseOf pims-ii:isMemberOfStructure];
      owl:someValuesFrom pims-ii:Object
   ];
   owl:disjointWith [
      a owl:Restriction;
      owl:onProperty [owl:inverseOf pims-ii:isSemioticMemberOf];
      owl:someValuesFrom pims-ii:Structure
   ];
   rdfs:comment "Structure, i.e., a semiotic collective the semiotic members of which complement each other, contributing in different ways (or, at least, not all int the same way) to their joint action as a referent or a representamen"^^xs:string.

pims-ii:Synecdoche a owl:Class;
   rdfs:label "Synecdoche"@en;
   rdfs:subClassOf pims-ii:Metonymization, [
      a owl:Restriction;
      owl:onProperty [owl:inverseOf pims-ii:isOldReferentInSynecdoche];
      owl:someValuesFrom pims-ii:Object
   ], [
      a owl:Restriction;
      owl:onProperty [owl:inverseOf pims-ii:changesReferentInSynecdoche];
      owl:someValuesFrom pims-ii:Object
   ], [
      a owl:Restriction;
      owl:onProperty [owl:inverseOf pims-ii:isNewReferentInSynecdoche];
      owl:someValuesFrom pims-ii:Object
   ];
   owl:disjointUnionOf (pims-ii:PartToWhole pims-ii:WholeToPart);
   rdfs:comment "Synecdoche, i.e., a metonymization where a sign is reassigned to a part of its old referent (WholeToPart) or vice versa (PartToWhole)"^^xs:string.

pims-ii:Telesis a owl:Class;
   rdfs:label "Telesis"@en;
   skos:altLabel "TEL"@en;
   rdfs:subClassOf pims-ii:Semiosis, pims-ii:CognitiveAction, [
      a owl:Restriction;
      owl:onProperty [owl:inverseOf pims-ii:isTelosIn];
      owl:someValuesFrom pims-ii:Object
   ], [
      a owl:Restriction;
      owl:onProperty [owl:inverseOf pims-ii:isObjectInTelesis];
      owl:someValuesFrom pims-ii:Object
   ], [
      a owl:Restriction;
      owl:onProperty [owl:inverseOf pims-ii:isResolutionInTelesis];
      owl:someValuesFrom pims-ii:Object
   ];
   owl:disjointUnionOf (pims-ii:Planning pims-ii:Steering pims-ii:Evaluation);
   rdfs:comment "Telesis (teleological semiosis), i.e., a semiosis where the sign is a telos (aim), the object is an action, claim, or situation against which that aim is evaluated, and the interpretant is a resolution, e.g., a revised objective, plan, or similar evaluation outcome"^^xs:string.

pims-ii:Term a owl:Class;
   rdfs:label "Term"@en;
   rdfs:subClassOf pims-ii:Conventional;
   owl:equivalentClass [
      a owl:Restriction;
      owl:onProperty [owl:inverseOf pims-ii:isAdmissibleValueFor];
      owl:someValuesFrom pims-ii:Value
   ];
   rdfs:comment "Term, i.e., a conventional that can evaluate to a value; terms include variables, values, and any mathematically and semantically valid ways of combining variables, values, and mathematical operators - note that it is required for a term to potentially take a value"^^xs:string.
   
pims-ii:Topical a owl:Class;
   rdfs:label "Topical"@en;
   skos:altLabel "TL"@en;
   rdfs:subClassOf pims-ii:Proposition;
   rdfs:comment "Topical proposition, i.e., something that can be understood as stating the topic of something"@en;
   skos:scopeNote "In particular, all questions are topical propositions, since they state the topic of their potential answer"@en;
   skos:scopeNote "A topic can be a product of (sub-)topics, that is the case if two aspects of something are being addressed jointly, with a genuine interaction between multiple factors; in this case, the whole topic is a topical product (subclass of topical), and its factors are related to it by pims-ii:isTopicalFactorIn. But something can also address multiple contributions to its subject matter independently, without a genuine interaction between the parts; in that case, the whole topic is a topical sum (disjoint with topical), its parts are topicals, and they are related to the whole by pims-ii:isTopicalSummandIn"@en.

pims-ii:TopicalProduct a owl:Class;
   rdfs:label "TopicalProduct"@en;
   rdfs:subClassOf pims-ii:Topical;
   owl:equivalentClass [
      a owl:Restriction;
      owl:onProperty [owl:inverseOf pims-ii:isTopicalFactorIn];
      owl:someValuesFrom [owl:unionOf (pims-ii:Topical pims-ii:TopicalSum)]
   ];
   rdfs:comment "Topical product, i.e., a topical proposition with multiple topical factors"@en.

pims-ii:TopicalSum a owl:Class;
   rdfs:label "TopicalSum"@en;
   skos:altLabel "TLS"@en;
   rdfs:subClassOf pims-ii:Plurality;
   owl:equivalentClass [
      a owl:Restriction;
      owl:onProperty [owl:inverseOf pims-ii:isTopicalSummandIn];
      owl:someValuesFrom pims-ii:Topical
   ];
   rdfs:comment "Topical sum, i.e., a plurality of topical propositions, where the individual elements (summands) don't genuinely interact but are just standing beside each other as independent, unrelated (or not very closely related) parts of what is addressed"@en.

pims-ii:TriadicCognition a owl:Class;
   rdfs:label "TriadicCognition"@en;
   rdfs:subClassOf pims-ii:CognitiveStep, pims-ii:CognitiveAction, [
      a owl:Restriction;
      owl:onProperty [owl:inverseOf pims-ii:isFirstElementIn];
      owl:someValuesFrom pims-ii:Object
   ], [
      a owl:Restriction;
      owl:onProperty [owl:inverseOf pims-ii:isSecondElementIn];
      owl:someValuesFrom pims-ii:Object
   ], [
      a owl:Restriction;
      owl:onProperty [owl:inverseOf pims-ii:isThirdElementIn];
      owl:someValuesFrom pims-ii:Object
   ], [
      a owl:Restriction;
      owl:onProperty [owl:inverseOf pims-ii:isGroundFor];
      owl:someValuesFrom pims-ii:Ground
   ];
   owl:disjointUnionOf (pims-ii:SemanticChange pims-ii:Semiosis);
   rdfs:comment "Triadic cognition, i.e., a cognitive step of the type s-o-s' (semiosis) or o-s-o' (semantic change), thus containing three elements, in line with the approach by Peirce"^^xs:string.

pims-ii:Triple a owl:Class;
   rdfs:label "Triple"@en;
   rdfs:subClassOf pims-ii:DataItem, [
      a owl:Restriction;
      owl:onProperty [owl:inverseOf pims-ii:isSubjectWithinTriple];
      owl:someValuesFrom pims-ii:IRI
   ], [
      a owl:Restriction;
      owl:onProperty [owl:inverseOf pims-ii:isPredicateWithinTriple];
      owl:someValuesFrom pims-ii:IRI
   ], [
      a owl:Restriction;
      owl:onProperty [owl:inverseOf pims-ii:isObjectWithinTriple];
      owl:someValuesFrom pims-ii:IRI
   ];
   rdfs:comment "Triple, i.e., a subject-predicate-object triple (connected by relations to the IRIs of the subject, predicate, and object)"^^xs:string.

pims-ii:UniqueIdentifier a owl:Class;
   rdfs:label "UniqueIdentifier"@en;
   rdfs:subClassOf pims-ii:Name;
   #
   # negative statement commented out to support SROIQ(D) compliance for domain ontologies situated below PIMS-II
   #
   # owl:equivalentClass [
   #    a owl:Restriction;
   #    owl:onProperty pims-ii:isNameFor;
   #    owl:cardinality 1
   # ];
   #
   rdfs:comment "Unique identifier, i.e., a rigid designator that is applied to exactly one object"^^xs:string.

pims-ii:Undertaking a owl:Class;
   rdfs:label "Undertaking"@en;
   rdfs:subClassOf pims-ii:Metonymization, [
      a owl:Restriction;
      owl:onProperty [owl:inverseOf pims-ii:isSituationInUndertaking];
      owl:someValuesFrom pims-ii:Object
   ], [
      a owl:Restriction;
      owl:onProperty [owl:inverseOf pims-ii:isResolutionInUndertaking];
      owl:someValuesFrom pims-ii:Object
   ], [
      a owl:Restriction;
      owl:onProperty [owl:inverseOf pims-ii:isActionInUndertaking];
      owl:someValuesFrom pims-ii:Object
   ], [
      a owl:Restriction;
      owl:onProperty [owl:inverseOf pims-ii:directlyGrounds];
      owl:someValuesFrom pims-ii:Telesis
   ];
   rdfs:comment "Undertaking, i.e., a metonymization by which a resolution, which was previously determined (by telesis) in response to the pre-existing situation, is actively taken up by the agent, motivating an action"^^xs:string.

pims-ii:Validation a owl:Class;
   rdfs:label "Validation"@en;
   skos:altLabel "VAL"@en;
   rdfs:subClassOf pims-ii:Evaluation, [
      a owl:Restriction;
      owl:onProperty [owl:inverseOf pims-ii:isTelosInValidation];
      owl:someValuesFrom pims-ii:Intention
   ], [
      a owl:Restriction;
      owl:onProperty [owl:inverseOf pims-ii:isValidatedIn];
      owl:someValuesFrom pims-ii:CognitiveAction
   ], [
      a owl:Restriction;
      owl:onProperty [owl:inverseOf pims-ii:isValidationOutcomeIn];
      owl:someValuesFrom pims-ii:ValidityClaim
   ];
   rdfs:comment "Validation, i.e., an evaluation of a cognition yielding a validity claim as its interpretant"@en.

pims-ii:Value a owl:Class;
   rdfs:label "Value"@en;
   rdfs:subClassOf pims-ii:Term, [
      a owl:Restriction;
      owl:onProperty pims-ii:isAdmissibleValueFor;
      owl:someValuesFrom pims-ii:Variable
   ];
   rdfs:comment "Value, i.e., an articulation that is by social convention understood to be potentially assignable to a variable"^^xs:string.

pims-ii:Variable a owl:Class;
   rdfs:label "Variable"@en;
   rdfs:subClassOf pims-ii:Term;
   rdfs:comment "Variable, i.e., a conventional that is employed for something to which values can be assigned (this may include different notations for the same variable including, e.g., computational representations); this is to be understood very generally, e.g., a variable may be an array or set of elements or have another kind of internal structure"^^xs:string.

pims-ii:Visualization a owl:Class;
   rdfs:label "Visualization"@en;
   rdfs:subClassOf pims-ii:Interpretation, [
      a owl:Restriction;
      owl:onProperty [owl:inverseOf pims-ii:isVisualizationInputIn];
      owl:someValuesFrom pims-ii:Object
   ], [
      a owl:Restriction;
      owl:onProperty [owl:inverseOf pims-ii:isVisualizedObjectIn];
      owl:someValuesFrom pims-ii:Object
   ], [
      a owl:Restriction;
      owl:onProperty [owl:inverseOf pims-ii:isVisualizationOutputIn];
      owl:someValuesFrom pims-ii:Object
   ];
   rdfs:comment "Visualization, i.e., an interpretation in which the object is the visualized system and the interpretant is a visual representation of the object - the sign is a pre-existing representamen for the same object, e.g., a simulation result"^^xs:string.

pims-ii:WholeToPart a owl:Class;
   rdfs:label "WholeToPart"@en;
   rdfs:subClassOf pims-ii:Synecdoche, [
      a owl:Restriction;
      owl:onProperty [owl:inverseOf pims-ii:isOldReferentInWholeToPart];
      owl:someValuesFrom pims-ii:Object
   ], [
      a owl:Restriction;
      owl:onProperty [owl:inverseOf pims-ii:changesReferentInWholeToPart];
      owl:someValuesFrom pims-ii:Object
   ], [
      a owl:Restriction;
      owl:onProperty [owl:inverseOf pims-ii:isNewReferentInWholeToPart];
      owl:someValuesFrom pims-ii:Object
   ];
   rdfs:comment "Whole-to-part synecdoche, i.e., a metonymization where the new referent is a spatiotemporal proper part of the old referent (additionally, the old and new referent need to be connected causally)"^^xs:string.

##################################################
# CORE MEREOSEMIOTICS: TRIADIC-ELEMENT RELATIONS #
##################################################

# Accumulation
#
pims-ii:isAccumulationInputIn a owl:ObjectProperty;
   rdfs:label "isAccumulationInputIn"@en;
   rdfs:range pims-ii:Accumulation;
   rdfs:subPropertyOf pims-ii:isInformationProcessingInputIn;
   rdfs:comment "(x isAccumulationInputIn y) == y is an accumulation where x is the input (initially given information), i.e., the first element; n.b., in an accumulation, the input needs to be constitutive of the output"^^xs:string.
pims-ii:isObjectInAccumulation a owl:ObjectProperty;
   rdfs:label "isObjectInAccumulation"@en;
   rdfs:range pims-ii:Accumulation;
   rdfs:subPropertyOf pims-ii:isObjectInInformationProcessing;
   rdfs:comment "(x isObjectInAccumulation y) == y is an accumulation where x is the object that the input and the output both represent, i.e., the second element"^^xs:string.
pims-ii:isAccumulationOutputIn a owl:ObjectProperty;
   rdfs:label "isAccumulationOutputIn"@en;
   rdfs:range pims-ii:Accumulation;
   rdfs:subPropertyOf pims-ii:isInformationProcessingOutputIn;
   rdfs:comment "(x isAccumulationOutputIn y) == y is an accumulation where x is the output (combined information), i.e., the third element; n.b., in a selection, the input and any additionally included elements need to be constitutive of the output"^^xs:string.
pims-ii:isIncludedInAccumulation a owl:ObjectProperty;
   rdfs:label "isIncludedInAccumulation"@en;
   rdfs:range pims-ii:Accumulation;
   rdfs:subPropertyOf pims-ii:isParticipantIn;
   rdfs:comment "(x isIncludedInAccumulation y) == y is an accumulation where x is combined with the accumulation input, yielding an output that x is constitutive of; n.b., x needs to act as a representamen for the object (e.g., as an interpretant from a preceding cognitive step with the same object)"^^xs:string.
pims-ii:isAccumulationConditionIn a owl:ObjectProperty;
   rdfs:label "isAccumulationConditionIn"@en;
   rdfs:domain pims-ii:Proposition;
   rdfs:range pims-ii:Accumulation;
   rdfs:subPropertyOf pims-ii:isRepresentamenFor;
   rdfs:comment "(x isAccumulationConditionIn y) == in the accumulation process y, the condition x controls in what way the input and the additionally included elements interact to yield a combined output"^^xs:string.

# CognitiveStep
#
pims-ii:isReferentIn a owl:ObjectProperty;
   rdfs:label "isReferentIn"@en;
   rdfs:range pims-ii:CognitiveStep;
   rdfs:subPropertyOf pims-ii:isRepresentationalElementIn;
   rdfs:comment "(x isReferentIn y) == x occurs in the cognitive step y in the function of the/a referent of a representamen"@en.
pims-ii:isRepresentamenIn a owl:ObjectProperty;
   rdfs:label "isRepresentamenIn"@en;
   rdfs:range pims-ii:CognitiveStep;
   rdfs:subPropertyOf pims-ii:isRepresentationalElementIn, pims-ii:isParticipantInCognition;
   rdfs:comment "(x isRepresentamenIn y) == x participates in the cognitive step y in the role of the/a representamen"@en.
pims-ii:isRepresentationalElementIn a owl:ObjectProperty;
   rdfs:label "isRepresentationalElementIn"@en;
   rdfs:range pims-ii:CognitiveStep;
   rdfs:subPropertyOf pims-ii:isMereosemioticallyRelatedTo;
   rdfs:comment "(x isRepresentationalElementIn y) == x acts as a representamen or referent in the cognitive step y"^^xs:string.

# Duplication
#
pims-ii:isOriginalIn a owl:ObjectProperty;
   rdfs:label "isOriginalIn"@en;
   rdfs:range pims-ii:Duplication;
   rdfs:subPropertyOf pims-ii:isInformationProcessingInputIn;
   rdfs:comment "(x isOriginalIn y) == y is a duplication step where x is the input (original version), i.e., the first element"^^xs:string.
pims-ii:isObjectInDuplication a owl:ObjectProperty;
   rdfs:label "isObjectInDuplication"@en;
   rdfs:range pims-ii:Duplication;
   rdfs:subPropertyOf pims-ii:isObjectInInformationProcessing;
   rdfs:comment "(x isObjectInDuplication y) == y is a duplication step where x is the object that the original and the duplicate both represent, i.e., the second element"^^xs:string.
pims-ii:isDuplicateIn a owl:ObjectProperty;
   rdfs:label "isDuplicateIn"@en;
   rdfs:range pims-ii:Duplication;
   rdfs:subPropertyOf pims-ii:isInformationProcessingOutputIn;
   rdfs:comment "(x isDuplicateIn y) == y is a duplication step where x is the output (duplicate), i.e., the third element"^^xs:string.

# Evaluation
#
pims-ii:isTelosInEvaluation a owl:ObjectProperty;
   rdfs:label "isTelosInEvaluation"@en;
   rdfs:range pims-ii:Evaluation;
   rdfs:subPropertyOf pims-ii:isTelosIn, pims-ii:isSignInInterpretation;
   rdfs:comment "(x isTelosInEvaluation y) == y is an evaluation (reflection ex post) where x acts as the telos (initial guiding objective), i.e., the first element"^^xs:string.
pims-ii:isEvaluatedIn a owl:ObjectProperty;
   rdfs:label "isEvaluatedIn"@en;
   rdfs:domain pims-ii:Action;
   rdfs:range pims-ii:Evaluation;
   rdfs:subPropertyOf pims-ii:isObjectInTelesis, pims-ii:isObjectInInterpretation, pims-ii:temporallyPrecedes;
   rdfs:comment "(x isEvaluatedIn y) == y is an evaluation (reflection ex post) where x is the action undergoing evaluation, i.e., the second element; n.b., the action needs to temporally precede the evaluation"^^xs:string.
pims-ii:isEvaluationOutcomeIn a owl:ObjectProperty;
   rdfs:label "isEvaluationOutcomeIn"@en;
   rdfs:range pims-ii:Evaluation;
   rdfs:subPropertyOf pims-ii:isResolutionInTelesis, pims-ii:isInterpretantInInterpretation;
   rdfs:comment "(x isEvaluationOutcomeIn y) == y is a an evaluation (reflection ex post) where x is the resolution (evaluation outcome), i.e., the third element"^^xs:string.
pims-ii:isEvaluatorIn a owl:ObjectProperty;
   rdfs:label "isEvaluatorIn"@en;
   skos:altLabel "\\ddot{P}_e"@en;
   rdfs:domain pims-ii:GoalDirectedAgent, pims-ii:Interlocutor;
   rdfs:range pims-ii:Evaluation;
   rdfs:subPropertyOf pims-ii:isInterpreterIn;
   rdfs:comment "(x isEvaluatorIn y) means that y is an evaluation and x is the interpreter in it"@en.

# Examination
#
pims-ii:isLegisignIn a owl:ObjectProperty;
   rdfs:label "isLegisignIn"@en;
   rdfs:range pims-ii:Examination;
   rdfs:subPropertyOf pims-ii:isObservationInputIn;
   rdfs:comment "(x isLegisignIn y) == y is an examination where x is applied to an object as a legisign, i.e., the first element, specifying patterns or rules the compliance with which is being assessed"^^xs:string.
pims-ii:isExaminedIn a owl:ObjectProperty;
   rdfs:label "isExaminedIn"@en;
   rdfs:range pims-ii:Examination;
   rdfs:subPropertyOf pims-ii:isObservedIn;
   rdfs:comment "(x isExaminedIn y) == y is an examination where x acts as the examined object, i.e., the second element, for which it is assessed to what extent (in which way, under what additional conditions, etc.) it conforms with the legisign"^^xs:string.
pims-ii:isExaminationOutcomeIn a owl:ObjectProperty;
   rdfs:label "isExaminationOutcomeIn"@en;
   rdfs:range pims-ii:Examination;
   rdfs:subPropertyOf pims-ii:isObservationOutcomeIn;
   rdfs:comment "(x isExaminationOutcomeIn y) == y is an examination where x is the examination outcome, i.e., the third element (e.g., yes the object agrees with the legisign, or it does so under this or that condition, etc.)"^^xs:string.

# GroundingInterpretation
#
pims-ii:groundsPresentStepIn a owl:ObjectProperty;
   rdfs:label "groundsPresentStepIn"@en;
   rdfs:domain pims-ii:Ground;
   rdfs:range pims-ii:GroundingInterpretation;
   rdfs:subPropertyOf pims-ii:isSignInInterpretation;
   rdfs:comment "(x groundsPresentStepIn y) == y is a grounding interpretation where x is the first element, i.e., a ground for the considered cognitive step"^^xs:string.
pims-ii:isPresentStepInGrounding a owl:ObjectProperty;
   rdfs:label "isPresentStepInGrounding"@en;
   rdfs:domain pims-ii:CognitiveStep;
   rdfs:range pims-ii:GroundingInterpretation;
   rdfs:subPropertyOf pims-ii:isObjectInInterpretation;
   rdfs:comment "(x isPresentStepInGrounding y) == y is a grounding interpretation where x is the second element, i.e., the considered cognitive step"^^xs:string.
pims-ii:groundsNextStepIn a owl:ObjectProperty;
   rdfs:label "groundsNextStepIn"@en;
   rdfs:domain pims-ii:Ground;
   rdfs:range pims-ii:GroundingInterpretation;
   rdfs:subPropertyOf pims-ii:isInterpretantInInterpretation, pims-ii:isGroundFor;
   rdfs:comment "(x groundsNextStepIn y) == y is a grounding interpretation where x is the third element, i.e., a ground for the subsequent cognitive step; thereby, x also serves as a ground for y itself"^^xs:string.

# GroundingMetonymization
#
pims-ii:isGroundingStepIn a owl:ObjectProperty;
   rdfs:label "isGroundingStepIn"@en;
   rdfs:domain pims-ii:CognitiveStep;
   rdfs:range pims-ii:GroundingMetonymization;
   rdfs:subPropertyOf pims-ii:isOldReferentInMetonymization;
   rdfs:comment "(x isGroundingStepIn y) == y is a grounding step where x is the grounding step, i.e., the first element"^^xs:string.
pims-ii:isGroundingPropositionIn a owl:ObjectProperty;
   rdfs:label "isGroundingPropositionIn"@en;
   rdfs:domain pims-ii:Ground;
   rdfs:range pims-ii:GroundingMetonymization;
   rdfs:subPropertyOf pims-ii:changesReferentInMetonymization, pims-ii:isGroundFor;
   rdfs:comment "(x isGroundingPropositionIn y) == y is a grounding step where x is the grounding proposition, i.e., the second element; therein, x is a ground for the grounded step, and x is also a ground for y itself"^^xs:string.
pims-ii:isGroundedStepIn a owl:ObjectProperty;
   rdfs:label "isGroundedStepIn"@en;
   rdfs:domain pims-ii:CognitiveStep;
   rdfs:range pims-ii:GroundingMetonymization;
   rdfs:subPropertyOf pims-ii:isNewReferentInMetonymization;
   rdfs:comment "(x isGroundedStepIn y) == y is a grounding step where x is the grounded step, i.e., the third element"^^xs:string.

# InformationProcessing
#
pims-ii:isInformationProcessingInputIn a owl:ObjectProperty;
   rdfs:label "isInformationProcessingInputIn"@en;
   rdfs:range pims-ii:InformationProcessing;
   rdfs:subPropertyOf pims-ii:isSignInInterpretation;
   rdfs:comment "(x isInformationProcessingInputIn y) == y is an information-processing step where x is the input, i.e., the first element"^^xs:string.
pims-ii:isObjectInInformationProcessing a owl:ObjectProperty;
   rdfs:label "isObjectInInformationProcessing"@en;
   rdfs:range pims-ii:InformationProcessing;
   rdfs:subPropertyOf pims-ii:isObjectInInterpretation;
   rdfs:comment "(x isObjectInInformationProcessing y) == y is an information-processing step where x is the object that the input and the output both represent, i.e., the second element"^^xs:string.
pims-ii:isInformationProcessingOutputIn a owl:ObjectProperty;
   rdfs:label "isInformationProcessingOutputIn"@en;
   rdfs:range pims-ii:InformationProcessing;
   rdfs:subPropertyOf pims-ii:isInterpretantInInterpretation;
   rdfs:comment "(x isInformationProcessingOutputIn y) == y is an information-processing step where x is the output, i.e., the third element"^^xs:string.

# Interpretation
#
pims-ii:isSignInInterpretation a owl:ObjectProperty;
   rdfs:label "isSignInInterpretation"@en;
   rdfs:range pims-ii:Interpretation;
   rdfs:subPropertyOf pims-ii:isSignIn;
   rdfs:comment "(x isSignInInterpretation y) == y is an interpretation where x acts as the sign, i.e., the first element"^^xs:string.
pims-ii:isObjectInInterpretation a owl:ObjectProperty;
   rdfs:label "isObjectInInterpretation"@en;
   rdfs:range pims-ii:Interpretation;
   rdfs:subPropertyOf pims-ii:isObjectIn;
   rdfs:comment "(x isObjectInInterpretation y) == y is an interpretation where x acts as the object, i.e., the second element; there is no need to the object of an interpretation to be present and participate in the interpretation process physically"^^xs:string.
pims-ii:isInterpretantInInterpretation a owl:ObjectProperty;
   rdfs:label "isInterpretantInInterpretation"@en;
   rdfs:range pims-ii:Interpretation;
   rdfs:subPropertyOf pims-ii:isInterpretantIn;
   rdfs:comment "(x isInterpretantInInterpretation y) == y is an interpretation where x acts as the interpretant, i.e., the third element"^^xs:string.

# InvestigationSetup
#
pims-ii:isObjectOfApplicationIn a owl:ObjectProperty;
   rdfs:label "isObjectOfApplicationIn"@en;
   rdfs:range pims-ii:InvestigationSetup;
   rdfs:subPropertyOf pims-ii:isOldReferentInMetonymization;
   rdfs:comment "(x isObjectOfApplicationIn y) == y is an investigation-setup action where x acts as the object of application (e.g., the system to which a use case refers), i.e., the first element; n.b., there needs to be a causal connection between the object of application and the object of investigation"^^xs:string.
pims-ii:isSignInInvestigation a owl:ObjectProperty;
   rdfs:label "isSignInInvestigation"@en;
   rdfs:range pims-ii:InvestigationSetup;
   rdfs:subPropertyOf pims-ii:changesReferentInMetonymization;
   rdfs:comment "(x isSignInInvestigation y) == y is an investigation-setup action where x acts as a representamen, i.e., the second element, both for the object of application (to which it is initially applied) and the object of investigation (to which it is reassigned such that the investigation can take place)"^^xs:string.
pims-ii:isObjectOfInvestigationIn a owl:ObjectProperty;
   rdfs:label "isObjectOfInvestigationIn"@en;
   rdfs:range pims-ii:InvestigationSetup;
   rdfs:subPropertyOf pims-ii:isNewReferentInMetonymization;
   rdfs:comment "(x isObjectOfInvestigationIn y) == y is an investigation-setup action where x acts as the object of investigation (e.g., the item subject to an experiment or a simulated process or system), i.e., as the third element; n.b., there needs to be a causal connection between the object of application and the object of investigation"^^xs:string.

# Measurement
#
pims-ii:isMeasurementInputIn a owl:ObjectProperty;
   rdfs:label "isMeasurementInputIn"@en;
   rdfs:range pims-ii:Measurement;
   rdfs:subPropertyOf pims-ii:isObservationInputIn;
   rdfs:comment "(x isMeasurementInputIn y) == y is a measurement where x serves as the input (sign), i.e., the first element, constituting the precondition in terms of available information and similar items"^^xs:string.
pims-ii:isMeasuredObjectIn a owl:ObjectProperty;
   rdfs:label "isMeasuredObjectIn"@en;
   rdfs:range pims-ii:Measurement;
   rdfs:subPropertyOf pims-ii:isObservedIn;
   rdfs:comment "(x isMeasuredObjectIn y) == y is a measurement where x acts as the object, i.e., the second element, that is subject to the measurement and for which a property is determined"^^xs:string.
pims-ii:isMeasurementOutcomeIn a owl:ObjectProperty;
   rdfs:label "isMeasurementOutcomeIn"@en;
   rdfs:range pims-ii:Measurement;
   rdfs:subPropertyOf pims-ii:isObservationOutcomeIn;
   rdfs:comment "(x isMeasurementOutcomeIn y) == y is a measurement where x is the measurement outcome, i.e., the third element (e.g., the value that is determined for the considered property of the measured object, the measurement error, and any other outcome)"^^xs:string.

# Metonymization
#
pims-ii:isOldReferentInMetonymization a owl:ObjectProperty;
   rdfs:label "isOldReferentInMetonymization"@en;
   rdfs:range pims-ii:Metonymization;
   rdfs:subPropertyOf pims-ii:isOldReferentIn;
   rdfs:comment "(x isOldReferentInMetonymization y) == y is a metonymization where x acts as the old referent, i.e., the first element; the old and the new referent need to have a causal connection"^^xs:string.
pims-ii:changesReferentInMetonymization a owl:ObjectProperty;
   rdfs:label "changesReferentInMetonymization"@en;
   rdfs:range pims-ii:Metonymization;
   rdfs:subPropertyOf pims-ii:changesReferentIn;
   rdfs:comment "(x changesReferentInMetonymization y) == y is a metonymization where x acts as the representamen, i.e., the second element"^^xs:string.
pims-ii:isNewReferentInMetonymization a owl:ObjectProperty;
   rdfs:label "isNewReferentInMetonymization"@en;
   rdfs:range pims-ii:Metonymization;
   rdfs:subPropertyOf pims-ii:isNewReferentIn;
   rdfs:comment "(x isNewReferentInMetonymization y) == y is a metonymization where x acts as the new referent, i.e., the third element; the old and the new referent need to have a causal connection"^^xs:string.

# Modelling
#
pims-ii:isModellingInputIn a owl:ObjectProperty;
   rdfs:label "isModellingInputIn"@en;
   rdfs:range pims-ii:Modelling;
   rdfs:subPropertyOf pims-ii:isSignInInterpretation;
   rdfs:comment "(x isModellingInputIn y) == y is a modelling (model construction or parameterization) step where x is the input (previous or unparameterized model, knowledge about the modelled system, etc.), i.e., the first element"^^xs:string.
pims-ii:isModelledIn a owl:ObjectProperty;
   rdfs:label "isModelledIn"@en;
   rdfs:range pims-ii:Modelling;
   rdfs:subPropertyOf pims-ii:isObjectInInterpretation;
   rdfs:comment "(x isModelledIn y) == y is a modelling (model construction or parameterization) step where x acts as the modelled object (system, substance, process, or similar), i.e., the second element"^^xs:string.
pims-ii:isModellingOutputIn a owl:ObjectProperty;
   rdfs:label "isModellingOutputIn"@en;
   rdfs:range pims-ii:Modelling;
   rdfs:subPropertyOf pims-ii:isInterpretantInInterpretation;
   rdfs:comment "(x isModellingOutputIn y) == y is a modelling (model construction or parameterization) step where x is the modelling output (e.g., a parameterized or improved model), i.e., the third element"^^xs:string.

# Observation
#
pims-ii:isObservationInputIn a owl:ObjectProperty;
   rdfs:label "isObservationInputIn"@en;
   rdfs:range pims-ii:Observation;
   rdfs:subPropertyOf pims-ii:isSignInPerception;
   rdfs:comment "(x isObservationInputIn y) == y is an observation where x designates input and/or advance knowledge relevant to the observation, i.e., the first element"^^xs:string.
pims-ii:isObservedIn a owl:ObjectProperty;
   rdfs:label "isObservedIn"@en;
   rdfs:range pims-ii:Observation;
   rdfs:subPropertyOf pims-ii:isPerceivedIn;
   rdfs:comment "(x isObservedIn y) == y is an observation where x acts as the observed object, i.e., the second element, for which the value of a property is to be determined"^^xs:string.
pims-ii:isObservationOutcomeIn a owl:ObjectProperty;
   rdfs:label "isObservationOutcomeIn"@en;
   rdfs:range pims-ii:Observation;
   rdfs:subPropertyOf pims-ii:isInterpretantInPerception;
   rdfs:comment "(x isObservationOutcomeIn y) == y is an observation where x is the observation outcome (the observed value of the target property), i.e., the third element"^^xs:string.

# Optimization
#
pims-ii:isOptimizationProblemIn a owl:ObjectProperty;
   rdfs:label "isOptimizationProblemIn"@en;
   rdfs:domain pims-ii:OptimizationProblem;
   rdfs:range pims-ii:Optimization;
   rdfs:subPropertyOf pims-ii:isSignInInterpretation, pims-ii:isAimIn;
   rdfs:comment "(x isOptimizationProblemIn y) == y is an optimization where x is the optimization problem, i.e., the first element."@en;
   skos:scopeNote "In (x isOptimizationProblemIn y), x is the aim/intention pursued by carrying out the optimization process y."@en.
pims-ii:isObjectInOptimization a owl:ObjectProperty;
   rdfs:label "isObjectInOptimization"@en;
   rdfs:range pims-ii:Optimization;
   rdfs:subPropertyOf pims-ii:isObjectInInterpretation;
   rdfs:comment "(x isObjectInOptimization y) == y is an optimization where x is that which the optimization is ultimately about, i.e., the second element"^^xs:string.
pims-ii:isOptimizationOutputIn a owl:ObjectProperty;
   rdfs:label "isOptimizationOutputIn"@en;
   rdfs:range pims-ii:Optimization;
   rdfs:subPropertyOf pims-ii:isInterpretantInInterpretation;
   rdfs:comment "(x isOptimizationOutputIn y) == y is an optimization where x is the optimization output, i.e., the third element"^^xs:string.
#
# variables occurring in optimization problems
#
pims-ii:isDesignParameterWithin a owl:ObjectProperty;
   rdfs:label "isDesignParameterWithin"@en;
   rdfs:domain pims-ii:Conventional;
   rdfs:range pims-ii:OptimizationProblem;
   rdfs:subPropertyOf pims-ii:isSemioticallyConstitutiveOf;
   rdfs:comment "(x isDesignParameterWithin y) == x is one of the parameters that make up the design space considered in the optimization problem y"@en.
pims-ii:isOptimizationObjectiveWithin a owl:ObjectProperty;
   rdfs:label "isOptimizationObjectiveWithin"@en;
   rdfs:domain pims-ii:Conventional;
   rdfs:range pims-ii:OptimizationProblem;
   rdfs:subPropertyOf pims-ii:isSemioticallyConstitutiveOf;
   rdfs:comment "(x isOptimizationObjectiveWithin y) == x is one of the optimization criteria that make up the objective space considered in the optimization problem y"@en.
pims-ii:isMaximizationObjectiveIn a owl:ObjectProperty;
   rdfs:label "isMaximizationObjectiveIn"@en;
   rdfs:domain pims-ii:Conventional;
   rdfs:range pims-ii:Optimization;
   rdfs:subPropertyOf pims-ii:isOptimizationObjectiveWithin;
   rdfs:comment "(x isMaximizationObjectiveIn y) == x is a maximization objective/criterion considered in the optimization problem y"@en.
pims-ii:isMinimizationObjectiveIn a owl:ObjectProperty;
   rdfs:label "isMaximizationObjectiveIn"@en;
   rdfs:domain pims-ii:Conventional;
   rdfs:range pims-ii:Optimization;
   rdfs:subPropertyOf pims-ii:isOptimizationObjectiveWithin;
   rdfs:comment "(x isMaximizationObjectiveIn y) == x is a maximization objective/criterion considered in the optimization problem y"@en.

# PartToWhole
#
pims-ii:isOldReferentInPartToWhole a owl:ObjectProperty;
   rdfs:label "isOldReferentInPartToWhole"@en;
   rdfs:range pims-ii:PartToWhole;
   rdfs:subPropertyOf pims-ii:isOldReferentInSynecdoche;
   rdfs:comment "(x isOldReferentInPartToWhole y) == y is a part-to-whole synecdoche where x acts as the old referent (the part), i.e., the first element"^^xs:string.
pims-ii:changesReferentInPartToWhole a owl:ObjectProperty;
   rdfs:label "changesReferentInPartToWhole"@en;
   rdfs:range pims-ii:PartToWhole;
   rdfs:subPropertyOf pims-ii:changesReferentInSynecdoche;
   rdfs:comment "(x changesReferentInPartToWhole y) == y is a part-to-whole synecdoche where x acts as the representamen, i.e., the second element"^^xs:string.
pims-ii:isNewReferentInPartToWhole a owl:ObjectProperty;
   rdfs:label "isNewReferentInPartToWhole"@en;
   rdfs:range pims-ii:PartToWhole;
   rdfs:subPropertyOf pims-ii:isNewReferentInSynecdoche;
   rdfs:comment "(x isNewReferentInPartToWhole y) == y is a part-to-whole synecdoche where x acts as the new referent (the whole), i.e., the third element"^^xs:string.

# Perception
#
pims-ii:isSignInPerception a owl:ObjectProperty;
   rdfs:label "isSignInPerception"@en;
   rdfs:range pims-ii:Perception;
   rdfs:subPropertyOf pims-ii:isSignIn;
   rdfs:comment "(x isSignInPerception y) == y is a perception where x acts as the sign, i.e., the first element"^^xs:string.
pims-ii:isPerceivedIn a owl:ObjectProperty;
   rdfs:label "isPerceivedIn"@en;
   rdfs:range pims-ii:Perception;
   rdfs:subPropertyOf pims-ii:isObjectIn, pims-ii:isParticipantInCognition;
   rdfs:comment "(x isPerceivedIn y) == y is a perception where x acts as the perceived object, i.e., the second element; the perceived object is a (mereotopological) participant of the perception, in other words, it needs to be physically present so that it can be perceived"^^xs:string.
pims-ii:isInterpretantInPerception a owl:ObjectProperty;
   rdfs:label "isInterpretantInPerception"@en;
   rdfs:range pims-ii:Perception;
   rdfs:subPropertyOf pims-ii:isInterpretantIn;
   rdfs:comment "(x isInterpretantInPerception y) == y is a perception where x acts as the interpretant, i.e., the third element"^^xs:string.

# Planning
#
pims-ii:isTelosInPlanning a owl:ObjectProperty;
   rdfs:label "isTelosInPlanning"@en;
   rdfs:range pims-ii:Planning;
   rdfs:subPropertyOf pims-ii:isTelosIn, pims-ii:isSignInPerception;
   rdfs:comment "(x isTelosInPlanning y) == y is a telesis carried out in advance of potentially undertaking an action, where x acts as the telos (initial guiding objective), i.e., the first element"^^xs:string.
pims-ii:isSituationInPlanning a owl:ObjectProperty;
   rdfs:label "isSituationInPlanning"@en;
   rdfs:range pims-ii:Planning;
   rdfs:subPropertyOf pims-ii:isObjectInTelesis, pims-ii:isPerceivedIn;
   rdfs:comment "(x isSituationInPlanning y) == y is a telesis carried out in advance of potentially undertaking an action, where x is the perceived present situation, i.e., the second element, against which the telos is evaluated"^^xs:string.
pims-ii:isResolutionInPlanning a owl:ObjectProperty;
   rdfs:label "isResolutionInPlanning"@en;
   rdfs:range pims-ii:Planning;
   rdfs:subPropertyOf pims-ii:isResolutionInTelesis, pims-ii:isInterpretantInPerception;
   rdfs:comment "(x isResolutionInPlanning y) == y is a telesis carried out in advance of potentially undertaking an action, where x is the planning outcome, i.e., the third element"^^xs:string.

# Selection
#
pims-ii:isSelectionInputIn a owl:ObjectProperty;
   rdfs:label "isSelectionInputIn"@en;
   rdfs:range pims-ii:Selection;
   rdfs:subPropertyOf pims-ii:isInformationProcessingInputIn;
   rdfs:comment "(x isSelectionInputIn y) == y is a selection where x is the input (initially given information), i.e., the first element; n.b., in a selection, the output needs to be constitutive of the input"^^xs:string.
pims-ii:isObjectInSelection a owl:ObjectProperty;
   rdfs:label "isObjectInSelection"@en;
   rdfs:range pims-ii:Selection;
   rdfs:subPropertyOf pims-ii:isObjectInInformationProcessing;
   rdfs:comment "(x isObjectInSelection y) == y is a selection where x is the object that the input and the output both represent, i.e., the second element"^^xs:string.
pims-ii:isSelectionOutputIn a owl:ObjectProperty;
   rdfs:label "isSelectionOutputIn"@en;
   rdfs:range pims-ii:Selection;
   rdfs:subPropertyOf pims-ii:isInformationProcessingOutputIn;
   rdfs:comment "(x isSelectionOutputIn y) == y is a selection where x is the output (retained information), i.e., the third element; n.b., in a selection, the output needs to be constitutive of the input"^^xs:string.
pims-ii:isSelectionConditionIn a owl:ObjectProperty;
   rdfs:label "isSelectionConditionIn"@en;
   rdfs:domain pims-ii:Proposition;
   rdfs:range pims-ii:Selection;
   rdfs:subPropertyOf pims-ii:isRepresentamenFor;
   rdfs:comment "(x isSelectionConditionIn y) == in the selection process y, the condition x controls what constitutive element(s) of the input are retained as part of the output"^^xs:string.

# SemanticChange
#
pims-ii:isOldReferentIn a owl:ObjectProperty;
   rdfs:label "isOldReferentIn"@en;
   rdfs:range pims-ii:SemanticChange;
   rdfs:subPropertyOf pims-ii:isFirstElementIn, pims-ii:isReferentIn;
   rdfs:comment "(x isOldReferentIn y) == y is a semantic change where x acts as the old referent, i.e., the first element"^^xs:string.
pims-ii:changesReferentIn a owl:ObjectProperty;
   rdfs:label "changesReferentIn"@en;
   rdfs:range pims-ii:SemanticChange;
   rdfs:subPropertyOf pims-ii:isSecondElementIn, pims-ii:isRepresentamenIn;
   rdfs:comment "(x changesReferentIn y) == y is a semantic change where x acts as the representamen, i.e., the second element"^^xs:string.
pims-ii:isNewReferentIn a owl:ObjectProperty;
   rdfs:label "isNewReferentIn"@en;
   rdfs:range pims-ii:SemanticChange;
   rdfs:subPropertyOf pims-ii:isThirdElementIn, pims-ii:isReferentIn;
   rdfs:comment "(x isNewReferentIn y) == y is a semantic change where x acts as the new referent, i.e., the third element"^^xs:string.

# Semiosis
#
pims-ii:isSignIn a owl:ObjectProperty;
   rdfs:label "isSignIn"@en;
   rdfs:range pims-ii:Semiosis;
   rdfs:subPropertyOf pims-ii:isFirstElementIn, pims-ii:isRepresentamenIn;
   rdfs:comment "(x isSignIn y) == y is a semiosis where x acts as the sign, i.e., the first element"^^xs:string.
pims-ii:isObjectIn a owl:ObjectProperty;
   rdfs:label "isObjectIn"@en;
   rdfs:range pims-ii:Semiosis;
   rdfs:subPropertyOf pims-ii:isSecondElementIn, pims-ii:isReferentIn;
   rdfs:comment "(x isObjectIn y) == y is a semiosis where x acts as the object, i.e., the second element"^^xs:string.
pims-ii:isInterpretantIn a owl:ObjectProperty;
   rdfs:label "isInterpretantIn"@en;
   rdfs:range pims-ii:Semiosis;
   rdfs:subPropertyOf pims-ii:isThirdElementIn, pims-ii:isRepresentamenIn;
   rdfs:comment "(x isInterpretantIn y) == y is a semiosis where x acts as the interpretant, i.e., the third element"^^xs:string.

# Simulation
#
pims-ii:isSimulationInputIn a owl:ObjectProperty;
   rdfs:label "isSimulationInputIn"@en;
   rdfs:range pims-ii:Simulation;
   rdfs:subPropertyOf pims-ii:isSignInInterpretation;
   rdfs:comment "(x isSimulationInputIn y) == y is a simulation where x is the simulation input (model, etc.), i.e., the first element"^^xs:string.
pims-ii:isSimulatedIn a owl:ObjectProperty;
   rdfs:label "isSimulatedIn"@en;
   rdfs:range pims-ii:Simulation;
   rdfs:subPropertyOf pims-ii:isObjectInInterpretation;
   rdfs:comment "(x isSimulatedIn y) == y is a simulation where x acts as the simulated object (system, substance, process, or similar), i.e., the second element"^^xs:string.
pims-ii:isSimulationOutputIn a owl:ObjectProperty;
   rdfs:label "isSimulationOutputIn"@en;
   rdfs:range pims-ii:Simulation;
   rdfs:subPropertyOf pims-ii:isInterpretantInInterpretation;
   rdfs:comment "(x isSimulationOutputIn y) == y is a simulation where x is the simulation output (computed property, higher-level model, or similar), i.e., the third element"^^xs:string.

# Steering
#
pims-ii:isTelosInSteering a owl:ObjectProperty;
   rdfs:label "isTelosInSteering"@en;
   rdfs:range pims-ii:Steering;
   rdfs:subPropertyOf pims-ii:isTelosIn, pims-ii:isSignInPerception;
   rdfs:comment "(x isTelosInSteering y) == y is a steering operation (reflection in actu) where x acts as the telos (initial guiding objective), i.e., the first element"^^xs:string.
pims-ii:isActionInSteering a owl:ObjectProperty;
   rdfs:label "isActionInSteering"@en;
   rdfs:domain pims-ii:Action;
   rdfs:range pims-ii:Steering;
   rdfs:subPropertyOf pims-ii:isObjectInTelesis, pims-ii:isPerceivedIn, [owl:inverseOf pims-ii:isProperParticipantIn];
   rdfs:comment "(x isActionInSteering y) == y is a steering operation (reflection in actu) where x is an ongoing action, i.e., the second element, against which the telos is evaluated"^^xs:string.
pims-ii:isResolutionInSteering a owl:ObjectProperty;
   rdfs:label "isResolutionInSteering"@en;
   rdfs:range pims-ii:Steering;
   rdfs:subPropertyOf pims-ii:isResolutionInTelesis, pims-ii:isInterpretantInPerception;
   rdfs:comment "(x isResolutionInSteering y) == y is a steering operation (reflection in actu) where x is the resolution, i.e., the third element"^^xs:string.

# Synecdoche
#
pims-ii:isOldReferentInSynecdoche a owl:ObjectProperty;
   rdfs:label "isOldReferentInSynecdoche"@en;
   rdfs:range pims-ii:Synecdoche;
   rdfs:subPropertyOf pims-ii:isOldReferentInMetonymization;
   rdfs:comment "(x isOldReferentInSynecdoche y) == y is a synecdoche where x acts as the old referent, i.e., the first element; the old and the new referent need to have a causal connection (n.b., the mereological relation in terms of proper parthood as such is insufficient)"^^xs:string.
pims-ii:changesReferentInSynecdoche a owl:ObjectProperty;
   rdfs:label "changesReferentInSynecdoche"@en;
   rdfs:range pims-ii:Synecdoche;
   rdfs:subPropertyOf pims-ii:changesReferentInMetonymization;
   rdfs:comment "(x changesReferentInSynecdoche y) == y is a synecdoche where x acts as the representamen, i.e., the second element"^^xs:string.
pims-ii:isNewReferentInSynecdoche a owl:ObjectProperty;
   rdfs:label "isNewReferentInSynecdoche"@en;
   rdfs:range pims-ii:Synecdoche;
   rdfs:subPropertyOf pims-ii:isNewReferentInMetonymization;
   rdfs:comment "(x isNewReferentInSynecdoche y) == y is a synecdoche where x acts as the new referent, i.e., the third element; the old and the new referent need to have a causal connection (n.b., the mereological relation in terms of proper parthood as such is insufficient)"^^xs:string.

# Telesis
#
pims-ii:isTelosIn a owl:ObjectProperty;
   rdfs:label "isTelosIn"@en;
   rdfs:domain pims-ii:Intention;
   rdfs:range pims-ii:Telesis;
   rdfs:subPropertyOf pims-ii:isSignIn;
   rdfs:comment "(x isTelosIn y) == y is a telesis where x acts as the telos (initial guiding objective), i.e., the first element"^^xs:string.
pims-ii:isObjectInTelesis a owl:ObjectProperty;
   rdfs:label "isObjectInTelesis"@en;
   rdfs:range pims-ii:Telesis;
   rdfs:subPropertyOf pims-ii:isObjectIn;
   rdfs:comment "(x isObjectInTelesis y) == y is a telesis where x acts as the object (action, claim, or situation against which an objective is evaluated), i.e., the second element"^^xs:string.
pims-ii:isResolutionInTelesis a owl:ObjectProperty;
   rdfs:label "isResolutionInTelesis"@en;
   rdfs:domain pims-ii:Intention;
   rdfs:range pims-ii:Telesis;
   rdfs:subPropertyOf pims-ii:isInterpretantIn;
   rdfs:comment "(x isResolutionInTelesis y) == y is a telesis where x acts as the resolution (a plan, revised objective, or other comparable sort of evaluation outcome), i.e., the third element"^^xs:string.

# TriadicCognition
#
pims-ii:isFirstElementIn a owl:ObjectProperty;
   rdfs:label "isFirstElementIn"@en;
   skos:altLabel "\\dot{E}"@en;
   rdfs:range pims-ii:TriadicCognition;
   rdfs:subPropertyOf pims-ii:isRepresentationalElementIn;
   rdfs:comment "(x isFirstElementIn y) means that x acts as the first element in y, which is a triadic cognition"@en.
pims-ii:isSecondElementIn a owl:ObjectProperty;
   rdfs:label "isSecondElementIn"@en;
   skos:altLabel "\\ddot{E}"@en;
   rdfs:range pims-ii:TriadicCognition;
   rdfs:subPropertyOf pims-ii:isRepresentationalElementIn;
   rdfs:comment "(x isSecondElementIn y) means that x acts as the second element in y, which is a triadic cognition"@en.
pims-ii:isThirdElementIn a owl:ObjectProperty;
   rdfs:label "isThirdElementIn"@en;
   skos:altLabel "\\dddot{E}"@en;
   rdfs:range pims-ii:TriadicCognition;
   rdfs:subPropertyOf pims-ii:isRepresentationalElementIn;
   rdfs:comment "(x isThirdElementIn y) means that x acts as the third element in y, which is a triadic cognition"@en.

# Undertaking
#
pims-ii:isSituationInUndertaking a owl:ObjectProperty;
   rdfs:label "isSituationInUndertaking"@en;
   rdfs:range pims-ii:Undertaking;
   rdfs:subPropertyOf pims-ii:isOldReferentInMetonymization;
   rdfs:comment "(x isSituationInUndertaking y) == y is an undertaking wherein x is the pre-existing situation, i.e., the first element"^^xs:string.
pims-ii:isResolutionInUndertaking a owl:ObjectProperty;
   rdfs:label "isResolutionInUndertaking"@en;
   rdfs:domain pims-ii:Intention;
   rdfs:range pims-ii:Undertaking;
   rdfs:subPropertyOf pims-ii:changesReferentInMetonymization;
   rdfs:comment "(x isResolutionInUndertaking y) == y is an undertaking where x is the resolution (obtained from a previous telesis), i.e., the second element"^^xs:string.
pims-ii:isActionInUndertaking a owl:ObjectProperty;
   rdfs:label "isActionInUndertaking"@en;
   rdfs:domain pims-ii:Action;
   rdfs:range pims-ii:Undertaking;
   rdfs:subPropertyOf pims-ii:isNewReferentInMetonymization, [owl:inverseOf pims-ii:temporallyPrecedes];
   rdfs:comment "(x isActionInUndertaking y) == y is an undertaking where x is the action that is undertaken, i.e., the third element"^^xs:string.

# Validation
#
pims-ii:isTelosInValidation a owl:ObjectProperty;
   rdfs:label "Validation"@en;
   rdfs:range pims-ii:Validation;
   rdfs:subPropertyOf pims-ii:isTelosInEvaluation;
   rdfs:comment "(x isTelosInValidation y) means that y is a validation where x acts as the telos (initial guiding objective), i.e., the first element"@en.
pims-ii:isValidatedIn a owl:ObjectProperty;
   rdfs:label "isEvaluatedIn"@en;
   rdfs:domain pims-ii:CognitiveAction;
   rdfs:range pims-ii:Validation;
   rdfs:subPropertyOf pims-ii:isEvaluatedIn;
   rdfs:comment "(x isValidatedIn y) means that y is a validation where x is the cognitive action undergoing validation, i.e., the second element"@en.
pims-ii:isValidationOutcomeIn a owl:ObjectProperty;
   rdfs:label "isValidationOutcomeIn"@en;
   rdfs:domain pims-ii:ValidityClaim;
   rdfs:range pims-ii:Validation;
   rdfs:subPropertyOf pims-ii:isEvaluationOutcomeIn;
   rdfs:comment"(x isValidationOutcomeIn y) means that x is the validity claim, i.e., the third element, obtained as an interpretant from the validation y"@en.

# Visualization
#
pims-ii:isVisualizationInputIn a owl:ObjectProperty;
   rdfs:label "isVisualizationInputIn"@en;
   rdfs:range pims-ii:Visualization;
   rdfs:subPropertyOf pims-ii:isSignInInterpretation;
   rdfs:comment "(x isVisualizationInputIn y) == y is a visualization process where x is the input (a pre-existing representamen for the visualized object, e.g., a simulation result), i.e., the first element"^^xs:string.
pims-ii:isVisualizedObjectIn a owl:ObjectProperty;
   rdfs:label "isVisualizedObjectIn"@en;
   rdfs:range pims-ii:Visualization;
   rdfs:subPropertyOf pims-ii:isObjectInInterpretation;
   rdfs:comment "(x isVisualizedObjectIn y) == y is a visualization process wherein x is the visualized object, i.e., the second element"^^xs:string.
pims-ii:isVisualizationOutputIn a owl:ObjectProperty;
   rdfs:label "isVisualizationOutputIn"@en;
   rdfs:range pims-ii:Visualization;
   rdfs:subPropertyOf pims-ii:isInterpretantInInterpretation;
   rdfs:comment "(x isVisualizationOutputIn y) == y is a visualization where x is the visualization output, i.e., the third element"^^xs:string.

# WholeToPart
#
pims-ii:isOldReferentInWholeToPart a owl:ObjectProperty;
   rdfs:label "isOldReferentInWholeToPart"@en;
   rdfs:range pims-ii:WholeToPart;
   rdfs:subPropertyOf pims-ii:isOldReferentInSynecdoche;
   rdfs:comment "(x isOldReferentInWholeToPart y) == y is a whole-to-part synecdoche where x acts as the old referent (the whole), i.e., the first element"^^xs:string.
pims-ii:changesReferentInWholeToPart a owl:ObjectProperty;
   rdfs:label "changesReferentInWholeToPart"@en;
   rdfs:range pims-ii:WholeToPart;
   rdfs:subPropertyOf pims-ii:changesReferentInSynecdoche;
   rdfs:comment "(x changesReferentInWholeToPart y) == y is a whole-to-part synecdoche where x acts as the representamen, i.e., the second element"^^xs:string.
pims-ii:isNewReferentInWholeToPart a owl:ObjectProperty;
   rdfs:label "isNewReferentInWholeToPart"@en;
   rdfs:range pims-ii:WholeToPart;
   rdfs:subPropertyOf pims-ii:isNewReferentInSynecdoche;
   rdfs:comment "(x isNewReferentInWholeToPart y) == y is a whole-to-part synecdoche where x acts as the new referent (the part), i.e., the third element"^^xs:string.

########################################
# CORE MEREOSEMIOTICS: OTHER RELATIONS #
########################################

pims-ii:articulates a owl:ObjectProperty;
   rdfs:label "articulates"@en;
   skos:altLabel "\\lhd_a"@en;
   rdfs:domain pims-ii:Articulation;
   rdfs:range pims-ii:Proposition;
   rdfs:subPropertyOf pims-ii:isSemioticMemberOf;
   rdfs:comment "(x articulates y) means that x is a semiotic member of the proposition y, giving a literal or non-literal (e.g., spoken) expression to its propositional content; n.b., x may also express other propositions beside y"@en.

pims-ii:articulatesLiterally a owl:ObjectProperty;
   rdfs:label "articulatesLiterally"@en;
   rdfs:domain pims-ii:CollectiveLiteral;
   rdfs:range pims-ii:Proposition;
   rdfs:subPropertyOf pims-ii:articulates;
   rdfs:comment "(x articulatesLiterally y) means that x is a collective literal expressing the proposition y, and possibly additional propositions beside y"^^xs:string.

pims-ii:articulatesNonliterally a owl:ObjectProperty;
   rdfs:label "articulatesNonliterally"@en;
   rdfs:domain pims-ii:Articulation, [owl:complementOf pims-ii:CollectiveLiteral];
   rdfs:range pims-ii:Proposition;
   rdfs:subPropertyOf pims-ii:articulates;
   rdfs:comment "(x articulatesNonliterally y) means that x is a collective non-literal expression (e.g., an utterance) of proposition y, and possibly additional propositions beside y"^^xs:string.

pims-ii:directlyGrounds a owl:ObjectProperty;
   rdfs:label "directlyGrounds"@en;
   skos:altLabel "\\hookrightarrow"@en;
   rdfs:domain [owl:unionOf (pims-ii:TriadicCognition pims-ii:Presupposition)];
   rdfs:range pims-ii:CognitiveStep;
   rdfs:subPropertyOf pims-ii:directlyPrecedesCognitiveStep, pims-ii:logicallyPrecedes;
   owl:propertyChainAxiom (pims-ii:isGroundingStepIn [owl:inverseOf pims-ii:isGroundedStepIn]);
   rdfs:comment "(x directlyGrounds y) == x is the cognitive step (or basic ground) that directly precedes y logically, such that a dyadic representation relation from y is taken over from x (or assumed to be grounded a priori due to x)"^^xs:string.

pims-ii:directlyPrecedesByRupture a owl:ObjectProperty;
   rdfs:label "directlyPrecedesByRupture"@en;
   rdfs:domain pims-ii:CognitiveStep;
   rdfs:range pims-ii:CognitiveStep;
   rdfs:subPropertyOf pims-ii:directlyPrecedesCognitiveStep;
   rdfs:comment "(x directlyPrecedesByRupture y) == x is the cognitive step that directly precedes y logically (and typically, y takes over a dyadic representation relation from x), but either x or y constitutes a cognitive rupture, i.e., it interrupts the chain of grounding"^^xs:string.

pims-ii:directlyPrecedesCognitiveStep a owl:ObjectProperty;
   rdfs:label "directlyPrecedesCognitiveStep"@en;
   rdfs:subPropertyOf pims-ii:directlyPrecedesStep;
   rdfs:comment "(x directlyPrecedesCognitiveStep y) == x is the cognitive step (or basic ground) that directly precedes y logically; typically, this means that y takes over a dyadic representation relation from x"^^xs:string.

pims-ii:hasCausalConnectionWith a owl:ObjectProperty, owl:ReflexiveProperty, owl:SymmetricProperty, owl:TransitiveProperty;
   rdfs:label "hasCausalConnectionWith"@en;
   skos:altLabel "\\dot{C}^\\star"@en;
   rdfs:subPropertyOf pims-ii:isMereosemioticallyRelatedTo;
   owl:propertyChainAxiom (pims-ii:isOldReferentInMetonymization [owl:inverseOf pims-ii:isNewReferentInMetonymization]);
   owl:propertyChainAxiom (pims-ii:isNewReferentInMetonymization [owl:inverseOf pims-ii:isOldReferentInMetonymization]);
   rdfs:comment "'Real causal connection' relation following Peirce, here, given by the transitive closure of 'hasDirectCausalConnectionWith'"@en;
   skos:scopeNote "this is to be understood broadly, as in Peirce, and can be a very indirect connection; here, this is relevant as follows: a) in a grounded cognition, there are only dyadic representation relations between representamina and their referents that have a real causal connection with each other; b) in a metonymization, there must be a real causal connection between the old and the new referent"@en.

pims-ii:hasDirectCausalConnectionWith a owl:ObjectProperty, owl:ReflexiveProperty, owl:SymmetricProperty;
   rdfs:label "hasDirectCausalConnectionWith"@en;
   skos:altLabel "\\dot{C}"@en;
   rdfs:subPropertyOf pims-ii:hasCausalConnectionWith;
   rdfs:comment "Direct causal connection (in a broad sense)"@en;
   skos:scopeNote "in particular, x and y are directly causally connected if (x isParticipantIn y), or if x and y are both steps in a process where x directly precedes y; however, spatiotemporal parthood is not enough to justify causal connectedness - x must actually play a role in bringing about y, or vice versa"@en.

pims-ii:hasNegation a owl:ObjectProperty;
   rdfs:label "hasNegation"@en;
   rdfs:domain pims-ii:RelationalIRI;
   rdfs:range pims-ii:RelationalIRI;
   rdfs:subPropertyOf pims-ii:isSemioticallyConstitutiveOf;
   rdfs:comment "(x hasNegation y) means that x and y are IRIs that can possibly occur in the predicate (middle) position of a triple, and that y is 'not x'; n.b., this is not a symmetrical relation, since 'not not x' is syntactically different from x"^^xs:string.

pims-ii:hasRepresentamen a owl:ObjectProperty;
   rdfs:label "hasRepresentamen"@en;
   skos:altLabel "R^-"@en;
   rdfs:subPropertyOf pims-ii:msHRHPIP, pims-ii:msHPIPHR, pims-ii:msHRIRHR;
   owl:inverseOf pims-ii:isRepresentamenFor;
   owl:propertyChainAxiom (pims-ii:isReferentIn [owl:inverseOf pims-ii:isRepresentamenIn]);
   rdfs:comment "Dyadic representation relation; (x hasRepresentamen y) means that there is a cognitive step z such that (x isReferentIn z) and (y isRepresentamenIn z)"@en.

pims-ii:isAdmissibleUnitFor a owl:ObjectProperty;
   rdfs:label "isAdmissibleUnitFor"@en;
   rdfs:domain pims-ii:MeasurementUnit;
   rdfs:range pims-ii:Variable;
   rdfs:subPropertyOf pims-ii:msHPIPIR;
   rdfs:comment "(x isAdmissibleUnitFor y) means that x is a unit that can be associated with the variable y; subsumption under msHPIPIR is explained as follows: There is a sign z for the variable y (where z is a description of admissible values of y) of which x is constitutive (and with which x hence overlaps)"^^xs:string.

pims-ii:isAdmissibleValueFor a owl:ObjectProperty;
   rdfs:label "isAdmissibleValueFor"@en;
   rdfs:domain pims-ii:Value;
   rdfs:range pims-ii:Term;
   rdfs:subPropertyOf pims-ii:msIPIRIR;
   rdfs:comment "(x isAdmissibleValueFor y) means that y is a term that could in principle evaluate to the value x; subsumption under msIPIRIR is explained as follows: There is a sign z for the term y (where z is the range of admissible values of y), for which in turn there is another sign z' (where z' lists members of z, explicitly including x) of which x is a part"^^xs:string.

pims-ii:isAntecedentWithin a owl:ObjectProperty;
   rdfs:label "isAntecedentWithin"@en;
   rdfs:domain pims-ii:Proposition;
   rdfs:range pims-ii:Rule;
   rdfs:subPropertyOf pims-ii:isSemioticallyConstitutiveOf;
   rdfs:comment "(x isAntecedentWithin y) means that x is the antecedent from the rule y"^^xs:string.

pims-ii:isAssertedBy a owl:ObjectProperty;
   rdfs:label "isAssertedBy"@en;
   skos:altLabel "B"@en;
   rdfs:domain pims-ii:Claim;
   rdfs:range pims-ii:Interlocutor;
   rdfs:subPropertyOf pims-ii:isExpressedBy;
   owl:propertyChainAxiom (pims-ii:isAssertedIn [owl:inverseOf pims-ii:isSpeakerIn]);
   rdfs:comment "(x isAssertedBy y) means that x is a claim that is affirmatively expressed/stated/uttered by the interlocutor y"@en.

pims-ii:isAssertedIn a owl:ObjectProperty;
   rdfs:label "isAssertedIn"@en;
   rdfs:domain pims-ii:Claim;
   rdfs:range pims-ii:ExpressiveAct;
   rdfs:subPropertyOf pims-ii:isExpressedIn;
   rdfs:comment "(x isAssertedIn y) means that x is a claim that is affirmatively expressed/stated/uttered in the expressive act y (by its speaker)"@en.

pims-ii:isAssessmentFor a owl:ObjectProperty;
   rdfs:label "isAssessmentFor"@en;
   rdfs:domain pims-ii:Assessment;
   rdfs:range pims-ii:CognitiveStep;
   rdfs:subPropertyOf pims-ii:isGroundFor;
   rdfs:comment "(g isAssessmentFor y) means that g is a ground for the cognitive step y, explaining how y is grounded in a way that provides a proposition on its validity, accuracy, and/or reliability, relating it to that of the previous step that directly grounds y"^^xs:string.

pims-ii:isAssignmentFor a owl:ObjectProperty;
   rdfs:label "isAssignmentFor"@en;
   skos:altLabel "\\hat{A}_D"@en;
   rdfs:domain pims-ii:Assignment;
   rdfs:subPropertyOf pims-ii:isAbout;
   rdfs:comment "(d isAssignmentFor o) means that d: x = y is an assignment that refers to o"@en;
   skos:example "e.g., x may be thermodynamic temperature, y may be a temperature value, and o may be an object of which the temperature has been measured"@en.

pims-ii:isCausallyDisconnectedFrom a owl:ObjectProperty, owl:SymmetricProperty;
   rdfs:label "isCausallyDisconnectedFrom"@en;
   rdfs:subPropertyOf pims-ii:isMereosemioticallyRelatedTo;
   rdfs:comment "(x isCausallyDisconnectedFrom y) means that between x and y there is no 'real causal connection' in the Peircean sense; therefore, x and y cannot be the old and new referents in a metonymization; similarly, x cannot act as a representamen for y in a grounded cognition (if it does, then the cognition is not grounded)"^^xs:string.

pims-ii:isClaimOf a owl:ObjectProperty;
   rdfs:label "isClaimOf"@en;
   rdfs:domain pims-ii:Claim;
   rdfs:range pims-ii:IntelligentAgent;
   rdfs:subPropertyOf pims-ii:overlapsWith;
   rdfs:comment "(x isClaimOf y) means that the x is a proposition that has some kind of belief-like or knowledge-like epistemic status for the intelligent agent y"@en;
   skos:scopeNote "the agent y explicitly stores x, hence requiring spatiotemporal overlap between x and y"@en.

pims-ii:isCognitiveSubstepOf a owl:ObjectProperty;
   rdfs:label "isCognitiveSubstepOf"@en;
   rdfs:domain pims-ii:CognitiveStep;
   rdfs:range pims-ii:CognitiveStep, pims-ii:CognitiveChain;
   rdfs:subPropertyOf pims-ii:isStepInCognitiveChain;
   rdfs:comment "In certain cases, multiple cognitive steps can be combined to yield one; e.g., the substep a: s - o - s' and the substep b: s' - o - s'' can be combined to yield a single triad, (a o b) = c: s - o - s''; in that case, c can be an element of a higher-order cognitive chain (of which it is a step), and a and b are its cognitive substeps"^^xs:string.

pims-ii:isConsequentWithin a owl:ObjectProperty;
   rdfs:label "isConsequentWithin"@en;
   rdfs:domain pims-ii:Proposition;
   rdfs:range pims-ii:Rule;
   rdfs:subPropertyOf pims-ii:isSemioticallyConstitutiveOf;
   rdfs:comment "(x isConsequentWithin y) means that x is a consequent from the rule y"^^xs:string.

pims-ii:isConstitutiveOf a owl:ObjectProperty;
   rdfs:label "isConstitutiveOf"@en;
   skos:altLabel "\\ddot{C}"@en;
   rdfs:subPropertyOf pims-ii:hasDirectCausalConnectionWith, pims-ii:overlapsWith, pims-ii:underlies;
   owl:propertyChainAxiom (pims-ii:isSelectionOutputIn [owl:inverseOf pims-ii:isSelectionInputIn]);
   owl:propertyChainAxiom (pims-ii:isAccumulationInputIn [owl:inverseOf pims-ii:isAccumulationOutputIn]);
   owl:propertyChainAxiom (pims-ii:isIncludedInAccumulation [owl:inverseOf pims-ii:isAccumulationOutputIn]);
   rdfs:comment "(x isConstitutiveOf y) means that, by virtue of an interaction requiring spatiotemporal overlap, x contributes causally to y fulfilling a certain function, exhibiting certain properties, or relating to other objects in the way it does, thereby creating a direct causal connection between x and y"@en.

pims-ii:isExpressedBy a owl:ObjectProperty;
   rdfs:label "isExpressedBy"@en;
   skos:altLabel "\\dot{B}"@en;
   rdfs:range pims-ii:Interlocutor;
   rdfs:subPropertyOf pims-ii:overlapsWith;
   owl:propertyChainAxiom (pims-ii:isExpressedIn [owl:inverseOf pims-ii:isSpeakerIn]);
   rdfs:comment "(x isExpressedBy y) means that x is expressed/stated/uttered by the interlocutor y; n.b., this does not necessarily mean that y affirms x (for that, use the subproperty isAssertedBy)"^^xs:string.

pims-ii:isExpressedIn a owl:ObjectProperty;
   rdfs:label "isExpressedIn"@en;
   rdfs:range pims-ii:ExpressiveAct;
   rdfs:subPropertyOf pims-ii:isParticipantInCognition;
   rdfs:comment "(x isExpressedIn y) means that x is expressed/stated/uttered in the expressive act y (by its speaker), possibly but not necessarily in an affirmative way"^^xs:string.

pims-ii:isFirstInDyad a owl:ObjectProperty;
   rdfs:label "isFirstInDyad"@en;
   skos:altLabel "\\dot{E}_D"@en;
   rdfs:domain pims-ii:Conventional;
   rdfs:range pims-ii:Dyad;
   rdfs:subPropertyOf pims-ii:isSemioticallyConstitutiveOf;
   rdfs:comment "(x isFirstInDyad d) means that x is the first element of the dyad d"^^xs:string.

pims-ii:isGroundFor a owl:ObjectProperty;
   rdfs:label "isGroundFor"@en;
   skos:altLabel "\\ddot{R}"@en;
   rdfs:domain pims-ii:Ground;
   rdfs:range pims-ii:CognitiveStep;
   rdfs:subPropertyOf pims-ii:isAbout;
   owl:propertyChainAxiom (pims-ii:isGroundingPropositionIn [owl:inverseOf pims-ii:isGroundedStepIn]);
   owl:propertyChainAxiom (pims-ii:groundsPresentStepIn [owl:inverseOf pims-ii:isPresentStepInGrounding]);
   rdfs:comment "(g isGroundFor y) means that g is a representamen for the cognitive step y, explaining how y is grounded"@en;
   skos:scopeNote "for g isGroundFor y, where x grounds y, there is a grounding metonymization where x is the old referent and y is the new referent of g"@en.

pims-ii:isHeldBy a owl:ObjectProperty;
   rdfs:label "isHeldBy"@en;
   rdfs:domain pims-ii:Claim;
   rdfs:range pims-ii:KnowledgeBase;
   rdfs:subPropertyOf pims-ii:isAssertedBy;
   rdfs:comment "(x isHeldBy y) means that the claim x is consistently asserted by the knowledge base y whenever it is queried about it; if y extends significantly through time and changes opinion about x (i.e., it does not assert it consistently over the whole time), it cannot be said to hold x as a claim, merely to assert it; in this case, it may be advisable to define a (temporal) part y' of y which can then be said to hold x as a claim"^^xs:string.

pims-ii:isJustificationFor a owl:ObjectProperty;
   rdfs:label "isJustificationFor"@en;
   rdfs:domain pims-ii:GroundingChain;
   rdfs:range pims-ii:GroundedCognition;
   rdfs:subPropertyOf pims-ii:isRepresentamenFor;
   rdfs:comment "(x isJustificationFor y) means that x is a grounding chain that provides epsitemic grounding for the cognition y, which thereby becomes a grounded cognition"^^xs:string.

pims-ii:isLeftHandSideIn a owl:ObjectProperty;
   rdfs:label "isLeftHandSideIn"@en;
   skos:altLabel "\\dot{E}_="@en;
   rdfs:domain pims-ii:Term;
   rdfs:range pims-ii:EqualityArticulation;
   rdfs:subPropertyOf pims-ii:isFirstInDyad;
   rdfs:comment "(x isLeftHandSideIn a) mans that a: x = y is an equality articulation with the term x as its left-hand side"^^xs:string.

pims-ii:isMagnitudeOf a owl:ObjectProperty;
   rdfs:label "isMagnitudeOf"@en;
   rdfs:domain pims-ii:Number;
   rdfs:range pims-ii:Value;
   rdfs:subPropertyOf pims-ii:isSemioticallyConstitutiveOf;
   rdfs:comment "(x isMagnitudeOf y) means that x is the numerical magnitude of y, e.g., in 200 kPa, x would be 200"^^xs:string.

pims-ii:isMemberOfPlurality a owl:ObjectProperty;
   rdfs:label "isMemberOfPlurality"@en;
   skos:altLabel "\\lhd_p"@en;
   rdfs:domain [owl:complementOf [owl:unionOf (pims-ii:Plurality pims-ii:Structure)]];
   rdfs:range pims-ii:Plurality;
   rdfs:subPropertyOf pims-ii:isSemioticMemberOf;
   rdfs:comment "(x isMemberOfPlurality y) means that x is a semiotic member of the plurality y, and that it participates in semiosis in the same way as its co-members x', x'', ... of the plurality y"^^xs:string.

pims-ii:isMemberOfStructure a owl:ObjectProperty;
   rdfs:label "isMemberOfStructure"@en;
   skos:altLabel "\\prec"@en;
   rdfs:domain [owl:complementOf pims-ii:Structure];
   rdfs:range pims-ii:Structure;
   rdfs:subPropertyOf pims-ii:isSemioticMemberOf;
   rdfs:comment "(x isMemberOfStructure y) means that x is a semiotic member of the structure y, and that it participates in semiosis differently from all of its co-members x', x'', ... of the structure y"^^xs:string.

pims-ii:isMereologicallyConstitutiveOf a owl:ObjectProperty;
   rdfs:label "isMereologicallyConstitutiveOf"@en;
   rdfs:subPropertyOf pims-ii:isConstitutiveOf, pims-ii:isProperPartOf;
   rdfs:comment "(x isMereologicallyConstitutiveOf y) means that x is constitutive of y by virtue of the way in which it is a proper part of y in 4D spacetime, e.g., as a necessary component of an item that was designed for a certain purpose"^^xs:string.

pims-ii:isNameFor a owl:ObjectProperty;
   rdfs:label "isNameFor"@en;
   rdfs:domain pims-ii:Name;
   rdfs:subPropertyOf pims-ii:isRepresentamenFor;
   rdfs:comment "(x isNameFor y), to be applied in the frequent special case where x is represented by a name for x, i.e., where social convention has established y as a rigid designator for x"^^xs:string.

pims-ii:isObjectWithinTriple a owl:ObjectProperty;
   rdfs:label "isObjectWithinTriple"@en;
   rdfs:domain [owl:unionOf (pims-ii:IndividualIRI pims-ii:ConceptualIRI)];
   rdfs:range pims-ii:Triple;
   rdfs:subPropertyOf pims-ii:isSemioticallyConstitutiveOf;
   rdfs:comment "(x isObjectWithinTriple y) means that y is a subject-predicate-object triple wherein x is the IRI of the object"^^xs:string.

pims-ii:isParticipantInCognition a owl:ObjectProperty;
   rdfs:label "isParticipantInCognition"@en;
   skos:altLabel "\\ddot{P}_\\kappa"@en;
   rdfs:range pims-ii:Cognition;
   rdfs:subPropertyOf pims-ii:isParticipantIn;
   rdfs:comment "(x isParticipantInCognition y) means that y is a cognition in which x is necessarily physically present and plays one of the roles characteristic for participation in a cognitive process as formalized by this ontology; this includes participation as a representamen, as a perceived object, as a step of a cognitive chain, or as an interpreter"^^xs:string.

pims-ii:isPredicateWithinTriple a owl:ObjectProperty;
   rdfs:label "isPredicateWithinTriple"@en;
   rdfs:domain pims-ii:RelationalIRI;
   rdfs:range pims-ii:Triple;
   rdfs:subPropertyOf pims-ii:isSemioticallyConstitutiveOf;
   rdfs:comment "(x isPredicateWithinTriple y) means that y is a subject-predicate-object triple wherein x is the IRI of the predicate"^^xs:string.

pims-ii:isReferenceFrameFor a owl:ObjectProperty;
   rdfs:label "isReferenceFrameFor"@en;
   skos:altLabel "\\dddot{R}"@en;
   rdfs:subPropertyOf pims-ii:sharesReferentWith;
   rdfs:comment "(s isReferenceFrameFor s') means that s is a representamen that provides relevant context, such as presuppositions or preconditions, to the representamen s'"@en.

pims-ii:isRepresentamenFor a owl:ObjectProperty;
   rdfs:label "isRepresentamenFor"@en;
   rdfs:subPropertyOf pims-ii:msIRHPIP, pims-ii:msHPIPIR, pims-ii:msIRHRIR;
   owl:inverseOf pims-ii:hasRepresentamen;
   owl:propertyChainAxiom (pims-ii:isRepresentamenIn [owl:inverseOf pims-ii:isReferentIn]);
   owl:propertyChainAxiom (pims-ii:isIncludedInAccumulation [owl:inverseOf pims-ii:isObjectInAccumulation]);
   owl:propertyChainAxiom (pims-ii:isGroundingPropositionIn [owl:inverseOf pims-ii:isGroundingStepIn]);
   owl:propertyChainAxiom (pims-ii:groundsNextStepIn [owl:inverseOf pims-ii:isPresentStepInGrounding]);
   rdfs:comment "Dyadic representation relation; (x isRepresentamenFor y) means that there is a cognitive step z such that (x isRepresentamenIn z) and (y isReferentIn z)"^^xs:string.

pims-ii:isRightHandSideIn a owl:ObjectProperty;
   rdfs:label "isRightHandSideIn"@en;
   skos:altLabel "\\ddot{E}_="@en;
   rdfs:domain pims-ii:Term;
   rdfs:range pims-ii:EqualityArticulation;
   rdfs:subPropertyOf pims-ii:isSecondInDyad;
   rdfs:comment "(y isRightHandSideIn a) mans that a: x = y is an equality articulation with the term y as its right-hand side"@en.

pims-ii:isSecondInDyad a owl:ObjectProperty;
   rdfs:label "isSecondInDyad"@en;
   skos:altLabel "\\ddot{E}_D"@en;
   rdfs:domain pims-ii:Conventional;
   rdfs:range pims-ii:Dyad;
   rdfs:subPropertyOf pims-ii:isSemioticallyConstitutiveOf;
   rdfs:comment "(y isSecondInDyad d) means that y is the second element of the dyad d"^^xs:string.

pims-ii:isSemioticMemberOf a owl:ObjectProperty;
   rdfs:label "isSemioticMemberOf"@en;
   skos:altLabel "\\ddot\\leq"@en;
   rdfs:domain [owl:complementOf pims-ii:Plurality];
   rdfs:range pims-ii:SemioticCollective;
   rdfs:subPropertyOf pims-ii:isMemberOf, pims-ii:isSemioticallyConstitutiveOf;
   rdfs:comment "(x isSemioticMemberOf y) means that x acts as a representamen or as a referent jointly with other co-members of the same semiotic collective y"^^xs:string.

pims-ii:isSemioticallyConstitutiveOf a owl:ObjectProperty;
   rdfs:label "isSemioticallyConstitutiveOf"@en;
   skos:altLabel "\\v{C}"@en;
   rdfs:range [
      a owl:Restriction;
      owl:onProperty pims-ii:isRepresentamenFor;
      owl:someValuesFrom pims-ii:Object
   ];
   rdfs:subPropertyOf pims-ii:isConstitutiveOf;
   rdfs:comment "(x isSemioticallyConstitutiveOf y) means that the evaluation or association with x plays a role in the way in which y functions as a representamen - n.b, this does not entail physical parthood; e.g., if 'q = 2f(p)' is given, the expression 'f(p) = ... (some term involving q)' may be seen as semiotically constituive of the first expression, precisely because it contains the right-hand side that was missing"^^xs:string.

pims-ii:isStepInCognitiveChain a owl:ObjectProperty;
   rdfs:label "isStepInCognitiveChain"@en;
   rdfs:domain pims-ii:CognitiveStep;
   rdfs:domain pims-ii:CognitiveChain;
   rdfs:subPropertyOf pims-ii:isStepIn, pims-ii:isParticipantInCognition;
   rdfs:comment "(x isStepInCognitiveChain y) means that y is a cognitive chain that consists of multiple logically connected cognitive steps (following Peirce, these are typically triads, i.e., semioses and semantic changes), and that x is one of these steps"^^xs:string.

pims-ii:isSubjectWithinTriple a owl:ObjectProperty;
   rdfs:label "isSubjectWithinTriple"@en;
   rdfs:domain pims-ii:IndividualIRI;
   rdfs:range pims-ii:Triple;
   rdfs:subPropertyOf pims-ii:isSemioticallyConstitutiveOf;
   rdfs:comment "(x isSubjectWithinTriple y) means that y is a subject-predicate-object triple wherein x is the IRI of the subject"^^xs:string.

pims-ii:isUnitOf a owl:ObjectProperty;
   rdfs:label "isUnitOf"@en;
   skos:altLabel "\\v{C}_u"@en;
   rdfs:domain pims-ii:MeasurementUnit;
   rdfs:range pims-ii:Value;
   rdfs:subPropertyOf pims-ii:isSemioticallyConstitutiveOf;
   rdfs:comment "(x isUnitOf y) means that x is the unit of y, e.g., in 200 kPa, x would be kPa"^^xs:string.

pims-ii:isValueInAssignment a owl:ObjectProperty;
   rdfs:label "isValueInAssignment"@en;
   skos:altLabel "\\ddot{D}"@en;
   rdfs:domain pims-ii:Value;
   rdfs:range pims-ii:Assignment;
   rdfs:subPropertyOf pims-ii:isRightHandSideIn;
   rdfs:comment "(y isValueInAssignment a) mans that a: x = y is an assignment where the value y is assigned to a variable x"^^xs:string.

pims-ii:isVariableInAssignment a owl:ObjectProperty;
   rdfs:label "isVariableInAssignment"@en;
   skos:altLabel "\\dot{D}"@en;
   rdfs:domain pims-ii:Variable;
   rdfs:range pims-ii:Assignment;
   rdfs:subPropertyOf pims-ii:isLeftHandSideIn;
   rdfs:comment "(x isVariableInAssignment a) mans that a: x = y is an assignment where a value y is assigned to the variable x"^^xs:string.

pims-ii:logicallyPrecedes a owl:ObjectProperty, owl:TransitiveProperty;
   rdfs:label "logicallyPrecedes"@en;
   skos:altLabel "\\hookrightarrow^+"@en;
   rdfs:domain pims-ii:Cognition;
   rdfs:range pims-ii:Cognition;
   rdfs:subPropertyOf pims-ii:precedesStep;
   rdfs:comment "(x logicallyPrecedes y) means that x and y are cognitive steps that are connected by a cognitive chain, leading from x and y, that does not contain a cognitive rupture"@en;
   skos:scopeNote "'logicallyPrecedes' is the transitive closure of 'directlyGrounds'"@en.

pims-ii:providesJustification a owl:ObjectProperty;
   rdfs:label "providesJustification"@en;
   rdfs:range pims-ii:GroundingChain;
   rdfs:subPropertyOf pims-ii:affirmsCognition;
   rdfs:comment "(x providesJustification y) means that x is about some cognition z, providing a justification of it by referring to y, i.e., a grounding chain that establishes the epistemic status of z; thereby, x does not only affirm z, but also its grounding chain y"^^xs:string.

pims-ii:realizes a owl:ObjectProperty;
   rdfs:label "realizes"@en;
   rdfs:domain [owl:complementOf pims-ii:SemioticCollective];
   rdfs:range pims-ii:Articulation;
   rdfs:subPropertyOf pims-ii:isSemioticMemberOf;
   rdfs:comment "(x realizes y) means that x, which is not a semiotic collective, is a literal or non-literal realization of the expression y"^^xs:string.

pims-ii:sharesReferentWith a owl:ObjectProperty, owl:SymmetricProperty;
   rdfs:label "sharesReferentWith"@en;
   rdfs:subPropertyOf pims-ii:msIRHRHPIP, pims-ii:msHPIPIRHR;
   rdfs:comment "(X sharesReferentWith Z) == there is a Y such that both X and Z isRepresentamenFor Y"^^xs:string.

pims-ii:sharesRepresentamenWith a owl:ObjectProperty, owl:SymmetricProperty;
   rdfs:label "sharesRepresentamenWith"@en;
   rdfs:subPropertyOf pims-ii:msHRIRHPIP, pims-ii:msHPIPHRIR;
   rdfs:comment "(X sharesRepresentamenWith Z) == there is a Y such that Y isRepresentamenFor both X and Z"^^xs:string.

pims-ii:underlies a owl:ObjectProperty, owl:TransitiveProperty;
   rdfs:label "underlies"@en;
   rdfs:subPropertyOf pims-ii:hasCausalConnectionWith;
   rdfs:comment "the relation 'underlies' is the transitive closure of the relation 'isConstitutiveOf'"^^xs:string.

#########################################
# MEREOSEMIOTIC CHAIN RELATIONS: BINARY #
#########################################

## P+P+ -> P+ -> isProperPartOf
#
## P+P- -> TQ -> isMereosemioticallyRelatedTo
#
## P-P+ -> overlapsWith
#
## P-P- -> P- -> hasProperPart
#
## P+R+
#
pims-ii:msIPIR a owl:ObjectProperty;
   rdfs:label "msIPIR"@en;
   rdfs:subPropertyOf pims-ii:msHPIPIR, pims-ii:msIPIRHPIP;
   owl:inverseOf pims-ii:msHRHP;
   owl:propertyChainAxiom (pims-ii:isProperPartOf pims-ii:isRepresentamenFor);
   rdfs:comment "(X msIP Z) == isProperPartOf o isRepresentamenFor == there is a Y such that (X isProperPartOf Y) and (Y isRepresentamenFor Z)"^^xs:string.
## P+R-
#
pims-ii:msIPHR a owl:ObjectProperty;
   rdfs:label "msIPHR"@en;
   rdfs:subPropertyOf pims-ii:msHPIPHR, pims-ii:msIPHRHPIP;
   owl:inverseOf pims-ii:msIRHP;
   owl:propertyChainAxiom (pims-ii:isProperPartOf pims-ii:hasRepresentamen);
   rdfs:comment "(X msIPHR Z) == isProperPartOf o hasRepresentamen == there is a Y such that (X isProperPartOf Y) and (Z isRepresentamenFor Y)"^^xs:string.
## P-R+
#
pims-ii:msHPIR a owl:ObjectProperty;
   rdfs:label "msHPIR"@en;
   rdfs:subPropertyOf pims-ii:msHPIPIR, pims-ii:msHPIRHPIP;
   owl:inverseOf pims-ii:msHRIP;
   owl:propertyChainAxiom (pims-ii:hasProperPart pims-ii:isRepresentamenFor);
   rdfs:comment "(X msHPIR Z) == hasProperPart o isRepresentamenFor == there is a Y such that (Y isProperPartOf X) and (Y is RepresentamenFor Z)"^^xs:string.
## P-R-
#
pims-ii:msHPHR a owl:ObjectProperty;
   rdfs:label "msHPHR"@en;
   rdfs:subPropertyOf pims-ii:msHPIPHR, pims-ii:msHPHRHPIP;
   owl:inverseOf pims-ii:msIRIP;
   owl:propertyChainAxiom (pims-ii:hasProperPart pims-ii:hasRepresentamen);
   rdfs:comment "(X msHPHR Z) == hasProperPart o hasRepresentamen == there is a Y such that (Y isProperPartOf X) and (Z isRepresentamenFor Y)"^^xs:string.
## R+P+
#
pims-ii:msIRIP a owl:ObjectProperty;
   rdfs:label "msIRIP"@en;
   rdfs:subPropertyOf pims-ii:msIRHPIP, pims-ii:msHPIPIRIP;
   owl:inverseOf pims-ii:msHPHR;
   owl:propertyChainAxiom (pims-ii:isRepresentamenFor pims-ii:isProperPartOf);
   rdfs:comment "(X msIRIP Z) == isRepresentamenFor o isProperPartOf == there is a Y such that (X isRepresentamenFor Y) and (Y isProperPartOf Z)"^^xs:string.
## R+P-
#
pims-ii:msIRHP a owl:ObjectProperty;
   rdfs:label "msIRHP"@en;
   rdfs:subPropertyOf pims-ii:msIRHPIP, pims-ii:msHPIPIRHP;
   owl:inverseOf pims-ii:msIPHR;
   owl:propertyChainAxiom (pims-ii:isRepresentamenFor pims-ii:hasProperPart);
   rdfs:comment "(X msIRHP Z) == isRepresentamenFor o hasProperPart == there is a Y such that (X isRepresentamenFor Y) and (Z isProperPartOf Y)"^^xs:string.
## R-P+
#
pims-ii:msHRIP a owl:ObjectProperty;
   rdfs:label "msHRIP"@en;
   rdfs:subPropertyOf pims-ii:msHRHPIP, pims-ii:msHPIPHRIP;
   owl:inverseOf pims-ii:msHPIR;
   owl:propertyChainAxiom (pims-ii:hasRepresentamen pims-ii:isProperPartOf);
   rdfs:comment "(X msHRIP Z) == hasRepresentamen o isProperPartOf == there is a Y such that (Y isRepresentamenFor X) and (Y isProperPartOf Z)"^^xs:string.
## R-P-
#
pims-ii:msHRHP a owl:ObjectProperty;
   rdfs:label "msHRHP"@en;
   rdfs:subPropertyOf pims-ii:msHRHPIP, pims-ii:msHPIPHRHP;
   owl:inverseOf pims-ii:msIPIR;
   owl:propertyChainAxiom (pims-ii:hasRepresentamen pims-ii:hasProperPart);
   rdfs:comment "(X msHRHP Z) == hasRepresentamen o hasProperPart == there is a Y such that (Y isRepresentamenFor X) and (Z isProperPartOf Y)"^^xs:string.
## R+R+
#
pims-ii:msIRIR a owl:ObjectProperty;
   rdfs:label "msIRIR"@en;
   rdfs:subPropertyOf pims-ii:msHPIPIRIR, pims-ii:msIRIRHPIP;
   owl:inverseOf pims-ii:msHRHR;
   owl:propertyChainAxiom (pims-ii:isRepresentamenFor pims-ii:isRepresentamenFor);
   rdfs:comment "(X msIRIR Z) == (isRepresentamenFor)^2 == there is a Y such that (X isRepresentamenFor Y) and (Y isRepresentamenFor Z)"^^xs:string.
## R+R- -> sharesReferentWith
#
## R-R+ -> sharesRepresentamenWith
#
## R-R-
#
pims-ii:msHRHR a owl:ObjectProperty;
   rdfs:label "msHRHR"@en;
   rdfs:subPropertyOf pims-ii:msHPIPHRHR, pims-ii:msHRHRHPIP;
   owl:inverseOf pims-ii:msIRIR;
   owl:propertyChainAxiom (pims-ii:hasRepresentamen pims-ii:hasRepresentamen);
   rdfs:comment "(X msHRHR Z) == (hasRepresentamen)^2 == there is a Y such that (Y isRepresentamenFor X) and (Z isRepresentamenFor Y)"^^xs:string.

##########################################
# MEREOSEMIOTIC CHAIN RELATIONS: TERNARY #
##########################################

## P-P+R+
#
pims-ii:msHPIPIR a owl:ObjectProperty;
   rdfs:label "msHPIPIR"@en;
   rdfs:subPropertyOf pims-ii:isMereosemioticallyRelatedTo;
   owl:inverseOf pims-ii:msHRHPIP;
   owl:propertyChainAxiom (pims-ii:overlapsWith pims-ii:isRepresentamenFor);
   rdfs:comment "(X msHPIPIR Z) == hasProperPart o isProperPartOf o isRepresentamenFor == there is a Y such that (X overlapsWith Y) and (Y isRepresentamenFor Z)"^^xs:string.
## P-P+R-
#
pims-ii:msHPIPHR a owl:ObjectProperty;
   rdfs:label "msHPIPHR"@en;
   rdfs:subPropertyOf pims-ii:isMereosemioticallyRelatedTo;
   owl:inverseOf pims-ii:msIRHPIP;
   owl:propertyChainAxiom (pims-ii:overlapsWith pims-ii:hasRepresentamen);
   rdfs:comment "(X msHPIPHR Z) == hasProperPart o isProperPartOf o hasRepresentamen == there is a Y such that (X overlapsWith Y) and (Z isRepresentamenFor Y)"^^xs:string.
## P+R+P+
#
pims-ii:msIPIRIP a owl:ObjectProperty;
   rdfs:label "msIPIRIP"@en;
   rdfs:subPropertyOf pims-ii:msHPIPIRIP, pims-ii:msIPIRHPIP;
   owl:inverseOf pims-ii:msHPHRHP;
   owl:propertyChainAxiom (pims-ii:msIPIR pims-ii:isProperPartOf);
   rdfs:comment "chain relation msIPIR o isProperPartOf".
## P+R+P-
#
pims-ii:msIPIRHP a owl:ObjectProperty;
   rdfs:label "msIPIRHP"@en;
   rdfs:subPropertyOf pims-ii:msHPIPIRHP, pims-ii:msIPIRHPIP;
   owl:inverseOf pims-ii:msIPHRHP;
   owl:propertyChainAxiom (pims-ii:msIPIR pims-ii:hasProperPart);
   rdfs:comment "chain relation msIPIR o hasProperPart".
## P+R-P+
#
pims-ii:msIPHRIP a owl:ObjectProperty;
   rdfs:label "msIPHRIP"@en;
   rdfs:subPropertyOf pims-ii:msHPIPHRIP, pims-ii:msIPHRHPIP;
   owl:inverseOf pims-ii:msHPIRHP;
   owl:propertyChainAxiom (pims-ii:msIPHR pims-ii:isProperPartOf);
   rdfs:comment "chain relation msIPHR o isProperPartOf".
## P+R-P-
#
pims-ii:msIPHRHP a owl:ObjectProperty;
   rdfs:label "msIPHRHP"@en;
   rdfs:subPropertyOf pims-ii:msHPIPHRHP, pims-ii:msIPHRHPIP;
   owl:inverseOf pims-ii:msIPIRHP;
   owl:propertyChainAxiom (pims-ii:msIPHR pims-ii:hasProperPart);
   rdfs:comment "chain relation msIPHR o hasProperPart".
## P-R+P+
#
pims-ii:msHPIRIP a owl:ObjectProperty;
   rdfs:label "msHPIRIP"@en;
   rdfs:subPropertyOf pims-ii:msHPIPIRIP, pims-ii:msHPIRHPIP;
   owl:inverseOf pims-ii:msHPHRIP;
   owl:propertyChainAxiom (pims-ii:msHPIR pims-ii:isProperPartOf);
   rdfs:comment "chain relation msHPIR o isProperPartOf".
## P-R+P-
#
pims-ii:msHPIRHP a owl:ObjectProperty;
   rdfs:label "msIPIRHP"@en;
   rdfs:subPropertyOf pims-ii:msHPIPIRHP, pims-ii:msHPIRHPIP;
   owl:inverseOf pims-ii:msIPHRIP;
   owl:propertyChainAxiom (pims-ii:msHPIR pims-ii:hasProperPart);
   rdfs:comment "chain relation msHPIR o hasProperPart".
## P-R-P+
#
pims-ii:msHPHRIP a owl:ObjectProperty;
   rdfs:label "msHPHRIP"@en;
   rdfs:subPropertyOf pims-ii:msHPIPHRIP, pims-ii:msHPHRHPIP;
   owl:inverseOf pims-ii:msHPIRIP;
   owl:propertyChainAxiom (pims-ii:msHPHR pims-ii:isProperPartOf);
   rdfs:comment "chain relation msHPHR o hasProperPart".
## P-R-P-
#
pims-ii:msHPHRHP a owl:ObjectProperty;
   rdfs:label "msHPHRHP"@en;
   rdfs:subPropertyOf pims-ii:msHPIPHRHP, pims-ii:msHPHRHPIP;
   owl:inverseOf pims-ii:msIPIRIP;
   owl:propertyChainAxiom (pims-ii:msHPHR pims-ii:hasProperPart);
   rdfs:comment "chain relation msHPHR o hasProperPart".
## P+R+R+
#
pims-ii:msIPIRIR a owl:ObjectProperty;
   rdfs:label "msIPIRIR"@en;
   rdfs:subPropertyOf pims-ii:msHPIPIRIR;
   owl:inverseOf pims-ii:msHRHRHP;
   owl:propertyChainAxiom (pims-ii:msIPIR pims-ii:isRepresentamenFor);
   rdfs:comment "chain relation msIPIR o isRepresentamenFor".
## P+R+R-
#
pims-ii:msIPIRHR a owl:ObjectProperty;
   rdfs:label "msIPIRHR"@en;
   rdfs:subPropertyOf pims-ii:msHPIPIRHR;
   owl:inverseOf pims-ii:msIRHRHP;
   owl:propertyChainAxiom (pims-ii:msIPIR pims-ii:hasRepresentamen);
   owl:propertyChainAxiom (pims-ii:isProperPartOf pims-ii:sharesReferentWith);
   rdfs:comment "chain relation isProperPartOf o sharesReferentWith".
## P+R-R+
#
pims-ii:msIPHRIR a owl:ObjectProperty;
   rdfs:label "msIPHRIR"@en;
   rdfs:subPropertyOf pims-ii:msHPIPHRIR;
   owl:inverseOf pims-ii:msHRIRHP;
   owl:propertyChainAxiom (pims-ii:msIPHR pims-ii:isRepresentamenFor);
   owl:propertyChainAxiom (pims-ii:isProperPartOf pims-ii:sharesRepresentamenWith);
   rdfs:comment "chain relation isProperPartOf o sharesRepresentamenWith".
## P+R-R-
#
pims-ii:msIPHRHR a owl:ObjectProperty;
   rdfs:label "msIPHRHR"@en;
   rdfs:subPropertyOf pims-ii:msHPIPHRHR;
   owl:inverseOf pims-ii:msIRIRHP;
   owl:propertyChainAxiom (pims-ii:msIPHR pims-ii:hasRepresentamen);
   rdfs:comment "chain relation msIPHR o hasRepresentamen".
## P-R+R+
#
pims-ii:msHPIRIR a owl:ObjectProperty;
   rdfs:label "msHPIRIR"@en;
   rdfs:subPropertyOf pims-ii:msHPIPIRIR;
   owl:inverseOf pims-ii:msHRHRIP;
   owl:propertyChainAxiom (pims-ii:msHPIR pims-ii:isRepresentamenFor);
   rdfs:comment "chain relation msHPIR o isRepresentamenFor".
## P-R+R-
#
pims-ii:msHPIRHR a owl:ObjectProperty;
   rdfs:label "msHPIRHR"@en;
   rdfs:subPropertyOf pims-ii:msHPIPIRHR;
   owl:inverseOf pims-ii:msIRHRIP;
   owl:propertyChainAxiom (pims-ii:msHPIR pims-ii:hasRepresentamen);
   owl:propertyChainAxiom (pims-ii:hasProperPart pims-ii:sharesReferentWith);
   rdfs:comment "chain relation hasProperPart o sharesReferentWith".
## P-R-R+
#
pims-ii:msHPHRIR a owl:ObjectProperty;
   rdfs:label "msHPHRIR"@en;
   rdfs:subPropertyOf pims-ii:msHPIPHRIR;
   owl:inverseOf pims-ii:msHRIRIP;
   owl:propertyChainAxiom (pims-ii:msHPHR pims-ii:isRepresentamenFor);
   owl:propertyChainAxiom (pims-ii:hasProperPart pims-ii:sharesRepresentamenWith);
   rdfs:comment "chain relation hasProperPart o sharesRepresentamenWith".
## P-R-R-
#
pims-ii:msHPHRHR a owl:ObjectProperty;
   rdfs:label "msHPHRHR"@en;
   rdfs:subPropertyOf pims-ii:msHPIPHRHR;
   owl:inverseOf pims-ii:msIRIRIP;
   owl:propertyChainAxiom (pims-ii:msHPHR pims-ii:hasRepresentamen);
   rdfs:comment "chain relation msHPHR o hasRepresentamen".
## R+P-P+
#
pims-ii:msIRHPIP a owl:ObjectProperty;
   rdfs:label "msIRHPIP"@en;
   rdfs:subPropertyOf pims-ii:isMereosemioticallyRelatedTo;
   owl:inverseOf pims-ii:msHPIPHR;
   owl:propertyChainAxiom (pims-ii:msIRHP pims-ii:isProperPartOf);
   owl:propertyChainAxiom (pims-ii:isRepresentamenFor pims-ii:overlapsWith);
   rdfs:comment "(X msIRHPIP Z) == isRepresentamenFor o hasProperPart o isProperPartOf == there is a Y such that (X isRepresentamenFor Y) and (Y overlapsWith Z)"^^xs:string.
## R-P-P+
#
pims-ii:msHRHPIP a owl:ObjectProperty;
   rdfs:label "msHRHPIP"@en;
   rdfs:subPropertyOf pims-ii:isMereosemioticallyRelatedTo;
   owl:inverseOf pims-ii:msHPIPIR;
   owl:propertyChainAxiom (pims-ii:msHRHP pims-ii:isProperPartOf);
   owl:propertyChainAxiom (pims-ii:hasRepresentamen pims-ii:overlapsWith);
   rdfs:comment "(X msHRHPIP Z) == hasRepresentamen o hasProperPart o isProperPartOf == there is a Y such that (Y isRepresentamenFor X) and (Y overlapsWith Z)"^^xs:string.
## R+P+R+
#
pims-ii:msIRIPIR a owl:ObjectProperty;
   rdfs:label "msIRIPIR"@en;
   rdfs:subPropertyOf pims-ii:msIRHPIPIR;
   owl:inverseOf pims-ii:msHRHPHR;
   owl:propertyChainAxiom (pims-ii:msIRIP pims-ii:isRepresentamenFor);
   rdfs:comment "chain relation msIRIP o isRepresentamenFor".
## R+P+R-
#
pims-ii:msIRIPHR a owl:ObjectProperty;
   rdfs:label "msIRIPHR"@en;
   rdfs:subPropertyOf pims-ii:msIRHPIPHR;
   owl:inverseOf pims-ii:msIRHPHR;
   owl:propertyChainAxiom (pims-ii:msIRIP pims-ii:hasRepresentamen);
   rdfs:comment "chain relation msIRIP o hasRepresentamen".
## R+P-R+
#
pims-ii:msIRHPIR a owl:ObjectProperty;
   rdfs:label "msIRHPIR"@en;
   rdfs:subPropertyOf pims-ii:msIRHPIPIR;
   owl:inverseOf pims-ii:msHRIPHR;
   owl:propertyChainAxiom (pims-ii:msIRHP pims-ii:isRepresentamenFor);
   rdfs:comment "chain relation msIRHP o isRepresentamenFor".
## R+P-R-
#
pims-ii:msIRHPHR a owl:ObjectProperty;
   rdfs:label "msIRHPHR"@en;
   rdfs:subPropertyOf pims-ii:msIRHPIPHR;
   owl:inverseOf pims-ii:msIRIPHR;
   owl:propertyChainAxiom (pims-ii:msIRHP pims-ii:hasRepresentamen);
   rdfs:comment "chain relation msIRHP o hasRepresentamen".
## R-P+R+
#
pims-ii:msHRIPIR a owl:ObjectProperty;
   rdfs:label "msHRIPIR"@en;
   rdfs:subPropertyOf pims-ii:msHRHPIPIR;
   owl:inverseOf pims-ii:msHRHPIR;
   owl:propertyChainAxiom (pims-ii:msHRIP pims-ii:isRepresentamenFor);
   rdfs:comment "chain relation msHRIP o isRepresentamenFor".
## R-P+R-
#
pims-ii:msHRIPHR a owl:ObjectProperty;
   rdfs:label "msHRIPHR"@en;
   rdfs:subPropertyOf pims-ii:msHRHPIPHR;
   owl:inverseOf pims-ii:msIRHPIR;
   owl:propertyChainAxiom (pims-ii:msHRIP pims-ii:hasRepresentamen);
   rdfs:comment "chain relation msHRIP o hasRepresentamen".
## R-P-R+
#
pims-ii:msHRHPIR a owl:ObjectProperty;
   rdfs:label "msHRHPIR"@en;
   rdfs:subPropertyOf pims-ii:msHRHPIPIR;
   owl:inverseOf pims-ii:msHRIPIR;
   owl:propertyChainAxiom (pims-ii:msHRHP pims-ii:isRepresentamenFor);
   rdfs:comment "chain relation msHRHP o isRepresentamenFor".
## R-P-R-
#
pims-ii:msHRHPHR a owl:ObjectProperty;
   rdfs:label "msHRHPHR"@en;
   rdfs:subPropertyOf pims-ii:msHRHPIPHR;
   owl:inverseOf pims-ii:msIRIPIR;
   owl:propertyChainAxiom (pims-ii:msHRHP pims-ii:hasRepresentamen);
   rdfs:comment "chain relation msHRHP o hasRepresentamen".
## R+R+P+
#
pims-ii:msIRIRIP a owl:ObjectProperty;
   rdfs:label "msIRIRIP"@en;
   rdfs:subPropertyOf pims-ii:msIRIRHPIP;
   owl:inverseOf pims-ii:msHPHRHR;
   owl:propertyChainAxiom (pims-ii:msIRIR pims-ii:isProperPartOf);
   rdfs:comment "chain relation msIRIR o isProperPartOf".
## R+R+P-
#
pims-ii:msIRIRHP a owl:ObjectProperty;
   rdfs:label "msIRIRHP"@en;
   rdfs:subPropertyOf pims-ii:msIRIRHPIP;
   owl:inverseOf pims-ii:msIPHRHR;
   owl:propertyChainAxiom (pims-ii:msIRIR pims-ii:hasProperPart);
   rdfs:comment "chain relation msIRIR o hasProperPart".
## R+R-P+
#
pims-ii:msIRHRIP a owl:ObjectProperty;
   rdfs:label "msIRHRIP"@en;
   rdfs:subPropertyOf pims-ii:msIRHRHPIP;
   owl:inverseOf pims-ii:msHPIRHR;
   owl:propertyChainAxiom (pims-ii:sharesReferentWith pims-ii:isProperPartOf);
   rdfs:comment "chain relation sharesReferentWith o isProperPartOf".
## R+R-P-
#
pims-ii:msIRHRHP a owl:ObjectProperty;
   rdfs:label "msIRHRHP"@en;
   rdfs:subPropertyOf pims-ii:msIRHRHPIP;
   owl:inverseOf pims-ii:msIPIRHR;
   owl:propertyChainAxiom (pims-ii:sharesReferentWith pims-ii:hasProperPart);
   rdfs:comment "chain relation sharesReferentWith o hasProperPart".
## R-R+P+
#
pims-ii:msHRIRIP a owl:ObjectProperty;
   rdfs:label "msHRIRIP"@en;
   rdfs:subPropertyOf pims-ii:msHRIRHPIP;
   owl:inverseOf pims-ii:msHPHRIR;
   owl:propertyChainAxiom (pims-ii:sharesRepresentamenWith pims-ii:isProperPartOf);
   rdfs:comment "chain relation sharesRepresentamenWith o isProperPartOf".
## R-R+P-
#
pims-ii:msHRIRHP a owl:ObjectProperty;
   rdfs:label "msHRIRHP"@en;
   rdfs:subPropertyOf pims-ii:msHRIRHPIP;
   owl:inverseOf pims-ii:msIPHRIR;
   owl:propertyChainAxiom (pims-ii:sharesRepresentamenWith pims-ii:hasProperPart);
   rdfs:comment "chain relation sharesRepresentamenWith o hasProperPart".
## R-R-P+
#
pims-ii:msHRHRIP a owl:ObjectProperty;
   rdfs:label "msHRHRIP"@en;
   rdfs:subPropertyOf pims-ii:msHRHRHPIP;
   owl:inverseOf pims-ii:msHPIRIR;
   owl:propertyChainAxiom (pims-ii:msHRHR pims-ii:isProperPartOf);
   rdfs:comment "chain relation msHRHR o isProperPartOf".
## R-R-P-
#
pims-ii:msHRHRHP a owl:ObjectProperty;
   rdfs:label "msHRHRHP"@en;
   rdfs:subPropertyOf pims-ii:msHRHRHPIP;
   owl:inverseOf pims-ii:msIPIRIR;
   owl:propertyChainAxiom (pims-ii:msHRHR pims-ii:hasProperPart);
   rdfs:comment "chain relation msHRHR o hasProperPart".
## R+R+R+
#
pims-ii:msIRIRIR a owl:ObjectProperty;
   rdfs:label "msIRIRIR"@en;
   rdfs:subPropertyOf pims-ii:isMereosemioticallyRelatedTo;
   owl:inverseOf pims-ii:msHRHRHR;
   owl:propertyChainAxiom (pims-ii:msIRIR pims-ii:isRepresentamenFor);
   rdfs:comment "chain relation msIRIR o isRepresentamenFor".
## R+R+R-
#
pims-ii:msIRIRHR a owl:ObjectProperty;
   rdfs:label "msIRIRHR"@en;
   rdfs:subPropertyOf pims-ii:isMereosemioticallyRelatedTo;
   owl:inverseOf pims-ii:msIRHRHR;
   owl:propertyChainAxiom (pims-ii:msIRIR pims-ii:hasRepresentamen);
   owl:propertyChainAxiom (pims-ii:isRepresentamenFor pims-ii:sharesReferentWith);
   rdfs:comment "chain relation isRepresentamenFor o sharesReferentWith".
## R+R-R+
#
pims-ii:msIRHRIR a owl:ObjectProperty;
   rdfs:label "msHRIRHR"@en;
   rdfs:subPropertyOf pims-ii:isMereosemioticallyRelatedTo;
   owl:inverseOf pims-ii:msHRIRHR;
   owl:propertyChainAxiom (pims-ii:sharesReferentWith pims-ii:isRepresentamenFor);
   owl:propertyChainAxiom (pims-ii:isRepresentamenFor pims-ii:sharesRepresentamenWith);
   rdfs:comment "chain relation sharesReferentWith o isRepresentamenFor".
## R+R-R-
#
pims-ii:msIRHRHR a owl:ObjectProperty;
   rdfs:label "msIRHRHR"@en;
   rdfs:subPropertyOf pims-ii:isMereosemioticallyRelatedTo;
   owl:inverseOf pims-ii:msIRIRHR;
   owl:propertyChainAxiom (pims-ii:sharesReferentWith pims-ii:hasRepresentamen);
   rdfs:comment "chain relation sharesReferentWith o hasRepresentamen".
## R-R+R+
#
pims-ii:msHRIRIR a owl:ObjectProperty;
   rdfs:label "msHRIRIR"@en;
   rdfs:subPropertyOf pims-ii:isMereosemioticallyRelatedTo;
   owl:inverseOf pims-ii:msHRHRIR;
   owl:propertyChainAxiom (pims-ii:sharesRepresentamenWith pims-ii:isRepresentamenFor);
   rdfs:comment "chain relation sharesRepresentamenWith o isRepresentamenFor".
## R-R+R-
#
pims-ii:msHRIRHR a owl:ObjectProperty;
   rdfs:label "msHRIRHR"@en;
   rdfs:subPropertyOf pims-ii:isMereosemioticallyRelatedTo;
   owl:inverseOf pims-ii:msIRHRIR;
   owl:propertyChainAxiom (pims-ii:sharesRepresentamenWith pims-ii:hasRepresentamen);
   owl:propertyChainAxiom (pims-ii:hasRepresentamen pims-ii:sharesReferentWith);
   rdfs:comment "chain relation hasRepresentamen o sharesReferentWith".
## R-R-R+
#
pims-ii:msHRHRIR a owl:ObjectProperty;
   rdfs:label "msHRHRIR"@en;
   rdfs:subPropertyOf pims-ii:isMereosemioticallyRelatedTo;
   owl:inverseOf pims-ii:msHRIRIR;
   owl:propertyChainAxiom (pims-ii:msHRHR pims-ii:isRepresentamenFor);
   owl:propertyChainAxiom (pims-ii:hasRepresentamen pims-ii:sharesRepresentamenWith);
   rdfs:comment "chain relation hasRepresentamen o sharesRepresentamenWith".
## R-R-R-
#
pims-ii:msHRHRHR a owl:ObjectProperty;
   rdfs:label "msHRHRHR"@en;
   rdfs:subPropertyOf pims-ii:isMereosemioticallyRelatedTo;
   owl:inverseOf pims-ii:msIRIRIR;
   owl:propertyChainAxiom (pims-ii:msHRHR pims-ii:hasRepresentamen);
   rdfs:comment "chain relation msHRHR o hasRepresentamen".

###########################################################
#        MEREOSEMIOTIC CHAIN RELATIONS: QUATERNARY        #
# only where overlapsWith (i.e., P-P+) occurs as a factor #
###########################################################

## P-P+R+P+
#
pims-ii:msHPIPIRIP a owl:ObjectProperty;
   rdfs:label "msHPIPIRIP"@en;
   rdfs:subPropertyOf pims-ii:isMereosemioticallyRelatedTo;
   owl:inverseOf pims-ii:msHPHRHPIP;
   owl:propertyChainAxiom (pims-ii:overlapsWith pims-ii:msIRIP);
   rdfs:comment "chain relation overlapsWith o msIRIP".
## P-P+R+P-
#
pims-ii:msHPIPIRHP a owl:ObjectProperty;
   rdfs:label "msHPIPIRHP"@en;
   rdfs:subPropertyOf pims-ii:isMereosemioticallyRelatedTo;
   owl:inverseOf pims-ii:msIPHRHPIP;
   owl:propertyChainAxiom (pims-ii:overlapsWith pims-ii:msIRHP);
   rdfs:comment "chain relation overlapsWith o msIRHP".
## P-P+R+R+
#
pims-ii:msHPIPIRIR a owl:ObjectProperty;
   rdfs:label "msHPIPIRIR"@en;
   rdfs:subPropertyOf pims-ii:isMereosemioticallyRelatedTo;
   owl:inverseOf pims-ii:msHRHRHPIP;
   owl:propertyChainAxiom (pims-ii:overlapsWith pims-ii:msIRIR);
   rdfs:comment "chain relation overlapsWith o msIRIR".
## P-P+R+R-
#
pims-ii:msHPIPIRHR a owl:ObjectProperty;
   rdfs:label "msHPIPIRHR"@en;
   rdfs:subPropertyOf pims-ii:isMereosemioticallyRelatedTo;
   owl:inverseOf pims-ii:msIRHRHPIP;
   owl:propertyChainAxiom (pims-ii:overlapsWith pims-ii:sharesReferentWith);
   rdfs:comment "chain relation overlapsWith o sharesReferentWith".
## P-P+R-P+
#
pims-ii:msHPIPHRIP a owl:ObjectProperty;
   rdfs:label "msHPIPHRIP"@en;
   rdfs:subPropertyOf pims-ii:isMereosemioticallyRelatedTo;
   owl:inverseOf pims-ii:msHPIRHPIP;
   owl:propertyChainAxiom (pims-ii:overlapsWith pims-ii:msHRIP);
   rdfs:comment "chain relation overlapsWith o msHRIP".
## P-P+R-P-
#
pims-ii:msHPIPHRHP a owl:ObjectProperty;
   rdfs:label "msHPIPHRHP"@en;
   rdfs:subPropertyOf pims-ii:isMereosemioticallyRelatedTo;
   owl:inverseOf pims-ii:msIPIRHPIP;
   owl:propertyChainAxiom (pims-ii:overlapsWith pims-ii:msHRHP);
   rdfs:comment "chain relation overlapsWith o msHRHP".
## P-P+R-R+
#
pims-ii:msHPIPHRIR a owl:ObjectProperty;
   rdfs:label "msHPIPHRIR"@en;
   rdfs:subPropertyOf pims-ii:isMereosemioticallyRelatedTo;
   owl:inverseOf pims-ii:msHRIRHPIP;
   owl:propertyChainAxiom (pims-ii:overlapsWith pims-ii:sharesRepresentamenWith);
   rdfs:comment "chain relation overlapsWith o sharesRepresentamenWith".
## P-P+R-R-
#
pims-ii:msHPIPHRHR a owl:ObjectProperty;
   rdfs:label "msHPIPHRHR"@en;
   rdfs:subPropertyOf pims-ii:isMereosemioticallyRelatedTo;
   owl:inverseOf pims-ii:msIRIRHPIP;
   owl:propertyChainAxiom (pims-ii:overlapsWith pims-ii:msHRHR);
   rdfs:comment "chain relation overlapsWith o msHRHR".
## P+R+P-P+
#
pims-ii:msIPIRHPIP a owl:ObjectProperty;
   rdfs:label "msIPIRHPIP"@en;
   rdfs:subPropertyOf pims-ii:isMereosemioticallyRelatedTo;
   owl:inverseOf pims-ii:msHPIPHRHP;
   owl:propertyChainAxiom (pims-ii:msIPIR pims-ii:overlapsWith);
   rdfs:comment "chain relation msIPIR o overlapsWith".
## P+R-P-P+
#
pims-ii:msIPHRHPIP a owl:ObjectProperty;
   rdfs:label "msIPHRHPIP"@en;
   rdfs:subPropertyOf pims-ii:isMereosemioticallyRelatedTo;
   owl:inverseOf pims-ii:msHPIPIRHP;
   owl:propertyChainAxiom (pims-ii:msIPHR pims-ii:overlapsWith);
   rdfs:comment "chain relation msIPHR o overlapsWith".
## P-R+P-P+
#
pims-ii:msHPIRHPIP a owl:ObjectProperty;
   rdfs:label "msHPIRHPIP"@en;
   rdfs:subPropertyOf pims-ii:isMereosemioticallyRelatedTo;
   owl:inverseOf pims-ii:msHPIPHRIP;
   owl:propertyChainAxiom (pims-ii:msHPIR pims-ii:overlapsWith);
   rdfs:comment "chain relation msHPIR o overlapsWith".
## P-R-P-P+
#
pims-ii:msHPHRHPIP a owl:ObjectProperty;
   rdfs:label "msHPHRHPIP"@en;
   rdfs:subPropertyOf pims-ii:isMereosemioticallyRelatedTo;
   owl:inverseOf pims-ii:msHPIPIRIP;
   owl:propertyChainAxiom (pims-ii:msHPHR pims-ii:overlapsWith);
   rdfs:comment "chain relation msHPHR o overlapsWith".
## R+P-P+R+
#
pims-ii:msIRHPIPIR a owl:ObjectProperty;
   rdfs:label "msIRHPIPIR"@en;
   rdfs:subPropertyOf pims-ii:isMereosemioticallyRelatedTo;
   owl:inverseOf pims-ii:msHRHPIPHR;
   owl:propertyChainAxiom (pims-ii:msIRHP pims-ii:msIPIR);
   owl:propertyChainAxiom (pims-ii:isRepresentamenFor pims-ii:overlapsWith pims-ii:isRepresentamenFor);
   rdfs:comment "chain relation msIRHP o msIPIR".
## R+P-P+R-
#
pims-ii:msIRHPIPHR a owl:ObjectProperty, owl:SymmetricProperty;
   rdfs:label "msIRHPIPHR"@en;
   rdfs:subPropertyOf pims-ii:isMereosemioticallyRelatedTo;
   owl:propertyChainAxiom (pims-ii:msIRHP pims-ii:msIPHR);
   owl:propertyChainAxiom (pims-ii:isRepresentamenFor pims-ii:overlapsWith pims-ii:hasRepresentamen);
   rdfs:comment "chain relation msIRHP o msIPHR".
## R-P-P+R+
#
pims-ii:msHRHPIPIR a owl:ObjectProperty, owl:SymmetricProperty;
   rdfs:label "msHRHPIPIR"@en;
   rdfs:subPropertyOf pims-ii:isMereosemioticallyRelatedTo;
   owl:propertyChainAxiom (pims-ii:msHRHP pims-ii:msIPIR);
   owl:propertyChainAxiom (pims-ii:hasRepresentamen pims-ii:overlapsWith pims-ii:isRepresentamenFor);
   rdfs:comment "chain relation msHRHP o msIPIR".
## R-P-P+R-
#
pims-ii:msHRHPIPHR a owl:ObjectProperty;
   rdfs:label "msHRHPIPHR"@en;
   rdfs:subPropertyOf pims-ii:isMereosemioticallyRelatedTo;
   owl:inverseOf pims-ii:msIRHPIPIR;
   owl:propertyChainAxiom (pims-ii:msHRHP pims-ii:msIPHR);
   owl:propertyChainAxiom (pims-ii:hasRepresentamen pims-ii:overlapsWith pims-ii:hasRepresentamen);
   rdfs:comment "chain relation msHRHP o msIPHR".
## R+R+P-P+
#
pims-ii:msIRIRHPIP a owl:ObjectProperty;
   rdfs:label "msIRIRHPIP"@en;
   rdfs:subPropertyOf pims-ii:isMereosemioticallyRelatedTo;
   owl:inverseOf pims-ii:msHPIPHRHR;
   owl:propertyChainAxiom (pims-ii:msIRIR pims-ii:overlapsWith);
   rdfs:comment "chain relation msIRIR o overlapsWith".
## R+R-P-P+
#
pims-ii:msIRHRHPIP a owl:ObjectProperty;
   rdfs:label "msIRHRHPIP"@en;
   rdfs:subPropertyOf pims-ii:isMereosemioticallyRelatedTo;
   owl:inverseOf pims-ii:msHPIPIRHR;
   owl:propertyChainAxiom (pims-ii:sharesReferentWith pims-ii:overlapsWith);
   rdfs:comment "chain relation sharesReferentWith o overlapsWith".
## R-R+P-P+
#
pims-ii:msHRIRHPIP a owl:ObjectProperty;
   rdfs:label "msHRIRHPIP"@en;
   rdfs:subPropertyOf pims-ii:isMereosemioticallyRelatedTo;
   owl:inverseOf pims-ii:msHPIPHRIR;
   owl:propertyChainAxiom (pims-ii:sharesRepresentamenWith pims-ii:overlapsWith);
   rdfs:comment "chain relation sharesRepresentamenWith o overlapsWith".
## R-R-P-P+
#
pims-ii:msHRHRHPIP a owl:ObjectProperty;
   rdfs:label "msHRHRHPIP"@en;
   rdfs:subPropertyOf pims-ii:isMereosemioticallyRelatedTo;
   owl:inverseOf pims-ii:msHPIPIRIR;
   owl:propertyChainAxiom (pims-ii:msHRHR pims-ii:overlapsWith);
   rdfs:comment "chain relation msHRHR o overlapsWith".

##################################
# AGENCY AND TELEOLOGY: CONCEPTS #
##################################

pims-ii:Action a owl:Class;
   rdfs:label "Action"@en;
   rdfs:subClassOf pims-ii:Process, [
      a owl:Restriction;
      owl:onProperty [owl:inverseOf pims-ii:isAgentIn];
      owl:someValuesFrom pims-ii:Agent
   ];
   rdfs:comment "Action, i.e., a process that is conducted/undertaken by an agent - the action has exactly one agent"^^xs:string.

pims-ii:Agent a owl:Class;
   rdfs:label "Agent"@en;
   rdfs:subClassOf pims-ii:Object;
   rdfs:comment "Agent, i.e., an object that interacts with its surroundings by a) perceiving and b) doing, i.e., an object that carries out actions, including perceptive actions"@en.

pims-ii:CognitiveAction a owl:Class;
   rdfs:label "CognitiveAction"@en;
   rdfs:subClassOf pims-ii:Cognition, pims-ii:Action, [
      a owl:Restriction;
      owl:onProperty [owl:inverseOf pims-ii:isInterpreterIn];
      owl:someValuesFrom pims-ii:Agent
   ];
   owl:intersectionOf (pims-ii:Cognition pims-ii:Action);
   rdfs:comment "Cognitive action, i.e., a cognition that is conducted/undertaken by an agent; the agent of a cognitive action is called its interpreter"^^xs:string.

pims-ii:CognitiveWorkflow a owl:Class;
   rdfs:label "CognitiveWorkflow"@en;
   rdfs:subClassOf pims-ii:CognitiveAction, pims-ii:CognitiveChain, pims-ii:PurposefulAction;
   owl:intersectionOf (pims-ii:CognitiveChain pims-ii:PurposefulAction);
   rdfs:comment "Cognitive workflow, i.e., a purposefully conducted cognitive chain"^^xs:string.

pims-ii:Communication a owl:Class;
   rdfs:label "Communication"@en;
   rdfs:subClassOf pims-ii:Cognition, [
      a owl:Restriction;
      owl:onProperty [owl:inverseOf pims-ii:isInterlocutorIn];
      owl:minCardinality 2
   ], [
      a owl:Restriction;
      owl:onProperty [owl:inverseOf pims-ii:isParticipantIn];
      owl:someValuesFrom pims-ii:ExpressiveAct
   ];
   rdfs:comment "Communication, i.e., a cognitive process wherein multiple interlocutors engage in an exchange with another; a communication involves at least one expressive act (with a well defined role, i.e. in terms of participation)"^^xs:string.

pims-ii:ExpressiveAct a owl:Class;
   rdfs:label "ExpressiveAct"@en;
   rdfs:subClassOf pims-ii:Communication, pims-ii:CognitiveAction, pims-ii:PurposefulAction, [
      a owl:Restriction;
      owl:onProperty [owl:inverseOf pims-ii:isSpeakerIn];
      owl:someValuesFrom pims-ii:Interlocutor
   ];
   rdfs:comment "Expressive act, i.e., a purposeful communication (e.g., a speech act or an analogous digital act of communicating) issued by its agent, the speaker (understood in a generalized sense, i.e., not limited to speech) - the purpose of the action consists of its illocutionary and perlocutionary intent"^^xs:string.

pims-ii:GoalDirectedAgent a owl:Class;
   rdfs:label "GoalDirectedAgent"@en;
   rdfs:subClassOf pims-ii:IntelligentAgent;
   owl:equivalentClass [
      a owl:Restriction;
      owl:onProperty [owl:inverseOf pims-ii:isGoalFor];
      owl:someValuesFrom pims-ii:Intention
   ];
   rdfs:comment "'Goal-directed agents are intelligent agents that have an internal representation of the goals they [tend to] achieve' (Conte, doi:10.1007/978-1-4614-1800-9_158, 2009)"@en;
   skos:scopeNote "Goal-directedness requires an explicit internal representation of intentions/objectives/goals of the agent; that is what distinguishes it from goal orientation. In PIMS-II, goal orientation is denoted by the relation isGoalOf (which does not require an internal mental representation of the goal), whereas conscious goal directedness is denoted by the relation isGoalFor."@en.

pims-ii:GoalOrientedAgent a owl:Class;
   rdfs:label "GoalOrientedAgent"@en;
   rdfs:subClassOf pims-ii:Agent;
   owl:equivalentClass [
      a owl:Restriction;
      owl:onProperty [owl:inverseOf pims-ii:isGoalOf];
      owl:someValuesFrom pims-ii:Intention
   ];
   rdfs:comment "Goal-oriented agent, i.e., an agent that exhibits the tendency 'to achieve a certain state of the world' (Conte, doi:10.1007/978-1-4614-1800-9_158, 2009)"@en;
   skos:scopeNote "A goal of a goal-oriented agent is a descriptor/representamen for that state of the world, and it is also a descriptor/representament for the agent itself. Goal orientation can emerge by a multitude of mechanisms, including natural selection. It does *not* require the agent to be consciously aware of its goals. In PIMS-II, goal orientation is denoted by the relation isGoalOf (which does not require an internal mental representation of the goal), whereas conscious goal directedness is denoted by the relation isGoalFor."@en.

pims-ii:IntelligentAgent a owl:Class;
   rdfs:label "IntelligentAgent"@en;
   rdfs:subClassOf pims-ii:GoalOrientedAgent;
   rdfs:comment "Intelligent agent, i.e., a goal-oriented agent that can internally make/hold claims (knowledge, beliefs, etc.). This requires the agent to have some kind of internal representation of its surroundings, and to store and process information about its surroundings. (Note that this does not require the agent to be queryable for its claims; for that purpose, use KnowledgeBase.)"^^xs:string.

pims-ii:Intention a owl:Class;
   rdfs:label "Intention"@en;
   rdfs:subClassOf pims-ii:Proposition;
   rdfs:comment "Intention, i.e., a proposition that constitutes an aim or goal"@en.

pims-ii:Interlocutor a owl:Class;
   rdfs:label "Interlocutor"@en;
   skos:altLabel "IO"@en;
   rdfs:subClassOf pims-ii:Agent;
   rdfs:comment "Interlocutor, i.e., an agent that can be addressed and is capable of addressing others in a communication process"@en.

pims-ii:KnowledgeBasedAgent a owl:Class;
   rdfs:label "KnowledgeBasedAgent"@en;
   rdfs:subClassOf pims-ii:IntelligentAgent, [
         a owl:Restriction;
         owl:onProperty [owl:inverseOf pims-ii:isMereologicallyConstitutiveOf];
         owl:someValuesFrom pims-ii:KnowledgeBase
      ];
   rdfs:comment "Knowledge-based agent, i.e., an intelligent agent that uses a knowledge base to store and process its opinions/claims/worldview"@en.

pims-ii:OptimizationProblem a owl:Class;
   rdfs:label "OptimizationProblem"@en;
   rdfs:subClassOf pims-ii:Intention;
   owl:equivalentClass [
      a owl:Restriction;
      owl:onProperty [owl:inverseOf pims-ii:isDesignParameterWithin];
      owl:someValuesFrom pims-ii:Conventional
   ], [
      a owl:Restriction;
      owl:onProperty [owl:inverseOf pims-ii:isOptimizationObjectiveWithin];
      owl:someValuesFrom pims-ii:Conventional
   ];
   rdfs:comment "Optimization problem, i.e., an intention expressed or expressible in terms of one or multiple objectives (objective space) and one or multiple design parameters (parameter space)"@en.

pims-ii:PurposefulAction a owl:Class;
    rdfs:label "PurposefulAction"@en;
    rdfs:subClassOf pims-ii:Action, [
       a owl:Restriction;
       owl:onProperty [owl:inverseOf pims-ii:isAgentIn];
       owl:allValuesFrom pims-ii:GoalDirectedAgent
    ], [
       a owl:Restriction;
       owl:onProperty [owl:inverseOf pims-ii:isAimIn];
       owl:someValuesFrom pims-ii:Intention
    ];
    rdfs:comment "Purposeful action, i.e., an action carried out with an aim of which its agent (hence, a goal-directed agent) is aware"@en.

pims-ii:RationalAgent a owl:Class;
   rdfs:label "RationalAgent"@en;
   rdfs:subClassOf pims-ii:IntelligentAgent, [
      a owl:Restriction;
      owl:onProperty [owl:inverseOf pims-ii:isGoalOf];
      owl:someValuesFrom pims-ii:OptimizationProblem
   ];
   owl:equivalentClass [
      a owl:Restriction;
      owl:onProperty [owl:inverseOf pims-ii:isPerformanceMeasureOf];
      owl:someValuesFrom pims-ii:Property
   ];
   rdfs:comment "A rational agent is an intelligent agent that exhibits rationality, i.e., a tendency toward maximizing a quantity: The performance measure of the agent."@en;
   skos:scopeNote "Similar as in the case of goal-orientation, rationality does *not* require the agent to be aware of its performance measure."@en.

###################################
# AGENCY AND TELEOLOGY: RELATIONS #
###################################

pims-ii:describesMethodAppliedIn a owl:ObjectProperty;
   rdfs:label "describesMethodAppliedIn"@en;
   skos:altLabel "\\v{R}"@en;
   rdfs:domain pims-ii:Articulation, [
      a owl:Restriction;
      owl:onProperty pims-ii:describesMethodEmployedBy;
      owl:someValuesFrom pims-ii:Agent
   ];
   rdfs:range pims-ii:Action;
   rdfs:subPropertyOf pims-ii:isRepresentamenFor;
   rdfs:comment "(x describesMethodAppliedIn y) means that x describes y in terms of the method that is employed"@en.

pims-ii:describesMethodEmployedBy a owl:ObjectProperty;
   rdfs:label "describesMethodEmployedBy"@en;
   rdfs:domain pims-ii:Articulation, [
      a owl:Restriction;
      owl:onProperty pims-ii:isRepresentamenFor;
      owl:someValuesFrom pims-ii:Object
   ];
   rdfs:range pims-ii:Agent;
   rdfs:subPropertyOf pims-ii:msIRHPIP;  # due to describesMethodEmployedBy == describesMethodAppliedIn (isAgentIn)^-
   owl:propertyChainAxiom (pims-ii:describesMethodAppliedIn [owl:inverseOf pims-ii:isAgentIn]);
   rdfs:comment "(x describesMethodEmployedBy y) means that the agent y follows a methodology described by x in carrying out an action"@en.

pims-ii:isAgentIn a owl:ObjectProperty;
   rdfs:label "isAgentIn"@en;
   skos:altLabel "\\ddot{P}_a"@en;
   rdfs:domain pims-ii:Agent;
   rdfs:range pims-ii:Action;
   rdfs:subPropertyOf pims-ii:isParticipantIn;
   rdfs:comment "(x isAgentIn y) means that x is *the* agent that conducts/undertakes the action y; n.b., an action has exactly one agent (which can be a straightforward item, or a plurality, a structure, or similar)"^^xs:string.

pims-ii:isAimIn a owl:ObjectProperty;
   rdfs:label "isAimIn"@en;
   skos:altLabel "R_\\alpha"@en;
   rdfs:domain pims-ii:Intention, [
      a owl:Restriction;
      owl:onProperty pims-ii:isGoalFor;
      owl:someValuesFrom pims-ii:GoalDirectedAgent
   ];
   rdfs:range pims-ii:Action;
   rdfs:subPropertyOf pims-ii:isRepresentamenFor;
   owl:propertyChainAxiom (pims-ii:isTelosInSteering [owl:inverseOf pims-ii:isActionInSteering]);
   owl:propertyChainAxiom (pims-ii:isResolutionInUndertaking [owl:inverseOf pims-ii:isActionInUndertaking]);
   rdfs:comment "(x isAimIn y) means that y is a purposeful action, and x is one of the aims followed by the agent of y by undertaking y"@en.

pims-ii:isGoalFor a owl:ObjectProperty;
   rdfs:label "isGoalFor"@en;
   skos:altLabel "\\dot{G}"@en;
   rdfs:domain pims-ii:Intention;
   rdfs:range pims-ii:GoalDirectedAgent;
   rdfs:subPropertyOf pims-ii:overlapsWith, pims-ii:isGoalOf;
   owl:propertyChainAxiom (pims-ii:isAimIn [owl:inverseOf pims-ii:isAgentIn]);
   owl:propertyChainAxiom (pims-ii:isTelosInSteering [owl:inverseOf pims-ii:isAgentIn]);
   owl:propertyChainAxiom (pims-ii:isResolutionInUndertaking [owl:inverseOf pims-ii:isAgentIn]);
   rdfs:comment "(x isGoalFor y) means that to the goal-directed agent y, the telos x represents something that is to be reached."@en;
   skos:example "In (x isGoalFor y), if the agent x wants to go to Paris, y is not physically the city of Paris as a 4D object, but rather the associated intention, i.e., a mental or textual representation of the agent achieving the objective and reaching Paris."@en;
   skos:scopeNote "A goal is both a representamen for a state of affairs desired by the agent and a representamen for the agent itself."@en.

pims-ii:isGoalOf a owl:ObjectProperty;
   rdfs:label "isGoalOf"@en;
   rdfs:domain pims-ii:Intention;
   rdfs:range pims-ii:GoalOrientedAgent;
   rdfs:subPropertyOf pims-ii:isRepresentamenFor;
   rdfs:comment "(x isGoalOf y) means that y is a goal-oriented agent with the tendency to work toward a state of affairs that is described/represented by y; accordingly, the goal y is also a representamen for the agent itself; this does *not* imply that the agent x is aware of pursuing y as a goal, or that y is somehow included in x as a mental representation - for that purpose, use the relation 'isGoalFor'"^^xs:string.

pims-ii:isInterpreterIn a owl:ObjectProperty;
   rdfs:label "isInterpreterIn"@en;
   rdfs:domain pims-ii:Agent;
   rdfs:range pims-ii:CognitiveAction;
   rdfs:subPropertyOf pims-ii:isAgentIn, pims-ii:isParticipantInCognition;
   rdfs:comment "(x isInterpreterIn y) means that x is the (unique) agent who conducts/undertakes the cognitive action y"^^xs:string.

pims-ii:isInterlocutorIn a owl:ObjectProperty;
   rdfs:label "isInterlocutorIn"@en;
   rdfs:domain pims-ii:Interlocutor;
   rdfs:range pims-ii:Communication;
   rdfs:subPropertyOf pims-ii:isParticipantIn;
   rdfs:comment "(x isInterlocutorIn y) means that x engages, jointly with other interlocutors, in the communication y"^^xs:string.

pims-ii:isListenerIn a owl:ObjectProperty;
   rdfs:label "isListenerIn"@en;
   rdfs:domain pims-ii:Interlocutor;
   rdfs:range pims-ii:ExpressiveAct;
   rdfs:subPropertyOf pims-ii:isInterlocutorIn;
   rdfs:comment "(x isListenerIn y) means that x is one of the interlocutors listening to the speaker's expressive act y"^^xs:string.

pims-ii:isPerformanceMeasureOf a owl:ObjectProperty;
   rdfs:label "isPerformanceMeasureOf"@en;
   rdfs:domain pims-ii:Property;
   rdfs:range pims-ii:RationalAgent;
   rdfs:subPropertyOf pims-ii:isRepresentamenFor;
   rdfs:comment "(x isPerformanceMeasureOf y) means that x is the single/unique performance measure of the rational agent y."@en;
   skos:scopeNote "This does not require the agent to be aware of its performance measure or to somehow contain it or an internal representation of it."@en.

pims-ii:isSpeakerIn a owl:ObjectProperty;
   rdfs:label "isSpeakerIn"@en;
   rdfs:domain pims-ii:Interlocutor;
   rdfs:range pims-ii:ExpressiveAct;
   rdfs:subPropertyOf pims-ii:isInterlocutorIn, pims-ii:isAgentIn;
   rdfs:comment "(x isSpeakerIn y) means that x is (the only) speaker in the expressive act y, where the role of the speaker is to be understood as that of an agent that conducts/undertakes the expressive act, i.e., it is not limited to vocal speech"@en.

pims-ii:isTargetPropertyIn a owl:ObjectProperty;
   rdfs:label "isTargetPropertyIn"@en;
   skos:altLabel "\\tilde{R}"@en;
   rdfs:domain pims-ii:Property;
   rdfs:range pims-ii:CognitiveAction;
   rdfs:subPropertyOf pims-ii:isRepresentamenFor;
   rdfs:comment "(x isTargetPropertyIn y) means that cognitive action x targets y as the property for which a value is to be determined by observation or by theoretical or computational methods"@en.

pims-ii:isToolIn a owl:ObjectProperty;
   rdfs:label "isToolIn"@en;
   skos:altLabel "\\ddot{P}_\\epsilon"@en;
   rdfs:range pims-ii:Action;
   rdfs:subPropertyOf pims-ii:isParticipantIn;
   rdfs:comment "(x isToolIn y) means that x is employed by an agent during the action y"@en.

#########################
# MODAL LOGIC: CONCEPTS #
#########################

pims-ii:AbsoluteLaw a owl:Class;
   rdfs:label "AbsoluteLaw"@en;
   rdfs:subClassOf pims-ii:Law;
   rdfs:comment "Absolute law, i.e., a law where the necessary entailment of the consequent(s) by the antecedent is expressed in terms of absolute logical/physical necessity"^^xs:string.

pims-ii:AbsoluteModalIRI a owl:Class;
   rdfs:label "AbsoluteModalIRI"@en;
   rdfs:subClassOf pims-ii:ModalIRI;
   rdfs:comment "Absolute modal IRI, i.e., the IRI of a relation that is defined by absolute necessity or possibility of another relation. Absolute necessity means 'logical or physical necessity', and absolute possibility means 'logical or physical possibility'. Accordingly, absolute modal relations do not require the specification of a modal context, i.e., the frame of reference for understanding what 'necessity' and 'possibility' mean does not need to be specified. "^^xs:string.

pims-ii:ContextualIRI a owl:Class;
   rdfs:label "ContextualIRI"@en;
   rdfs:subClassOf pims-ii:IRI;
   owl:disjointWith pims-ii:RelationalIRI;
   rdfs:comment "Contextual IRI, i.e., the internationalized resource identifier of a modal context, i.e., the frame of reference for a qualified-modal semiotic collective; that context defines how exactly necessity and possibility are to be understood"^^xs:string.

pims-ii:Law a owl:Class;
   rdfs:label "Law"@en;
   rdfs:subClassOf pims-ii:Rule;
   owl:disjointUnionOf (pims-ii:AbsoluteLaw pims-ii:QualifiedLaw);
   rdfs:comment "Law, i.e., a proposition consisting of an antecedent and one or multiple consequent(s) such that the antecedent is stated to necessarily imply the consequent(s)"^^xs:string.

pims-ii:ModalIRI a owl:Class;
   rdfs:label "ModalIRI"@en;
   rdfs:subClassOf pims-ii:RelationalIRI;
   owl:disjointUnionOf (pims-ii:AbsoluteModalIRI pims-ii:QualifiedModalIRI);
   rdfs:comment "Modal IRI, i.e., the IRI of a relation that is defined by (absolute or qualified) necessity or possibility of another relation"^^xs:string.

pims-ii:QualifiedLaw a owl:Class;
   rdfs:label "QualifiedLaw"@en;
   skos:altLabel "QL"@en;
   rdfs:subClassOf pims-ii:Law;
   owl:equivalentClass [
      a owl:Restriction;
      owl:onProperty [owl:inverseOf pims-ii:isContextWithinLaw];
      owl:someValuesFrom pims-ii:ContextualIRI
   ];
   rdfs:comment "Qualified law, i.e., a law where the necessary entailment of the consequent(s) by the antecedent is expressed in terms of qualified necessity, to be understood in terms of its modal context"^^xs:string.

pims-ii:QualifiedModalIRI a owl:Class;
   rdfs:label "QualifiedModalIRI"@en;
   rdfs:subClassOf pims-ii:ModalIRI;
   owl:equivalentClass [
      a owl:Restriction;
      owl:onProperty [owl:inverseOf pims-ii:isContextOfRelation];
      owl:someValuesFrom pims-ii:ContextualIRI
   ];
   rdfs:comment "Qualified modal IRI, i.e., the IRI of a relation that is defined by qualified necessity or possibility of another relation"@en;
   skos:scopeNote "Qualified modal relations require the specification of a modal context, i.e., a frame of reference for understanding what 'necessity' and 'possibility' exactly mean."@en.

##########################
# MODAL LOGIC: RELATIONS #
##########################

pims-ii:hasAbsoluteNecessityMode a owl:ObjectProperty;
   rdfs:label "hasAbsoluteNecessityMode"@en;
   rdfs:domain pims-ii:RelationalIRI;
   rdfs:range pims-ii:AbsoluteModalIRI;
   rdfs:subPropertyOf pims-ii:hasNecessityMode;
   rdfs:comment "(x hasAbsoluteNecessityMode y) means that x is a relational IRI and y is an absolute modal IRI for 'necessarily x'"@en.

pims-ii:hasAbsolutePossibilityMode a owl:ObjectProperty;
   rdfs:label "hasAbsolutePossibilityMode"@en;
   rdfs:domain pims-ii:RelationalIRI;
   rdfs:range pims-ii:AbsoluteModalIRI;
   rdfs:subPropertyOf pims-ii:hasPossibilityMode;
   rdfs:comment "(x hasAbsolutePossibilityMode y) means that x is a relational IRI and y is an absolute modal IRI for 'possibly x'"@en.

pims-ii:hasNecessityMode a owl:ObjectProperty;
   rdfs:label "hasNecessityMode"@en;
   rdfs:domain pims-ii:RelationalIRI;
   rdfs:range pims-ii:ModalIRI;
   rdfs:subPropertyOf pims-ii:isSemioticallyConstitutiveOf;
   rdfs:comment "(x hasNecessityMode y) means that x is a relational IRI and y is a modal IRI for 'necessarily x'"@en.

pims-ii:hasPossibilityMode a owl:ObjectProperty;
   rdfs:label "hasPossibilityMode"@en;
   rdfs:domain pims-ii:RelationalIRI;
   rdfs:range pims-ii:ModalIRI;
   rdfs:subPropertyOf pims-ii:isSemioticallyConstitutiveOf;
   rdfs:comment "(x hasPossibilityMode y) means that x is a relational IRI and y is a modal IRI for 'possibly x'"@en.

pims-ii:hasQualifiedNecessityMode a owl:ObjectProperty;
   rdfs:label "hasQualifiedNecessityMode"@en;
   rdfs:domain pims-ii:RelationalIRI;
   rdfs:range pims-ii:QualifiedModalIRI;
   rdfs:subPropertyOf pims-ii:hasNecessityMode;
   rdfs:comment "(x hasQualifiedNecessityMode y) means that x is a relational IRI and y is a qualified modal IRI for 'necessarily x'"@en.

pims-ii:hasQualifiedPossibilityMode a owl:ObjectProperty;
   rdfs:label "hasQualifiedPossibilityMode"@en;
   rdfs:domain pims-ii:RelationalIRI;
   rdfs:range pims-ii:QualifiedModalIRI;
   rdfs:subPropertyOf pims-ii:hasPossibilityMode;
   rdfs:comment "(x hasQualifiedPossibilityMode y) means that x is a relational IRI and y is a qualified modal IRI for 'possibly x'"@en.

pims-ii:isContextOfRelation a owl:ObjectProperty;
   rdfs:label "isContextOfRelation"@en;
   rdfs:domain pims-ii:ContextualIRI;
   rdfs:range pims-ii:QualifiedModalIRI;
   rdfs:subPropertyOf pims-ii:isSemioticallyConstitutiveOf;
   rdfs:comment "(x isContextOfRelation y) means that x is an IRI for the modal context of qualified possibility/necessity in the relative modal IRI y"@en.

pims-ii:isContextWithinLaw a owl:ObjectProperty;
   rdfs:label "isContextWithinLaw"@en;
   rdfs:domain pims-ii:ContextualIRI;
   rdfs:range pims-ii:QualifiedLaw;
   rdfs:subPropertyOf pims-ii:isSemioticallyConstitutiveOf;
   rdfs:comment "(x isContextWithinLaw y) means that x is an IRI for the modal context of relatively necessary implication in the relative law y"@en.

############################################################################
# MULTI-ARGUMENT PREDICATES IMPLEMENTED AS RELATIONS WITH RDF:LIST OBJECTS #
############################################################################

rdf:List
   skos:scopeNote "Syntactic construct (x1 x2 x3 x4) used within the resource description framework (RDF) for a list"@en;
   rdfs:comment "the first element is related to the list by rdf:first, the second by (rdf:rest o rdf:first), the third by (rdf:rest o rdf:rest o rdf:first), and so on; where the list ends, it is related by rdf:rest to rdf:nil"@en;
   skos:example "See also: https://ontola.io/blog/ordered-data-in-rdf/"@en.
rdf:first
   rdfs:domain rdf:List;
   rdfs:comment "relates a rdf:List to its first element"@en;
   skos:example "e.g., if L = (x y z), this would be 'L rdf:first x'"@en.
rdf:rest
   rdfs:domain rdf:List;
   rdfs:comment "relates a rdf:List to the part that remains when its first element is removed"@en;
   skos:example "e.g., if L = (x y z), this would be 'L rdf:rest (y z)'; if a list has only one element, the rest is rdf:nil, e.g., if L = (x), such that 'L rdf:first x', this would be 'L rdf:rest rdf:nil'"@en.

pims-ii:isRelatedToList a owl:ObjectProperty;
   rdfs:label "isRelatedToList"@en;
   rdfs:range rdf:List;
   rdfs:comment "Top property for multi-argument predicates that are implemented as 'x isRelatedToList (y1 y2 ... yn)', i.e., such that the object is an rdf:List"@en.

pims-ii:isFusionOf a owl:ObjectProperty;
   rdfs:label "isFusionOf"@en;
   skos:altLabel "\\sigma"@en;
   rdfs:subPropertyOf pims-ii:isRelatedToList;
   rdfs:range rdf:List;
   rdfs:comment "x isFusionOf (y1 y2 ... yn) means that x is the spatiotemporal union (i.e., fusion) of all the elements included in the list (y1 y2 ... yn)"@en.
rdf:List a rdfs:Class.
pims-ii:isImproperPartOf owl:propertyChainAxiom ([owl:inverseOf rdf:first] [owl:inverseOf pims-ii:isFusionOf]).
pims-ii:isProperPartOf owl:propertyChainAxiom ([owl:inverseOf rdf:first] [owl:inverseOf rdf:rest] [owl:inverseOf pims-ii:isFusionOf]).
pims-ii:isProperPartOf owl:propertyChainAxiom ([owl:inverseOf rdf:first] [owl:inverseOf rdf:rest] [owl:inverseOf rdf:rest] [owl:inverseOf pims-ii:isFusionOf]).

pims-ii:isTriadOf a owl:ObjectProperty;
   rdfs:label "isTriadOf"@en;
   skos:altLabel "3"@en;
   rdfs:domain pims-ii:TriadicCognition;
   rdfs:range rdf:List;
   rdfs:subPropertyOf pims-ii:isRelatedToList;
   rdfs:comment "'x isTriadOf (e1 e2 e3)' is a shorthand for 'e1 isFirstElementIn x; e2 isSecondElementIn x; e3 isThirdElementIn x'"@en.
rdf:List a rdfs:Class.
pims-ii:isFirstElementIn owl:propertyChainAxiom ([owl:inverseOf rdf:first] [owl:inverseOf pims-ii:isTriadOf]).
pims-ii:isSecondElementIn owl:propertyChainAxiom ([owl:inverseOf rdf:first] [owl:inverseOf rdf:rest] [owl:inverseOf pims-ii:isTriadOf]).
pims-ii:isThirdElementIn owl:propertyChainAxiom ([owl:inverseOf rdf:first] [owl:inverseOf rdf:rest] [owl:inverseOf rdf:rest] [owl:inverseOf pims-ii:isTriadOf]).

################################
# EPISTEMIC METADATA: CONCEPTS #
################################

pims-ii:AbstractModelPropertyClaim a owl:Class;
   rdfs:label "AbstractModelPropertyClaim"@en;
   skos:altLabel "AMPC"@en;
   rdfs:subClassOf pims-ii:ModelPropertyClaim;
   rdfs:comment "Abstract model property claim (CMPC), i.e., a model property claim that is not immediately applied to the corresponding property of a real physical system"@en.

pims-ii:ConceptualKnowledgeClaim a owl:Class;
   rdfs:label "ConceptualKnowledgeClaim"@en;
   skos:altLabel "CKC"@en;
   rdfs:subClassOf pims-ii:KnowledgeClaim;
   owl:disjointWith pims-ii:PropertyClaim;
   rdfs:comment "Conceptual knowledge claim (CKC), i.e., a knowledge claim establishing the ontological status of a lexeme"@en.

pims-ii:ConcreteModelPropertyClaim a owl:Class;
   rdfs:label "ConcretePropertyClaim"@en;
   skos:altLabel "CMPC"@en;
   rdfs:subClassOf pims-ii:ModelPropertyClaim, pims-ii:PhysicalPropertyClaim;
   rdfs:comment "Concrete model property claim (CMPC), i.e., a model property claim that is immediately also applied to the corresponding property of a real physical system"@en.

pims-ii:EPRC a owl:Class;
   rdfs:label "EPRC"@en;
   rdfs:subClassOf pims-ii:ExactAgreementReproducibilityClaim, pims-ii:ProvenanceConsciousReproducibilityClaim;
   owl:intersectionOf (pims-ii:ExactAgreementReproducibilityClaim pims-ii:ProvenanceConsciousReproducibilityClaim);
   rdfs:comment "EPRC, i.e., an exact-agreement provenance-conscious reproducibility claim"@en.

pims-ii:EPTRC a owl:Class;
   rdfs:label "EPTRC"@en;
   rdfs:subClassOf pims-ii:EPRC, pims-ii:ETRC, pims-ii:PTRC;
   owl:intersectionOf (pims-ii:ExactAgreementReproducibilityClaim pims-ii:ProvenanceConsciousReproducibilityClaim pims-ii:TeamChangeReproducibilityClaim);
   rdfs:comment "EPTRC, i.e., an exact-agreement provenance-conscious team-change reproducibility claim"@en.

pims-ii:ETRC a owl:Class;
   rdfs:label "ETRC"@en;
   rdfs:subClassOf pims-ii:ExactAgreementReproducibilityClaim, pims-ii:TeamChangeReproducibilityClaim;
   owl:intersectionOf (pims-ii:ExactAgreementReproducibilityClaim pims-ii:TeamChangeReproducibilityClaim);
   rdfs:comment "ETRC, i.e., an exact-agreement team-change reproducibility claim"@en.

pims-ii:ExactAgreementReproducibilityClaim a owl:Class;
   rdfs:label "ExactAgreementReproducibilityClaim"@en;
   skos:altLabel "ERC"@en;
   rdfs:subClassOf pims-ii:ReproducibilityClaim;
   rdfs:comment "Exact-agreement reproducibility claim (ERC), i.e., a reproducibility claim obtained as an outcome of an attempt at obtaining exactly the same outcome as the original study"@en;
   skos:scopeNote "The criterion for an ERC is that it has no outcome paradata - all the outcome metadata are orthodata"@en.

pims-ii:KnowledgeClaim a owl:Class;
   rdfs:label "KnowledgeClaim"@en;
   skos:altLabel "KC"@en;
   rdfs:subClassOf pims-ii:Claim, [
      a owl:Restriction;
      owl:onProperty pims-ii:isInterpretantIn;
      owl:someValuesFrom pims-ii:Semiosis
   ], [
      a owl:Restriction;
      owl:onProperty pims-ii:hasSubjectMatter;
      owl:someValuesFrom pims-ii:Question
   ];
   owl:disjointWith pims-ii:ValidityClaim;
   rdfs:comment "Knowledge claim (KC), i.e., a claim about something with respect to its knowledge status"@en;
   skos:scopeNote "The subject matter of a knowledge claim must be a (single) question, namely the one that is answered by the claim; in particular, therefore, its subject matter may not be a sum (plurality) of unrelated questions - in such a case, split it up into multiple independent knowledge claims"@en;
   skos:scopeNote "A knowledge claim states 'what data mean,' i.e., in what way some agent of the academic discourse has given some data an interpretation as constituting knowledge. A knowledge claim asserts what was found from research data: 'Research data δ made agent a know φ,' which can be expanded as 'the interpreation of research data δ by interpreter a yielded the knowledge claim φ as an interpretant.'"@en.

pims-ii:ModelPropertyClaim a owl:Class;
   rdfs:label "PropertyClaim"@en;
   skos:altLabel "MPC"@en;
   rdfs:subClassOf pims-ii:PropertyClaim;
   owl:disjointUnionOf (pims-ii:AbstractModelPropertyClaim pims-ii:ConcreteModelPropertyClaim);
   rdfs:comment "Model property claim (MPC), i.e., a PC concerning a property of a model"@en;
   skos:scopeNote "Claim expressed through a PC: 'From data δ, property p of object o under conditions c was found by agent a to have the value v'"@en.

pims-ii:NegativeKnowledgeClaim a owl:Class;
   rdfs:label "NegativeKnowledgeClaim"@en;
   skos:altLabel "NKC"@en;
   rdfs:subClassOf pims-ii:KnowledgeClaim;
   rdfs:comment "Negative knowledge claim (NKC), i.e., a knowledge claim that expresses what we don't know, a gap or limitation of our knowledge"@en.
   
pims-ii:PhysicalPropertyClaim a owl:Class;
   rdfs:label "PropertyClaim"@en;
   skos:altLabel "PPC"@en;
   rdfs:subClassOf pims-ii:PropertyClaim;
   rdfs:comment "Physical property claim (PPC), i.e., a PC concerning a property of a physical system"@en;
   skos:scopeNote "Claim expressed through a PC: 'From data δ, property p of object o under conditions c was found by agent a to have the value v'"@en.

pims-ii:ProofBasedValidityClaim a owl:Class;
   rdfs:label "ProofBasedValidityClaim"@en;
   skos:altLabel "PVC"@en;
   rdfs:subClassOf pims-ii:ValidityClaim;
   owl:disjointWith pims-ii:ReproducibilityClaim, pims-ii:TestBasedValidityClaim;
   rdfs:comment "Proof-based validity claim (PVC), i.e., a validity claim obtained by formal verification, i.e., by deductive logical and mathematical reasoning"@en.

pims-ii:PropertyClaim a owl:Class;
   rdfs:label "PropertyClaim"@en;
   skos:altLabel "PC"@en;
   rdfs:subClassOf pims-ii:KnowledgeClaim;
   owl:disjointWith pims-ii:ConceptualKnowledgeClaim;
   rdfs:comment "Property claim (PC), i.e., a knowledge claim concerning a property"@en;
   skos:scopeNote "Claim expressed through a PC: 'From data δ, property p of object o under conditions c was found by agent a to have the value v'"@en.

pims-ii:ProvenanceConsciousReproducibilityClaim a owl:Class;
   rdfs:label "ProvenanceConsciousReproducibilityClaim"@en;
   skos:altLabel "PRC"@en;
   rdfs:subClassOf pims-ii:ReproducibilityClaim;
   rdfs:comment "Provenance-conscious reproducibility claim (PRC), i.e., a reproducibility claim obtained from an attempt that was subject to the requirement to retain the original research process or aspects of it"@en;
   skos:scopeNote "The criterion for a PRC is that there are provenance orthodata, not only provenance paradata"@en.

pims-ii:PTRC a owl:Class;
   rdfs:label "PTRC"@en;
   rdfs:subClassOf pims-ii:ProvenanceConsciousReproducibilityClaim, pims-ii:TeamChangeReproducibilityClaim;
   owl:intersectionOf (pims-ii:ProvenanceConsciousReproducibilityClaim pims-ii:TeamChangeReproducibilityClaim);
   rdfs:comment "PTRC, i.e., a provenance-conscious team-change reproducibility claim"@en.

pims-ii:ReproducibilityClaim a owl:Class;
   rdfs:label "ReproducibilityClaim"@en;
   skos:altLabel "RC"@en;
   rdfs:subClassOf pims-ii:QualifiedLaw, pims-ii:ValidityClaim;
   owl:disjointWith pims-ii:ProofBasedValidityClaim, pims-ii:TestBasedValidityClaim;
   rdfs:comment "Reproducibility claim (RC), i.e., a validity claim obtained as an outcome of a reproduction attempt/reproducibility study"@en.

pims-ii:TeamChangeReproducibilityClaim a owl:Class;
   rdfs:label "TeamChangeReproducibilityClaim"@en;
   skos:altLabel "TRC"@en;
   rdfs:subClassOf pims-ii:ReproducibilityClaim;
   rdfs:comment "Team-change reproducibility claim (TRC), i.e., a reproducibility claim obtained as an outcome of a reproducibility study conducted by an independent team"@en;
   skos:scopeNote "Criterion: Interpreter(s) disjoint with the interpreter(s) from the original research process"@en.

pims-ii:TestBasedValidityClaim a owl:Class;
   rdfs:label "TestBasedValidityClaim"@en;
   skos:altLabel "TVC"@en;
   rdfs:subClassOf pims-ii:ValidityClaim;
   owl:disjointWith pims-ii:ProofBasedValidityClaim, pims-ii:ReproducibilityClaim;
   rdfs:comment "Test-based validity claim (TVC), i.e., a validity claim obtained from validation or testing"@en;
   skos:scopeNote "Validation and testing are an integral part of the activity by which the validated knowledge claim and/or the associated data are produced, as opposed to reproducibility studies which are done subsequently in a separate activity"@en.

pims-ii:ValidityClaim a owl:Class;
   rdfs:label "ValidityClaim"@en;
   skos:altLabel "VC"@en;
   rdfs:subClassOf pims-ii:Claim, [
      a owl:Restriction;
      owl:onProperty pims-ii:isAbout;
      owl:someValuesFrom pims-ii:Claim
   ];
   owl:equivalentClass [
      a owl:Restriction;
      owl:onProperty pims-ii:isValidationOutcomeIn;
      owl:someValuesFrom pims-ii:Validation
   ];
   owl:disjointWith pims-ii:KnowledgeClaim;
   rdfs:comment "Validity claim (VC), i.e., a claim about another claim, saying something about that claim's (in-)accuracy or somebody's (dis-)trust in the claim"@en.

#################################
# EPISTEMIC METADATA: RELATIONS #
#################################

pims-ii:affirmsCognition a owl:ObjectProperty;
   rdfs:label "affirmsCognition"@en;
   skos:altLabel "\\hat{A}_\\kappa"@en;
   rdfs:range pims-ii:Cognition;
   rdfs:subPropertyOf pims-ii:isAbout;
   owl:propertyChainAxiom (pims-ii:providesJustification pims-ii:isJustificationFor);
   rdfs:comment "(x affirmsCognition y) means that x is about the cognition y, affirming its validity"@en.

pims-ii:hasSubjectMatter a owl:ObjectProperty, owl:FunctionalProperty;
   rdfs:label "hasSubjectMatter"@en;
   skos:altLabel "A"@en;
   rdfs:range [owl:unionOf (pims-ii:Topical pims-ii:TopicalSum)];
   rdfs:subPropertyOf pims-ii:isAbout;
   skos:scopeNote "following Yablo, there is such a thing as *the* subject matter of something, in other words, hasSubjectMatter is a functional property"@en;
   rdfs:comment "(x hasSubjectMatter y) means that x is a proposition or articulation that addresses the topic or sum (i.e., plurality) of topics y, i.e., that has y as its subject matter"@en.

pims-ii:isAbout a owl:ObjectProperty;
   rdfs:label "isAbout"@en;
   skos:altLabel "\\hat{A}"@en;
   rdfs:domain [owl:unionOf (pims-ii:Articulation pims-ii:Proposition)];
   rdfs:subPropertyOf pims-ii:isRepresentamenFor;
   rdfs:comment "(x isAbout y) means that x is a proposition and y is the object that x is related to by aboutness"@en;
   skos:scopeNote "it can make sense to use a structure or plurality to indicate the complex ways in which x can be about a combination of interrelated objects"@en.

pims-ii:isOrthodataWithin a owl:ObjectProperty;
   rdfs:label "isOrthodataWithin"@en;
   skos:altLabel "\\v{C}_\\perp"@en;
   rdfs:domain pims-ii:DigitalArticulation;
   rdfs:range pims-ii:Rule;
   rdfs:subPropertyOf pims-ii:isSemioticallyConstitutiveOf;
   rdfs:comment "(x isOrthodataWithin y) means that x articulates a substantial aspect of either the antecedent or the consequent side of the rule y"@en.

pims-ii:isParadataWithin a owl:ObjectProperty;
   rdfs:label "isParadataWithin"@en;
   skos:altLabel "\\v{C}_\\parallel"@en;
   rdfs:domain pims-ii:DigitalArticulation;
   rdfs:range pims-ii:Rule;
   rdfs:subPropertyOf pims-ii:isSemioticallyConstitutiveOf;
   rdfs:comment "(x isParadataWithin y) means that x articulates something explicitly said to be unsubstantial to the rule y, and thereby semiotically constitutive of it, e.g., by a mechanism of logical subtraction"@en.

pims-ii:isResultOf a owl:ObjectProperty;
   rdfs:label "isResultOf"@en;
   skos:altLabel "\\bar{R}"@en;
   rdfs:domain [
      a owl:Restriction;
      owl:onProperty pims-ii:isInterpretantIn;
      owl:someValuesFrom pims-ii:Interpretation
   ];
   rdfs:range pims-ii:Cognition;
   rdfs:subPropertyOf pims-ii:isParticipantInCognition;
   rdfs:comment "(x isResultOf y) if x is an outcome/result of the cognitive process y"@en;
   skos:scopeNote "an outcome/result of a cognition must occur in the role of the interpretant somewhere within that cognition"@en;
   skos:example "outcomes/results of a research process can be a research data set, one or multiple knowledge claims, or some combination thereof such as a FAIR digital object"@en.

pims-ii:isTopicalFactorIn a owl:ObjectProperty;
   rdfs:label "isTopicalFactorIn"@en;
   skos:altLabel "\\v{C}_T"@en;
   rdfs:domain [owl:unionOf (pims-ii:Topical pims-ii:TopicalSum)];
   rdfs:range pims-ii:TopicalProduct;
   rdfs:subPropertyOf pims-ii:isSemioticallyConstitutiveOf;
   rdfs:comment "(x isTopicalFactorIn y) means that x is combined with other subtopics into the topical proposition y, such that x and the other subtopics are not just standing beside each other, but exhibiting some meaningful interaction"@en.

pims-ii:isTopicalSummandIn a owl:ObjectProperty;
   rdfs:label "isTopicalSummandIn"@en;
   skos:altLabel "\\lhd_T"@en;
   rdfs:domain pims-ii:Topical;
   rdfs:range pims-ii:TopicalSum;
   rdfs:subPropertyOf pims-ii:isMemberOfPlurality;
   rdfs:comment "(x isTopicalSummandIn y) means that x is one of the topics contained in y, a collection of topics that are not immediately closely related to each other"@en;
   skos:scopeNote "If multiple topics are combined in a way that relates them closely to each other, with some meaningful interaction between them, the relation isTopicalFactorIn should be used, and the whole should then be a topical product, not a topical sum".
